<?xml version="1.0"?>
<rdf:RDF xmlns="http://www.w3id.org/issi/"
     xml:base="http://www.w3id.org/issi/"
     xmlns:dc="http://purl.org/dc/elements/1.1/"
     xmlns:org="http://www.w3.org/ns/org#"
     xmlns:owl="http://www.w3.org/2002/07/owl#"
     xmlns:rdf="http://www.w3.org/1999/02/22-rdf-syntax-ns#"
     xmlns:xml="http://www.w3.org/XML/1998/namespace"
     xmlns:xsd="http://www.w3.org/2001/XMLSchema#"
     xmlns:foaf="http://xmlns.com/foaf/0.1/"
     xmlns:rdfs="http://www.w3.org/2000/01/rdf-schema#"
     xmlns:skos="http://www.w3.org/2004/02/skos/core#"
     xmlns:vann="http://purl.org/vocab/vann/"
     xmlns:iirds="http://iirds.tekom.de/iirds#"
     xmlns:terms="http://purl.org/dc/terms/"
     xmlns:schema="http://schema.org/"
     xmlns:wgs84_pos="http://www.w3.org/2003/01/geo/wgs84_pos#">
    <owl:Ontology rdf:about="http://www.w3id.org/issi/">
        <owl:versionIRI rdf:resource="http://www.w3id.org/issi/0.0.1"/>
        <owl:imports rdf:resource="http://example.org/mto/mtconnectmachinedata#"/>
        <owl:imports rdf:resource="http://www.w3.org/2006/time#2016"/>
        <owl:imports rdf:resource="http://www.w3.org/2006/vcard/ns"/>
        <owl:imports rdf:resource="http://www.w3.org/ns/org#"/>
        <dc:title xml:lang="en">Intelligent Service Support for Industry 4.0</dc:title>
        <dc:title xml:lang="de">Intelligente Service-Unterstützung für Industrie 4.0</dc:title>
        <terms:creator>Edward Dinu</terms:creator>
        <terms:creator>Raed Ben Younes</terms:creator>
        <rdfs:label xml:lang="en">Intelligent Service Support (Industry 4.0)</rdfs:label>
        <rdfs:label xml:lang="de">Intelligente Service-Unterstützung (Industrie 4.0)</rdfs:label>
        <owl:versionInfo>0.0.1</owl:versionInfo>
    </owl:Ontology>
    


    <!-- 
    ///////////////////////////////////////////////////////////////////////////////////////
    //
    // Annotation properties
    //
    ///////////////////////////////////////////////////////////////////////////////////////
     -->

    


    <!-- http://iirds.tekom.de/iirds#dateOfCreation -->

    <owl:AnnotationProperty rdf:about="http://iirds.tekom.de/iirds#dateOfCreation">
        <rdfs:subPropertyOf rdf:resource="http://purl.org/dc/terms/created"/>
        <rdfs:range rdf:resource="http://www.w3.org/2001/XMLSchema#dateTimeStamp"/>
        <rdfs:domain rdf:resource="http://iirds.tekom.de/iirds#InformationUnit"/>
    </owl:AnnotationProperty>
    


    <!-- http://iirds.tekom.de/iirds#description -->

    <owl:AnnotationProperty rdf:about="http://iirds.tekom.de/iirds#description">
        <rdfs:subPropertyOf rdf:resource="http://purl.org/dc/terms/description"/>
        <rdfs:range rdf:resource="http://www.w3.org/2000/01/rdf-schema#Literal"/>
        <rdfs:domain rdf:resource="http://iirds.tekom.de/iirds#iirdsDomainEntity"/>
    </owl:AnnotationProperty>
    


    <!-- http://iirds.tekom.de/iirds#format -->

    <owl:AnnotationProperty rdf:about="http://iirds.tekom.de/iirds#format">
        <rdfs:subPropertyOf rdf:resource="http://purl.org/dc/terms/format"/>
        <rdfs:range rdf:resource="http://www.w3.org/2000/01/rdf-schema#Literal"/>
        <rdfs:domain rdf:resource="http://iirds.tekom.de/iirds#Rendition"/>
    </owl:AnnotationProperty>
    


    <!-- http://iirds.tekom.de/iirds#has-abstract -->

    <owl:AnnotationProperty rdf:about="http://iirds.tekom.de/iirds#has-abstract">
        <rdfs:subPropertyOf rdf:resource="http://purl.org/dc/terms/abstract"/>
    </owl:AnnotationProperty>
    


    <!-- http://iirds.tekom.de/iirds#has-event-code -->

    <owl:AnnotationProperty rdf:about="http://iirds.tekom.de/iirds#has-event-code"/>
    


    <!-- http://iirds.tekom.de/iirds#has-event-type -->

    <owl:AnnotationProperty rdf:about="http://iirds.tekom.de/iirds#has-event-type"/>
    


    <!-- http://iirds.tekom.de/iirds#has-subject -->

    <owl:AnnotationProperty rdf:about="http://iirds.tekom.de/iirds#has-subject">
        <rdfs:subPropertyOf rdf:resource="http://purl.org/dc/terms/subject"/>
        <rdfs:range rdf:resource="http://iirds.tekom.de/iirds#InformationSubject"/>
    </owl:AnnotationProperty>
    


    <!-- http://iirds.tekom.de/iirds#identifier -->

    <owl:AnnotationProperty rdf:about="http://iirds.tekom.de/iirds#identifier">
        <rdfs:subPropertyOf rdf:resource="http://purl.org/dc/terms/identifier"/>
        <rdfs:range rdf:resource="http://www.w3.org/2000/01/rdf-schema#Literal"/>
        <rdfs:domain rdf:resource="http://iirds.tekom.de/iirds#Identity"/>
    </owl:AnnotationProperty>
    


    <!-- http://iirds.tekom.de/iirds#is-replacement-of -->

    <owl:AnnotationProperty rdf:about="http://iirds.tekom.de/iirds#is-replacement-of">
        <rdfs:subPropertyOf rdf:resource="http://purl.org/dc/terms/replaces"/>
        <rdfs:range rdf:resource="http://iirds.tekom.de/iirds#InformationUnit"/>
    </owl:AnnotationProperty>
    


    <!-- http://iirds.tekom.de/iirds#is-version-of -->

    <owl:AnnotationProperty rdf:about="http://iirds.tekom.de/iirds#is-version-of">
        <rdfs:subPropertyOf rdf:resource="http://purl.org/dc/terms/isVersionOf"/>
        <rdfs:range rdf:resource="http://iirds.tekom.de/iirds#InformationObject"/>
    </owl:AnnotationProperty>
    


    <!-- http://iirds.tekom.de/iirds#language -->

    <owl:AnnotationProperty rdf:about="http://iirds.tekom.de/iirds#language">
        <rdfs:subPropertyOf rdf:resource="http://purl.org/dc/terms/language"/>
        <rdfs:range rdf:resource="http://www.w3.org/2000/01/rdf-schema#Literal"/>
        <rdfs:domain rdf:resource="http://iirds.tekom.de/iirds#InformationUnit"/>
    </owl:AnnotationProperty>
    


    <!-- http://iirds.tekom.de/iirds#revision -->

    <owl:AnnotationProperty rdf:about="http://iirds.tekom.de/iirds#revision">
        <rdfs:subPropertyOf rdf:resource="http://purl.org/dc/terms/title"/>
        <rdfs:range rdf:resource="http://www.w3.org/2000/01/rdf-schema#Literal"/>
        <rdfs:domain rdf:resource="http://iirds.tekom.de/iirds#InformationUnit"/>
    </owl:AnnotationProperty>
    


    <!-- http://iirds.tekom.de/iirds#rights -->

    <owl:AnnotationProperty rdf:about="http://iirds.tekom.de/iirds#rights">
        <rdfs:subPropertyOf rdf:resource="http://purl.org/dc/elements/1.1/rights"/>
        <rdfs:range rdf:resource="http://www.w3.org/2000/01/rdf-schema#Literal"/>
        <rdfs:domain rdf:resource="http://iirds.tekom.de/iirds#InformationUnit"/>
    </owl:AnnotationProperty>
    


    <!-- http://iirds.tekom.de/iirds#title -->

    <owl:AnnotationProperty rdf:about="http://iirds.tekom.de/iirds#title">
        <rdfs:subPropertyOf rdf:resource="http://purl.org/dc/terms/title"/>
        <rdfs:range rdf:resource="http://www.w3.org/2000/01/rdf-schema#Literal"/>
        <rdfs:domain rdf:resource="http://iirds.tekom.de/iirds#InformationUnit"/>
    </owl:AnnotationProperty>
    


    <!-- http://purl.org/dc/elements/1.1/date -->

    <owl:AnnotationProperty rdf:about="http://purl.org/dc/elements/1.1/date"/>
    


    <!-- http://purl.org/dc/elements/1.1/description -->

    <owl:AnnotationProperty rdf:about="http://purl.org/dc/elements/1.1/description"/>
    


    <!-- http://purl.org/dc/elements/1.1/rights -->

    <owl:AnnotationProperty rdf:about="http://purl.org/dc/elements/1.1/rights"/>
    


    <!-- http://purl.org/dc/elements/1.1/title -->

    <owl:AnnotationProperty rdf:about="http://purl.org/dc/elements/1.1/title"/>
    


    <!-- http://purl.org/dc/terms/abstract -->

    <owl:AnnotationProperty rdf:about="http://purl.org/dc/terms/abstract"/>
    


    <!-- http://purl.org/dc/terms/description -->

    <owl:AnnotationProperty rdf:about="http://purl.org/dc/terms/description"/>
    


    <!-- http://purl.org/dc/terms/format -->

    <owl:AnnotationProperty rdf:about="http://purl.org/dc/terms/format"/>
    


    <!-- http://purl.org/dc/terms/identifier -->

    <owl:AnnotationProperty rdf:about="http://purl.org/dc/terms/identifier"/>
    


    <!-- http://purl.org/dc/terms/language -->

    <owl:AnnotationProperty rdf:about="http://purl.org/dc/terms/language"/>
    


    <!-- http://purl.org/dc/terms/replaces -->

    <owl:AnnotationProperty rdf:about="http://purl.org/dc/terms/replaces"/>
    


    <!-- http://purl.org/dc/terms/subject -->

    <owl:AnnotationProperty rdf:about="http://purl.org/dc/terms/subject"/>
    


    <!-- http://purl.org/dc/terms/title -->

    <owl:AnnotationProperty rdf:about="http://purl.org/dc/terms/title"/>
    


    <!-- http://schema.org/domainIncludes -->

    <owl:AnnotationProperty rdf:about="http://schema.org/domainIncludes"/>
    


    <!-- http://schema.org/rangeIncludes -->

    <owl:AnnotationProperty rdf:about="http://schema.org/rangeIncludes"/>
    


    <!-- http://www.w3.org/2003/01/geo/wgs84_pos#alt -->

    <owl:AnnotationProperty rdf:about="http://www.w3.org/2003/01/geo/wgs84_pos#alt">
        <rdfs:comment>The WGS84 altitude of a SpatialThing (decimal meters 
above the local reference ellipsoid).</rdfs:comment>
        <rdfs:label>altitude</rdfs:label>
        <rdfs:domain rdf:resource="http://www.w3.org/2003/01/geo/wgs84_pos#SpatialThing"/>
    </owl:AnnotationProperty>
    


    <!-- http://www.w3.org/2003/01/geo/wgs84_pos#lat -->

    <owl:AnnotationProperty rdf:about="http://www.w3.org/2003/01/geo/wgs84_pos#lat">
        <rdfs:comment>The WGS84 latitude of a SpatialThing (decimal degrees).</rdfs:comment>
        <rdfs:label>latitude</rdfs:label>
        <rdfs:domain rdf:resource="http://www.w3.org/2003/01/geo/wgs84_pos#SpatialThing"/>
    </owl:AnnotationProperty>
    


    <!-- http://www.w3.org/2003/01/geo/wgs84_pos#location -->

    <owl:AnnotationProperty rdf:about="http://www.w3.org/2003/01/geo/wgs84_pos#location">
        <rdfs:subPropertyOf rdf:resource="http://xmlns.com/foaf/0.1/based_near"/>
        <rdfs:range rdf:resource="http://www.w3.org/2003/01/geo/wgs84_pos#SpatialThing"/>
    </owl:AnnotationProperty>
    


    <!-- http://www.w3.org/2003/01/geo/wgs84_pos#long -->

    <owl:AnnotationProperty rdf:about="http://www.w3.org/2003/01/geo/wgs84_pos#long">
        <rdfs:comment>The WGS84 longitude of a SpatialThing (decimal degrees).</rdfs:comment>
        <rdfs:label>longitude</rdfs:label>
        <rdfs:domain rdf:resource="http://www.w3.org/2003/01/geo/wgs84_pos#SpatialThing"/>
    </owl:AnnotationProperty>
    


    <!-- http://xmlns.com/foaf/0.1/based_near -->

    <owl:AnnotationProperty rdf:about="http://xmlns.com/foaf/0.1/based_near"/>
    


    <!-- 
    ///////////////////////////////////////////////////////////////////////////////////////
    //
    // Object Properties
    //
    ///////////////////////////////////////////////////////////////////////////////////////
     -->

    


    <!-- http://iirds.tekom.de/iirds#has-abstract -->

    <owl:ObjectProperty rdf:about="http://iirds.tekom.de/iirds#has-abstract">
        <rdfs:subPropertyOf rdf:resource="http://iirds.tekom.de/iirds#iirdsRelationConcept"/>
        <rdfs:domain rdf:resource="http://iirds.tekom.de/iirds#InformationUnit"/>
    </owl:ObjectProperty>
    


    <!-- http://iirds.tekom.de/iirds#has-component -->

    <owl:ObjectProperty rdf:about="http://iirds.tekom.de/iirds#has-component">
        <rdfs:subPropertyOf rdf:resource="http://iirds.tekom.de/iirds#iirdsRelationConcept"/>
        <rdfs:domain rdf:resource="http://iirds.tekom.de/iirds#Component"/>
        <rdfs:range rdf:resource="http://iirds.tekom.de/iirds#Component"/>
    </owl:ObjectProperty>
    


    <!-- http://iirds.tekom.de/iirds#has-content-lifecycle-status -->

    <owl:ObjectProperty rdf:about="http://iirds.tekom.de/iirds#has-content-lifecycle-status">
        <rdfs:subPropertyOf rdf:resource="http://iirds.tekom.de/iirds#relates-to-administrative-metadata"/>
        <rdfs:domain rdf:resource="http://iirds.tekom.de/iirds#InformationUnit"/>
        <rdfs:range rdf:resource="http://iirds.tekom.de/iirds#ContentLifeCycleStatus"/>
    </owl:ObjectProperty>
    


    <!-- http://iirds.tekom.de/iirds#has-content-lifecycle-status-value -->

    <owl:ObjectProperty rdf:about="http://iirds.tekom.de/iirds#has-content-lifecycle-status-value">
        <rdfs:subPropertyOf rdf:resource="http://iirds.tekom.de/iirds#iirdsRelationConcept"/>
        <rdfs:domain rdf:resource="http://iirds.tekom.de/iirds#ContentLifeCycleStatus"/>
        <rdfs:range rdf:resource="http://iirds.tekom.de/iirds#ContentLifeCycleStatusValue"/>
    </owl:ObjectProperty>
    


    <!-- http://iirds.tekom.de/iirds#has-directory-structure-type -->

    <owl:ObjectProperty rdf:about="http://iirds.tekom.de/iirds#has-directory-structure-type">
        <rdfs:subPropertyOf rdf:resource="http://iirds.tekom.de/iirds#iirdsRelationConcept"/>
        <rdfs:domain rdf:resource="http://iirds.tekom.de/iirds#DirectoryNode"/>
        <rdfs:range rdf:resource="http://iirds.tekom.de/iirds#DirectoryNodeType"/>
    </owl:ObjectProperty>
    


    <!-- http://iirds.tekom.de/iirds#has-document-type -->

    <owl:ObjectProperty rdf:about="http://iirds.tekom.de/iirds#has-document-type">
        <rdfs:subPropertyOf rdf:resource="http://iirds.tekom.de/iirds#has-information-type"/>
        <rdfs:domain rdf:resource="http://iirds.tekom.de/iirds#Document"/>
        <rdfs:range rdf:resource="http://iirds.tekom.de/iirds#DocumentType"/>
    </owl:ObjectProperty>
    


    <!-- http://iirds.tekom.de/iirds#has-end-selector -->

    <owl:ObjectProperty rdf:about="http://iirds.tekom.de/iirds#has-end-selector">
        <rdfs:subPropertyOf rdf:resource="http://iirds.tekom.de/iirds#has-selector"/>
        <rdfs:domain rdf:resource="http://iirds.tekom.de/iirds#RangeSelector"/>
        <rdfs:range rdf:resource="http://iirds.tekom.de/iirds#FragmentSelector"/>
    </owl:ObjectProperty>
    


    <!-- http://iirds.tekom.de/iirds#has-event-code -->

    <owl:ObjectProperty rdf:about="http://iirds.tekom.de/iirds#has-event-code">
        <rdfs:subPropertyOf rdf:resource="http://iirds.tekom.de/iirds#iirdsRelationConcept"/>
        <rdfs:domain rdf:resource="http://iirds.tekom.de/iirds#Event"/>
    </owl:ObjectProperty>
    


    <!-- http://iirds.tekom.de/iirds#has-event-type -->

    <owl:ObjectProperty rdf:about="http://iirds.tekom.de/iirds#has-event-type">
        <rdfs:subPropertyOf rdf:resource="http://iirds.tekom.de/iirds#iirdsRelationConcept"/>
        <rdfs:domain rdf:resource="http://iirds.tekom.de/iirds#Event"/>
    </owl:ObjectProperty>
    


    <!-- http://iirds.tekom.de/iirds#has-first-child -->

    <owl:ObjectProperty rdf:about="http://iirds.tekom.de/iirds#has-first-child">
        <rdfs:subPropertyOf rdf:resource="http://iirds.tekom.de/iirds#iirdsRelationConcept"/>
        <rdfs:domain rdf:resource="http://iirds.tekom.de/iirds#DirectoryNode"/>
        <rdfs:range rdf:resource="http://iirds.tekom.de/iirds#DirectoryNode"/>
    </owl:ObjectProperty>
    


    <!-- http://iirds.tekom.de/iirds#has-identity -->

    <owl:ObjectProperty rdf:about="http://iirds.tekom.de/iirds#has-identity">
        <rdfs:subPropertyOf rdf:resource="http://iirds.tekom.de/iirds#relates-to-administrative-metadata"/>
        <rdfs:range rdf:resource="http://iirds.tekom.de/iirds#Identity"/>
    </owl:ObjectProperty>
    


    <!-- http://iirds.tekom.de/iirds#has-identity-domain -->

    <owl:ObjectProperty rdf:about="http://iirds.tekom.de/iirds#has-identity-domain">
        <rdfs:subPropertyOf rdf:resource="http://iirds.tekom.de/iirds#iirdsRelationConcept"/>
        <rdfs:domain rdf:resource="http://iirds.tekom.de/iirds#Identity"/>
        <rdfs:range rdf:resource="http://iirds.tekom.de/iirds#IdentityDomain"/>
    </owl:ObjectProperty>
    


    <!-- http://iirds.tekom.de/iirds#has-information-type -->

    <owl:ObjectProperty rdf:about="http://iirds.tekom.de/iirds#has-information-type">
        <rdfs:subPropertyOf rdf:resource="http://iirds.tekom.de/iirds#iirdsRelationConcept"/>
        <rdfs:domain rdf:resource="http://iirds.tekom.de/iirds#InformationUnit"/>
        <rdfs:range rdf:resource="http://iirds.tekom.de/iirds#InformationType"/>
    </owl:ObjectProperty>
    


    <!-- http://iirds.tekom.de/iirds#has-next-sibling -->

    <owl:ObjectProperty rdf:about="http://iirds.tekom.de/iirds#has-next-sibling">
        <rdfs:subPropertyOf rdf:resource="http://iirds.tekom.de/iirds#iirdsRelationConcept"/>
        <rdfs:domain rdf:resource="http://iirds.tekom.de/iirds#DirectoryNode"/>
        <rdfs:range rdf:resource="http://iirds.tekom.de/iirds#DirectoryNode"/>
    </owl:ObjectProperty>
    


    <!-- http://iirds.tekom.de/iirds#has-party-role -->

    <owl:ObjectProperty rdf:about="http://iirds.tekom.de/iirds#has-party-role">
        <rdfs:subPropertyOf rdf:resource="http://iirds.tekom.de/iirds#iirdsRelationConcept"/>
        <rdfs:domain rdf:resource="http://iirds.tekom.de/iirds#Party"/>
        <rdfs:range rdf:resource="http://iirds.tekom.de/iirds#PartyRole"/>
    </owl:ObjectProperty>
    


    <!-- http://iirds.tekom.de/iirds#has-planning-time -->

    <owl:ObjectProperty rdf:about="http://iirds.tekom.de/iirds#has-planning-time">
        <rdfs:subPropertyOf rdf:resource="http://iirds.tekom.de/iirds#relates-to-functional-metadata"/>
        <rdfs:domain rdf:resource="http://iirds.tekom.de/iirds#InformationUnit"/>
        <rdfs:range rdf:resource="http://iirds.tekom.de/iirds#PlanningTime"/>
    </owl:ObjectProperty>
    


    <!-- http://iirds.tekom.de/iirds#has-rendition -->

    <owl:ObjectProperty rdf:about="http://iirds.tekom.de/iirds#has-rendition">
        <rdfs:subPropertyOf rdf:resource="http://iirds.tekom.de/iirds#iirdsRelationConcept"/>
        <rdfs:domain rdf:resource="http://iirds.tekom.de/iirds#InformationUnit"/>
        <rdfs:range rdf:resource="http://iirds.tekom.de/iirds#Rendition"/>
    </owl:ObjectProperty>
    


    <!-- http://iirds.tekom.de/iirds#has-selector -->

    <owl:ObjectProperty rdf:about="http://iirds.tekom.de/iirds#has-selector">
        <rdfs:subPropertyOf rdf:resource="http://iirds.tekom.de/iirds#iirdsRelationConcept"/>
        <rdfs:domain rdf:resource="http://iirds.tekom.de/iirds#Rendition"/>
        <rdfs:range rdf:resource="http://iirds.tekom.de/iirds#Selector"/>
    </owl:ObjectProperty>
    


    <!-- http://iirds.tekom.de/iirds#has-start-selector -->

    <owl:ObjectProperty rdf:about="http://iirds.tekom.de/iirds#has-start-selector">
        <rdfs:subPropertyOf rdf:resource="http://iirds.tekom.de/iirds#has-selector"/>
        <rdfs:domain rdf:resource="http://iirds.tekom.de/iirds#RangeSelector"/>
        <rdfs:range rdf:resource="http://iirds.tekom.de/iirds#FragmentSelector"/>
    </owl:ObjectProperty>
    


    <!-- http://iirds.tekom.de/iirds#has-subject -->

    <owl:ObjectProperty rdf:about="http://iirds.tekom.de/iirds#has-subject">
        <rdfs:subPropertyOf rdf:resource="http://iirds.tekom.de/iirds#has-information-type"/>
        <rdfs:domain rdf:resource="http://iirds.tekom.de/iirds#InformationUnit"/>
    </owl:ObjectProperty>
    


    <!-- http://iirds.tekom.de/iirds#has-topic-type -->

    <owl:ObjectProperty rdf:about="http://iirds.tekom.de/iirds#has-topic-type">
        <rdfs:subPropertyOf rdf:resource="http://iirds.tekom.de/iirds#has-information-type"/>
        <rdfs:domain rdf:resource="http://iirds.tekom.de/iirds#InformationUnit"/>
        <rdfs:range rdf:resource="http://iirds.tekom.de/iirds#TopicType"/>
    </owl:ObjectProperty>
    


    <!-- http://iirds.tekom.de/iirds#iirdsRelationConcept -->

    <owl:ObjectProperty rdf:about="http://iirds.tekom.de/iirds#iirdsRelationConcept">
        <rdfs:domain rdf:resource="http://iirds.tekom.de/iirds#iirdsDomainEntity"/>
        <rdfs:range rdf:resource="http://iirds.tekom.de/iirds#iirdsDomainEntity"/>
    </owl:ObjectProperty>
    


    <!-- http://iirds.tekom.de/iirds#is-applicable-for-document-type -->

    <owl:ObjectProperty rdf:about="http://iirds.tekom.de/iirds#is-applicable-for-document-type">
        <rdfs:subPropertyOf rdf:resource="http://iirds.tekom.de/iirds#has-information-type"/>
        <rdfs:domain rdf:resource="http://iirds.tekom.de/iirds#InformationUnit"/>
        <rdfs:range rdf:resource="http://iirds.tekom.de/iirds#DocumentType"/>
    </owl:ObjectProperty>
    


    <!-- http://iirds.tekom.de/iirds#is-part-of-package -->

    <owl:ObjectProperty rdf:about="http://iirds.tekom.de/iirds#is-part-of-package">
        <rdfs:subPropertyOf rdf:resource="http://iirds.tekom.de/iirds#iirdsRelationConcept"/>
        <rdfs:domain rdf:resource="http://iirds.tekom.de/iirds#InformationUnit"/>
        <rdfs:range rdf:resource="http://iirds.tekom.de/iirds#Package"/>
    </owl:ObjectProperty>
    


    <!-- http://iirds.tekom.de/iirds#is-replacement-of -->

    <owl:ObjectProperty rdf:about="http://iirds.tekom.de/iirds#is-replacement-of">
        <rdfs:subPropertyOf rdf:resource="http://iirds.tekom.de/iirds#iirdsRelationConcept"/>
        <rdfs:domain rdf:resource="http://iirds.tekom.de/iirds#InformationUnit"/>
    </owl:ObjectProperty>
    


    <!-- http://iirds.tekom.de/iirds#is-version-of -->

    <owl:ObjectProperty rdf:about="http://iirds.tekom.de/iirds#is-version-of">
        <rdfs:subPropertyOf rdf:resource="http://iirds.tekom.de/iirds#iirdsRelationConcept"/>
        <rdfs:domain rdf:resource="http://iirds.tekom.de/iirds#InformationUnit"/>
    </owl:ObjectProperty>
    


    <!-- http://iirds.tekom.de/iirds#relates-to-administrative-metadata -->

    <owl:ObjectProperty rdf:about="http://iirds.tekom.de/iirds#relates-to-administrative-metadata">
        <rdfs:subPropertyOf rdf:resource="http://iirds.tekom.de/iirds#iirdsRelationConcept"/>
        <rdfs:domain rdf:resource="http://iirds.tekom.de/iirds#iirdsDomainEntity"/>
        <rdfs:range rdf:resource="http://iirds.tekom.de/iirds#AdministrativeMetadata"/>
    </owl:ObjectProperty>
    


    <!-- http://iirds.tekom.de/iirds#relates-to-component -->

    <owl:ObjectProperty rdf:about="http://iirds.tekom.de/iirds#relates-to-component">
        <rdfs:subPropertyOf rdf:resource="http://iirds.tekom.de/iirds#relates-to-product-metadata"/>
        <rdfs:domain rdf:resource="http://iirds.tekom.de/iirds#InformationUnit"/>
        <rdfs:range rdf:resource="http://iirds.tekom.de/iirds#Component"/>
    </owl:ObjectProperty>
    


    <!-- http://iirds.tekom.de/iirds#relates-to-event -->

    <owl:ObjectProperty rdf:about="http://iirds.tekom.de/iirds#relates-to-event">
        <rdfs:subPropertyOf rdf:resource="http://iirds.tekom.de/iirds#relates-to-functional-metadata"/>
        <rdfs:domain rdf:resource="http://iirds.tekom.de/iirds#InformationUnit"/>
        <rdfs:range rdf:resource="http://iirds.tekom.de/iirds#Event"/>
    </owl:ObjectProperty>
    


    <!-- http://iirds.tekom.de/iirds#relates-to-functional-metadata -->

    <owl:ObjectProperty rdf:about="http://iirds.tekom.de/iirds#relates-to-functional-metadata">
        <rdfs:subPropertyOf rdf:resource="http://iirds.tekom.de/iirds#iirdsRelationConcept"/>
        <rdfs:domain rdf:resource="http://iirds.tekom.de/iirds#InformationUnit"/>
        <rdfs:range rdf:resource="http://iirds.tekom.de/iirds#FunctionalMetadata"/>
    </owl:ObjectProperty>
    


    <!-- http://iirds.tekom.de/iirds#relates-to-information-unit -->

    <owl:ObjectProperty rdf:about="http://iirds.tekom.de/iirds#relates-to-information-unit">
        <rdfs:subPropertyOf rdf:resource="http://iirds.tekom.de/iirds#iirdsRelationConcept"/>
        <rdfs:domain rdf:resource="http://iirds.tekom.de/iirds#DirectoryNode"/>
        <rdfs:range rdf:resource="http://iirds.tekom.de/iirds#InformationUnit"/>
    </owl:ObjectProperty>
    


    <!-- http://iirds.tekom.de/iirds#relates-to-party -->

    <owl:ObjectProperty rdf:about="http://iirds.tekom.de/iirds#relates-to-party">
        <rdfs:subPropertyOf rdf:resource="http://iirds.tekom.de/iirds#relates-to-administrative-metadata"/>
        <rdfs:range rdf:resource="http://iirds.tekom.de/iirds#Party"/>
    </owl:ObjectProperty>
    


    <!-- http://iirds.tekom.de/iirds#relates-to-product-feature -->

    <owl:ObjectProperty rdf:about="http://iirds.tekom.de/iirds#relates-to-product-feature">
        <rdfs:subPropertyOf rdf:resource="http://iirds.tekom.de/iirds#relates-to-product-metadata"/>
        <rdfs:domain rdf:resource="http://iirds.tekom.de/iirds#InformationUnit"/>
        <rdfs:range rdf:resource="http://iirds.tekom.de/iirds#ProductFeature"/>
    </owl:ObjectProperty>
    


    <!-- http://iirds.tekom.de/iirds#relates-to-product-lifecycle-phase -->

    <owl:ObjectProperty rdf:about="http://iirds.tekom.de/iirds#relates-to-product-lifecycle-phase">
        <rdfs:subPropertyOf rdf:resource="http://iirds.tekom.de/iirds#relates-to-product-metadata"/>
        <rdfs:domain rdf:resource="http://iirds.tekom.de/iirds#InformationUnit"/>
        <rdfs:range rdf:resource="http://iirds.tekom.de/iirds#ProductLifeCyclePhase"/>
    </owl:ObjectProperty>
    


    <!-- http://iirds.tekom.de/iirds#relates-to-product-metadata -->

    <owl:ObjectProperty rdf:about="http://iirds.tekom.de/iirds#relates-to-product-metadata">
        <rdfs:subPropertyOf rdf:resource="http://iirds.tekom.de/iirds#iirdsRelationConcept"/>
        <rdfs:domain rdf:resource="http://iirds.tekom.de/iirds#InformationUnit"/>
        <rdfs:range rdf:resource="http://iirds.tekom.de/iirds#ProductMetadata"/>
    </owl:ObjectProperty>
    


    <!-- http://iirds.tekom.de/iirds#relates-to-product-variant -->

    <owl:ObjectProperty rdf:about="http://iirds.tekom.de/iirds#relates-to-product-variant">
        <rdfs:subPropertyOf rdf:resource="http://iirds.tekom.de/iirds#relates-to-product-metadata"/>
        <rdfs:domain rdf:resource="http://iirds.tekom.de/iirds#InformationUnit"/>
        <rdfs:range rdf:resource="http://iirds.tekom.de/iirds#ProductVariant"/>
    </owl:ObjectProperty>
    


    <!-- http://iirds.tekom.de/iirds#relates-to-qualification -->

    <owl:ObjectProperty rdf:about="http://iirds.tekom.de/iirds#relates-to-qualification">
        <rdfs:subPropertyOf rdf:resource="http://iirds.tekom.de/iirds#relates-to-functional-metadata"/>
        <rdfs:domain rdf:resource="http://iirds.tekom.de/iirds#InformationUnit"/>
        <rdfs:range rdf:resource="http://iirds.tekom.de/iirds#Qualification"/>
    </owl:ObjectProperty>
    


    <!-- http://iirds.tekom.de/iirds#relates-to-supply -->

    <owl:ObjectProperty rdf:about="http://iirds.tekom.de/iirds#relates-to-supply">
        <rdfs:subPropertyOf rdf:resource="http://iirds.tekom.de/iirds#relates-to-functional-metadata"/>
        <rdfs:domain rdf:resource="http://iirds.tekom.de/iirds#InformationUnit"/>
        <rdfs:range rdf:resource="http://iirds.tekom.de/iirds#Supply"/>
    </owl:ObjectProperty>
    


    <!-- http://iirds.tekom.de/iirds#relates-to-vcard -->

    <owl:ObjectProperty rdf:about="http://iirds.tekom.de/iirds#relates-to-vcard">
        <rdfs:subPropertyOf rdf:resource="http://iirds.tekom.de/iirds#iirdsRelationConcept"/>
        <rdfs:domain rdf:resource="http://iirds.tekom.de/iirds#Party"/>
        <rdfs:range rdf:resource="http://www.w3.org/2006/vcard/ns#Kind"/>
    </owl:ObjectProperty>
    


    <!-- http://www.w3.org/2003/01/geo/wgs84_pos#location -->

    <owl:ObjectProperty rdf:about="http://www.w3.org/2003/01/geo/wgs84_pos#location"/>
    


    <!-- 
    ///////////////////////////////////////////////////////////////////////////////////////
    //
    // Data properties
    //
    ///////////////////////////////////////////////////////////////////////////////////////
     -->

    


    <!-- http://iirds.tekom.de/iirds#dateOfCreation -->

    <owl:DatatypeProperty rdf:about="http://iirds.tekom.de/iirds#dateOfCreation">
        <rdfs:subPropertyOf rdf:resource="http://iirds.tekom.de/iirds#iirdsAttribute"/>
    </owl:DatatypeProperty>
    


    <!-- http://iirds.tekom.de/iirds#dateOfEffect -->

    <owl:DatatypeProperty rdf:about="http://iirds.tekom.de/iirds#dateOfEffect">
        <rdfs:subPropertyOf rdf:resource="http://iirds.tekom.de/iirds#iirdsAttribute"/>
        <rdfs:domain rdf:resource="http://iirds.tekom.de/iirds#ContentLifeCycleStatus"/>
        <rdfs:range rdf:resource="http://www.w3.org/2001/XMLSchema#dateTimeStamp"/>
    </owl:DatatypeProperty>
    


    <!-- http://iirds.tekom.de/iirds#dateOfExpiry -->

    <owl:DatatypeProperty rdf:about="http://iirds.tekom.de/iirds#dateOfExpiry">
        <rdfs:subPropertyOf rdf:resource="http://iirds.tekom.de/iirds#iirdsAttribute"/>
        <rdfs:domain rdf:resource="http://iirds.tekom.de/iirds#ContentLifeCycleStatus"/>
        <rdfs:range rdf:resource="http://www.w3.org/2001/XMLSchema#dateTimeStamp"/>
    </owl:DatatypeProperty>
    


    <!-- http://iirds.tekom.de/iirds#dateOfLastModification -->

    <owl:DatatypeProperty rdf:about="http://iirds.tekom.de/iirds#dateOfLastModification">
        <rdfs:subPropertyOf rdf:resource="http://iirds.tekom.de/iirds#iirdsAttribute"/>
        <rdfs:range rdf:resource="http://www.w3.org/2001/XMLSchema#dateTimeStamp"/>
    </owl:DatatypeProperty>
    


    <!-- http://iirds.tekom.de/iirds#dateOfStatus -->

    <owl:DatatypeProperty rdf:about="http://iirds.tekom.de/iirds#dateOfStatus">
        <rdfs:subPropertyOf rdf:resource="http://iirds.tekom.de/iirds#iirdsAttribute"/>
        <rdfs:domain rdf:resource="http://iirds.tekom.de/iirds#ContentLifeCycleStatus"/>
        <rdfs:range rdf:resource="http://www.w3.org/2001/XMLSchema#dateTimeStamp"/>
    </owl:DatatypeProperty>
    


    <!-- http://iirds.tekom.de/iirds#description -->

    <owl:DatatypeProperty rdf:about="http://iirds.tekom.de/iirds#description">
        <rdfs:subPropertyOf rdf:resource="http://iirds.tekom.de/iirds#iirdsAttribute"/>
    </owl:DatatypeProperty>
    


    <!-- http://iirds.tekom.de/iirds#duration -->

    <owl:DatatypeProperty rdf:about="http://iirds.tekom.de/iirds#duration">
        <rdfs:subPropertyOf rdf:resource="http://iirds.tekom.de/iirds#iirdsAttribute"/>
        <rdfs:domain rdf:resource="http://iirds.tekom.de/iirds#PlanningTime"/>
        <rdfs:range rdf:resource="http://www.w3.org/2001/XMLSchema#duration"/>
    </owl:DatatypeProperty>
    


    <!-- http://iirds.tekom.de/iirds#format -->

    <owl:DatatypeProperty rdf:about="http://iirds.tekom.de/iirds#format">
        <rdfs:subPropertyOf rdf:resource="http://iirds.tekom.de/iirds#iirdsAttribute"/>
    </owl:DatatypeProperty>
    


    <!-- http://iirds.tekom.de/iirds#formatRestriction -->

    <owl:DatatypeProperty rdf:about="http://iirds.tekom.de/iirds#formatRestriction">
        <rdfs:subPropertyOf rdf:resource="http://iirds.tekom.de/iirds#iirdsAttribute"/>
        <rdfs:domain rdf:resource="http://iirds.tekom.de/iirds#Package"/>
        <rdfs:range rdf:resource="http://www.w3.org/2000/01/rdf-schema#Literal"/>
    </owl:DatatypeProperty>
    


    <!-- http://iirds.tekom.de/iirds#frequency -->

    <owl:DatatypeProperty rdf:about="http://iirds.tekom.de/iirds#frequency">
        <rdfs:subPropertyOf rdf:resource="http://iirds.tekom.de/iirds#iirdsAttribute"/>
        <rdfs:domain rdf:resource="http://iirds.tekom.de/iirds#MaintenanceInterval"/>
        <rdfs:range rdf:resource="http://www.w3.org/2000/01/rdf-schema#Literal"/>
    </owl:DatatypeProperty>
    


    <!-- http://iirds.tekom.de/iirds#identifier -->

    <owl:DatatypeProperty rdf:about="http://iirds.tekom.de/iirds#identifier">
        <rdfs:subPropertyOf rdf:resource="http://iirds.tekom.de/iirds#iirdsAttribute"/>
    </owl:DatatypeProperty>
    


    <!-- http://iirds.tekom.de/iirds#iiRDSVersion -->

    <owl:DatatypeProperty rdf:about="http://iirds.tekom.de/iirds#iiRDSVersion">
        <rdfs:subPropertyOf rdf:resource="http://iirds.tekom.de/iirds#iirdsAttribute"/>
        <rdfs:domain rdf:resource="http://iirds.tekom.de/iirds#Package"/>
        <rdfs:range rdf:resource="http://www.w3.org/2000/01/rdf-schema#Literal"/>
    </owl:DatatypeProperty>
    


    <!-- http://iirds.tekom.de/iirds#iirdsAttribute -->

    <owl:DatatypeProperty rdf:about="http://iirds.tekom.de/iirds#iirdsAttribute">
        <rdfs:range rdf:resource="http://www.w3.org/2000/01/rdf-schema#Literal"/>
    </owl:DatatypeProperty>
    


    <!-- http://iirds.tekom.de/iirds#language -->

    <owl:DatatypeProperty rdf:about="http://iirds.tekom.de/iirds#language">
        <rdfs:subPropertyOf rdf:resource="http://iirds.tekom.de/iirds#iirdsAttribute"/>
    </owl:DatatypeProperty>
    


    <!-- http://iirds.tekom.de/iirds#purpose -->

    <owl:DatatypeProperty rdf:about="http://iirds.tekom.de/iirds#purpose">
        <rdfs:subPropertyOf rdf:resource="http://iirds.tekom.de/iirds#iirdsAttribute"/>
        <rdfs:domain rdf:resource="http://iirds.tekom.de/iirds#ContentLifeCycleStatus"/>
        <rdfs:range rdf:resource="http://www.w3.org/2000/01/rdf-schema#Literal"/>
    </owl:DatatypeProperty>
    


    <!-- http://iirds.tekom.de/iirds#revision -->

    <owl:DatatypeProperty rdf:about="http://iirds.tekom.de/iirds#revision">
        <rdfs:subPropertyOf rdf:resource="http://iirds.tekom.de/iirds#iirdsAttribute"/>
    </owl:DatatypeProperty>
    


    <!-- http://iirds.tekom.de/iirds#rights -->

    <owl:DatatypeProperty rdf:about="http://iirds.tekom.de/iirds#rights">
        <rdfs:subPropertyOf rdf:resource="http://iirds.tekom.de/iirds#iirdsAttribute"/>
    </owl:DatatypeProperty>
    


    <!-- http://iirds.tekom.de/iirds#source -->

    <owl:DatatypeProperty rdf:about="http://iirds.tekom.de/iirds#source">
        <rdfs:subPropertyOf rdf:resource="http://iirds.tekom.de/iirds#iirdsAttribute"/>
        <rdfs:domain rdf:resource="http://iirds.tekom.de/iirds#Rendition"/>
        <rdfs:range rdf:resource="http://www.w3.org/2000/01/rdf-schema#Literal"/>
    </owl:DatatypeProperty>
    


    <!-- http://iirds.tekom.de/iirds#statusComment -->

    <owl:DatatypeProperty rdf:about="http://iirds.tekom.de/iirds#statusComment">
        <rdfs:subPropertyOf rdf:resource="http://iirds.tekom.de/iirds#iirdsAttribute"/>
        <rdfs:domain rdf:resource="http://iirds.tekom.de/iirds#ContentLifeCycleStatus"/>
        <rdfs:range rdf:resource="http://www.w3.org/2000/01/rdf-schema#Literal"/>
    </owl:DatatypeProperty>
    


    <!-- http://iirds.tekom.de/iirds#synonym -->

    <owl:DatatypeProperty rdf:about="http://iirds.tekom.de/iirds#synonym">
        <rdfs:subPropertyOf rdf:resource="http://iirds.tekom.de/iirds#iirdsAttribute"/>
        <rdfs:domain rdf:resource="http://iirds.tekom.de/iirds#iirdsDomainEntity"/>
        <rdfs:range rdf:resource="http://www.w3.org/2000/01/rdf-schema#Literal"/>
    </owl:DatatypeProperty>
    


    <!-- http://iirds.tekom.de/iirds#title -->

    <owl:DatatypeProperty rdf:about="http://iirds.tekom.de/iirds#title">
        <rdfs:subPropertyOf rdf:resource="http://iirds.tekom.de/iirds#iirdsAttribute"/>
    </owl:DatatypeProperty>
    


    <!-- 
    ///////////////////////////////////////////////////////////////////////////////////////
    //
    // Classes
    //
    ///////////////////////////////////////////////////////////////////////////////////////
     -->

    


    <!-- http://iirds.tekom.de/iirds#AdministrativeMetadata -->

    <owl:Class rdf:about="http://iirds.tekom.de/iirds#AdministrativeMetadata">
        <rdfs:subClassOf rdf:resource="http://iirds.tekom.de/iirds#iirdsDomainEntity"/>
    </owl:Class>
    


    <!-- http://iirds.tekom.de/iirds#AfterUse -->

    <owl:Class rdf:about="http://iirds.tekom.de/iirds#AfterUse">
        <rdfs:subClassOf rdf:resource="http://iirds.tekom.de/iirds#ProductLifeCyclePhase"/>
    </owl:Class>
    


    <!-- http://iirds.tekom.de/iirds#Collection -->

    <owl:Class rdf:about="http://iirds.tekom.de/iirds#Collection">
        <rdfs:subClassOf rdf:resource="http://iirds.tekom.de/iirds#InformationSubject"/>
    </owl:Class>
    


    <!-- http://iirds.tekom.de/iirds#Component -->

    <owl:Class rdf:about="http://iirds.tekom.de/iirds#Component">
        <rdfs:subClassOf rdf:resource="http://iirds.tekom.de/iirds#ProductMetadata"/>
    </owl:Class>
    


    <!-- http://iirds.tekom.de/iirds#Concept -->

    <owl:Class rdf:about="http://iirds.tekom.de/iirds#Concept">
        <rdfs:subClassOf rdf:resource="http://iirds.tekom.de/iirds#TopicType"/>
    </owl:Class>
    


    <!-- http://iirds.tekom.de/iirds#Conformity -->

    <owl:Class rdf:about="http://iirds.tekom.de/iirds#Conformity">
        <rdfs:subClassOf rdf:resource="http://iirds.tekom.de/iirds#InformationSubject"/>
    </owl:Class>
    


    <!-- http://iirds.tekom.de/iirds#ContentLifeCycleStatus -->

    <owl:Class rdf:about="http://iirds.tekom.de/iirds#ContentLifeCycleStatus">
        <rdfs:subClassOf rdf:resource="http://iirds.tekom.de/iirds#AdministrativeMetadata"/>
    </owl:Class>
    


    <!-- http://iirds.tekom.de/iirds#ContentLifeCycleStatusValue -->

    <owl:Class rdf:about="http://iirds.tekom.de/iirds#ContentLifeCycleStatusValue">
        <rdfs:subClassOf rdf:resource="http://iirds.tekom.de/iirds#AdministrativeMetadata"/>
    </owl:Class>
    


    <!-- http://iirds.tekom.de/iirds#DesignAndRealization -->

    <owl:Class rdf:about="http://iirds.tekom.de/iirds#DesignAndRealization">
        <rdfs:subClassOf rdf:resource="http://iirds.tekom.de/iirds#ProductLifeCyclePhase"/>
    </owl:Class>
    


    <!-- http://iirds.tekom.de/iirds#DirectoryNode -->

    <owl:Class rdf:about="http://iirds.tekom.de/iirds#DirectoryNode">
        <rdfs:subClassOf rdf:resource="http://iirds.tekom.de/iirds#iirdsDomainEntity"/>
    </owl:Class>
    


    <!-- http://iirds.tekom.de/iirds#DirectoryNodeType -->

    <owl:Class rdf:about="http://iirds.tekom.de/iirds#DirectoryNodeType">
        <rdfs:subClassOf rdf:resource="http://iirds.tekom.de/iirds#InformationType"/>
    </owl:Class>
    


    <!-- http://iirds.tekom.de/iirds#Document -->

    <owl:Class rdf:about="http://iirds.tekom.de/iirds#Document">
        <rdfs:subClassOf rdf:resource="http://iirds.tekom.de/iirds#InformationUnit"/>
    </owl:Class>
    


    <!-- http://iirds.tekom.de/iirds#DocumentType -->

    <owl:Class rdf:about="http://iirds.tekom.de/iirds#DocumentType">
        <rdfs:subClassOf rdf:resource="http://iirds.tekom.de/iirds#InformationType"/>
    </owl:Class>
    


    <!-- http://iirds.tekom.de/iirds#DocumentationMetadata -->

    <owl:Class rdf:about="http://iirds.tekom.de/iirds#DocumentationMetadata">
        <rdfs:subClassOf rdf:resource="http://iirds.tekom.de/iirds#iirdsDomainEntity"/>
    </owl:Class>
    


    <!-- http://iirds.tekom.de/iirds#DownTime -->

    <owl:Class rdf:about="http://iirds.tekom.de/iirds#DownTime">
        <rdfs:subClassOf rdf:resource="http://iirds.tekom.de/iirds#PlanningTime"/>
    </owl:Class>
    


    <!-- http://iirds.tekom.de/iirds#Event -->

    <owl:Class rdf:about="http://iirds.tekom.de/iirds#Event">
        <rdfs:subClassOf rdf:resource="http://iirds.tekom.de/iirds#FunctionalMetadata"/>
    </owl:Class>
    


    <!-- http://iirds.tekom.de/iirds#Form -->

    <owl:Class rdf:about="http://iirds.tekom.de/iirds#Form">
        <rdfs:subClassOf rdf:resource="http://iirds.tekom.de/iirds#TopicType"/>
    </owl:Class>
    


    <!-- http://iirds.tekom.de/iirds#Formality -->

    <owl:Class rdf:about="http://iirds.tekom.de/iirds#Formality">
        <rdfs:subClassOf rdf:resource="http://iirds.tekom.de/iirds#InformationSubject"/>
    </owl:Class>
    


    <!-- http://iirds.tekom.de/iirds#Fragment -->

    <owl:Class rdf:about="http://iirds.tekom.de/iirds#Fragment">
        <rdfs:subClassOf rdf:resource="http://iirds.tekom.de/iirds#InformationUnit"/>
    </owl:Class>
    


    <!-- http://iirds.tekom.de/iirds#FragmentSelector -->

    <owl:Class rdf:about="http://iirds.tekom.de/iirds#FragmentSelector">
        <rdfs:subClassOf rdf:resource="http://iirds.tekom.de/iirds#Selector"/>
    </owl:Class>
    


    <!-- http://iirds.tekom.de/iirds#FunctionalMetadata -->

    <owl:Class rdf:about="http://iirds.tekom.de/iirds#FunctionalMetadata">
        <rdfs:subClassOf rdf:resource="http://iirds.tekom.de/iirds#DocumentationMetadata"/>
    </owl:Class>
    


    <!-- http://iirds.tekom.de/iirds#Functionality -->

    <owl:Class rdf:about="http://iirds.tekom.de/iirds#Functionality">
        <rdfs:subClassOf rdf:resource="http://iirds.tekom.de/iirds#InformationSubject"/>
    </owl:Class>
    


    <!-- http://iirds.tekom.de/iirds#Identity -->

    <owl:Class rdf:about="http://iirds.tekom.de/iirds#Identity">
        <rdfs:subClassOf rdf:resource="http://iirds.tekom.de/iirds#AdministrativeMetadata"/>
    </owl:Class>
    


    <!-- http://iirds.tekom.de/iirds#IdentityDomain -->

    <owl:Class rdf:about="http://iirds.tekom.de/iirds#IdentityDomain">
        <rdfs:subClassOf rdf:resource="http://iirds.tekom.de/iirds#AdministrativeMetadata"/>
    </owl:Class>
    


    <!-- http://iirds.tekom.de/iirds#InformationObject -->

    <owl:Class rdf:about="http://iirds.tekom.de/iirds#InformationObject">
        <rdfs:subClassOf rdf:resource="http://iirds.tekom.de/iirds#iirdsDomainEntity"/>
    </owl:Class>
    


    <!-- http://iirds.tekom.de/iirds#InformationSubject -->

    <owl:Class rdf:about="http://iirds.tekom.de/iirds#InformationSubject">
        <rdfs:subClassOf rdf:resource="http://iirds.tekom.de/iirds#InformationType"/>
    </owl:Class>
    


    <!-- http://iirds.tekom.de/iirds#InformationType -->

    <owl:Class rdf:about="http://iirds.tekom.de/iirds#InformationType">
        <rdfs:subClassOf rdf:resource="http://iirds.tekom.de/iirds#iirdsDomainEntity"/>
    </owl:Class>
    


    <!-- http://iirds.tekom.de/iirds#InformationUnit -->

    <owl:Class rdf:about="http://iirds.tekom.de/iirds#InformationUnit">
        <rdfs:subClassOf rdf:resource="http://iirds.tekom.de/iirds#iirdsDomainEntity"/>
    </owl:Class>
    


    <!-- http://iirds.tekom.de/iirds#Learning -->

    <owl:Class rdf:about="http://iirds.tekom.de/iirds#Learning">
        <rdfs:subClassOf rdf:resource="http://iirds.tekom.de/iirds#TopicType"/>
    </owl:Class>
    


    <!-- http://iirds.tekom.de/iirds#MaintenanceInterval -->

    <owl:Class rdf:about="http://iirds.tekom.de/iirds#MaintenanceInterval">
        <rdfs:subClassOf rdf:resource="http://iirds.tekom.de/iirds#PlanningTime"/>
    </owl:Class>
    


    <!-- http://iirds.tekom.de/iirds#Package -->

    <owl:Class rdf:about="http://iirds.tekom.de/iirds#Package">
        <rdfs:subClassOf rdf:resource="http://iirds.tekom.de/iirds#InformationUnit"/>
    </owl:Class>
    


    <!-- http://iirds.tekom.de/iirds#Party -->

    <owl:Class rdf:about="http://iirds.tekom.de/iirds#Party">
        <rdfs:subClassOf rdf:resource="http://iirds.tekom.de/iirds#AdministrativeMetadata"/>
    </owl:Class>
    


    <!-- http://iirds.tekom.de/iirds#PartyRole -->

    <owl:Class rdf:about="http://iirds.tekom.de/iirds#PartyRole">
        <rdfs:subClassOf rdf:resource="http://iirds.tekom.de/iirds#AdministrativeMetadata"/>
    </owl:Class>
    


    <!-- http://iirds.tekom.de/iirds#PlanningTime -->

    <owl:Class rdf:about="http://iirds.tekom.de/iirds#PlanningTime">
        <rdfs:subClassOf rdf:resource="http://iirds.tekom.de/iirds#FunctionalMetadata"/>
    </owl:Class>
    


    <!-- http://iirds.tekom.de/iirds#Process -->

    <owl:Class rdf:about="http://iirds.tekom.de/iirds#Process">
        <rdfs:subClassOf rdf:resource="http://iirds.tekom.de/iirds#InformationSubject"/>
    </owl:Class>
    


    <!-- http://iirds.tekom.de/iirds#ProductFeature -->

    <owl:Class rdf:about="http://iirds.tekom.de/iirds#ProductFeature">
        <rdfs:subClassOf rdf:resource="http://iirds.tekom.de/iirds#ProductMetadata"/>
    </owl:Class>
    


    <!-- http://iirds.tekom.de/iirds#ProductFunction -->

    <owl:Class rdf:about="http://iirds.tekom.de/iirds#ProductFunction">
        <rdfs:subClassOf rdf:resource="http://iirds.tekom.de/iirds#ProductFeature"/>
    </owl:Class>
    


    <!-- http://iirds.tekom.de/iirds#ProductLifeCyclePhase -->

    <owl:Class rdf:about="http://iirds.tekom.de/iirds#ProductLifeCyclePhase">
        <rdfs:subClassOf rdf:resource="http://iirds.tekom.de/iirds#ProductMetadata"/>
    </owl:Class>
    


    <!-- http://iirds.tekom.de/iirds#ProductMetadata -->

    <owl:Class rdf:about="http://iirds.tekom.de/iirds#ProductMetadata">
        <rdfs:subClassOf rdf:resource="http://iirds.tekom.de/iirds#DocumentationMetadata"/>
    </owl:Class>
    


    <!-- http://iirds.tekom.de/iirds#ProductProperty -->

    <owl:Class rdf:about="http://iirds.tekom.de/iirds#ProductProperty">
        <rdfs:subClassOf rdf:resource="http://iirds.tekom.de/iirds#ProductFeature"/>
    </owl:Class>
    


    <!-- http://iirds.tekom.de/iirds#ProductVariant -->

    <owl:Class rdf:about="http://iirds.tekom.de/iirds#ProductVariant">
        <rdfs:subClassOf rdf:resource="http://iirds.tekom.de/iirds#ProductMetadata"/>
    </owl:Class>
    


    <!-- http://iirds.tekom.de/iirds#PuttingToUse -->

    <owl:Class rdf:about="http://iirds.tekom.de/iirds#PuttingToUse">
        <rdfs:subClassOf rdf:resource="http://iirds.tekom.de/iirds#ProductLifeCyclePhase"/>
    </owl:Class>
    


    <!-- http://iirds.tekom.de/iirds#Qualification -->

    <owl:Class rdf:about="http://iirds.tekom.de/iirds#Qualification">
        <rdfs:subClassOf rdf:resource="http://iirds.tekom.de/iirds#FunctionalMetadata"/>
    </owl:Class>
    


    <!-- http://iirds.tekom.de/iirds#RangeSelector -->

    <owl:Class rdf:about="http://iirds.tekom.de/iirds#RangeSelector">
        <rdfs:subClassOf rdf:resource="http://iirds.tekom.de/iirds#Selector"/>
    </owl:Class>
    


    <!-- http://iirds.tekom.de/iirds#Reference -->

    <owl:Class rdf:about="http://iirds.tekom.de/iirds#Reference">
        <rdfs:subClassOf rdf:resource="http://iirds.tekom.de/iirds#TopicType"/>
    </owl:Class>
    


    <!-- http://iirds.tekom.de/iirds#Rendition -->

    <owl:Class rdf:about="http://iirds.tekom.de/iirds#Rendition">
        <rdfs:subClassOf rdf:resource="http://iirds.tekom.de/iirds#iirdsDomainEntity"/>
    </owl:Class>
    


    <!-- http://iirds.tekom.de/iirds#Role -->

    <owl:Class rdf:about="http://iirds.tekom.de/iirds#Role">
        <rdfs:subClassOf rdf:resource="http://iirds.tekom.de/iirds#Qualification"/>
    </owl:Class>
    


    <!-- http://iirds.tekom.de/iirds#Safety -->

    <owl:Class rdf:about="http://iirds.tekom.de/iirds#Safety">
        <rdfs:subClassOf rdf:resource="http://iirds.tekom.de/iirds#InformationSubject"/>
    </owl:Class>
    


    <!-- http://iirds.tekom.de/iirds#Selector -->

    <owl:Class rdf:about="http://iirds.tekom.de/iirds#Selector">
        <rdfs:subClassOf rdf:resource="http://iirds.tekom.de/iirds#iirdsDomainEntity"/>
    </owl:Class>
    


    <!-- http://iirds.tekom.de/iirds#SkillLevel -->

    <owl:Class rdf:about="http://iirds.tekom.de/iirds#SkillLevel">
        <rdfs:subClassOf rdf:resource="http://iirds.tekom.de/iirds#Qualification"/>
    </owl:Class>
    


    <!-- http://iirds.tekom.de/iirds#Supply -->

    <owl:Class rdf:about="http://iirds.tekom.de/iirds#Supply">
        <rdfs:subClassOf rdf:resource="http://iirds.tekom.de/iirds#FunctionalMetadata"/>
    </owl:Class>
    


    <!-- http://iirds.tekom.de/iirds#Task -->

    <owl:Class rdf:about="http://iirds.tekom.de/iirds#Task">
        <rdfs:subClassOf rdf:resource="http://iirds.tekom.de/iirds#TopicType"/>
    </owl:Class>
    


    <!-- http://iirds.tekom.de/iirds#TechnicalData -->

    <owl:Class rdf:about="http://iirds.tekom.de/iirds#TechnicalData">
        <rdfs:subClassOf rdf:resource="http://iirds.tekom.de/iirds#InformationSubject"/>
    </owl:Class>
    


    <!-- http://iirds.tekom.de/iirds#TechnicalOverview -->

    <owl:Class rdf:about="http://iirds.tekom.de/iirds#TechnicalOverview">
        <rdfs:subClassOf rdf:resource="http://iirds.tekom.de/iirds#InformationSubject"/>
    </owl:Class>
    


    <!-- http://iirds.tekom.de/iirds#Topic -->

    <owl:Class rdf:about="http://iirds.tekom.de/iirds#Topic">
        <rdfs:subClassOf rdf:resource="http://iirds.tekom.de/iirds#InformationUnit"/>
    </owl:Class>
    


    <!-- http://iirds.tekom.de/iirds#TopicType -->

    <owl:Class rdf:about="http://iirds.tekom.de/iirds#TopicType">
        <rdfs:subClassOf rdf:resource="http://iirds.tekom.de/iirds#InformationType"/>
    </owl:Class>
    


    <!-- http://iirds.tekom.de/iirds#Troubleshooting -->

    <owl:Class rdf:about="http://iirds.tekom.de/iirds#Troubleshooting">
        <rdfs:subClassOf rdf:resource="http://iirds.tekom.de/iirds#TopicType"/>
    </owl:Class>
    


    <!-- http://iirds.tekom.de/iirds#Use -->

    <owl:Class rdf:about="http://iirds.tekom.de/iirds#Use">
        <rdfs:subClassOf rdf:resource="http://iirds.tekom.de/iirds#ProductLifeCyclePhase"/>
    </owl:Class>
    


    <!-- http://iirds.tekom.de/iirds#WarningMessage -->

    <owl:Class rdf:about="http://iirds.tekom.de/iirds#WarningMessage">
        <rdfs:subClassOf rdf:resource="http://iirds.tekom.de/iirds#Safety"/>
    </owl:Class>
    


    <!-- http://iirds.tekom.de/iirds#WorkingTime -->

    <owl:Class rdf:about="http://iirds.tekom.de/iirds#WorkingTime">
        <rdfs:subClassOf rdf:resource="http://iirds.tekom.de/iirds#PlanningTime"/>
    </owl:Class>
    


    <!-- http://iirds.tekom.de/iirds#iirdsDomainEntity -->

    <owl:Class rdf:about="http://iirds.tekom.de/iirds#iirdsDomainEntity"/>
    


    <!-- http://iirds.tekom.de/iirds#nil -->

    <owl:Class rdf:about="http://iirds.tekom.de/iirds#nil">
        <rdfs:subClassOf rdf:resource="http://iirds.tekom.de/iirds#DirectoryNode"/>
    </owl:Class>
    


    <!-- http://www.w3.org/2003/01/geo/wgs84_pos#Point -->

    <owl:Class rdf:about="http://www.w3.org/2003/01/geo/wgs84_pos#Point">
        <rdfs:subClassOf rdf:resource="http://www.w3.org/2003/01/geo/wgs84_pos#SpatialThing"/>
        <rdfs:comment> 
Uniquely identified by lat/long/alt. i.e.

spaciallyIntersects(P1, P2) :- lat(P1, LAT), long(P1, LONG), alt(P1, ALT),
  lat(P2, LAT), long(P2, LONG), alt(P2, ALT).

sameThing(P1, P2) :- type(P1, Point), type(P2, Point), spaciallyIntersects(P1, P2).
  </rdfs:comment>
        <rdfs:comment>A point, typically described using a coordinate system relative to Earth, such as WGS84.
  </rdfs:comment>
        <rdfs:label>point</rdfs:label>
    </owl:Class>
    


    <!-- http://www.w3.org/2003/01/geo/wgs84_pos#SpatialThing -->

    <owl:Class rdf:about="http://www.w3.org/2003/01/geo/wgs84_pos#SpatialThing">
        <rdfs:comment>Anything with spatial extent, i.e. size, shape, or position.
 e.g. people, places, bowling balls, as well as abstract areas like cubes.
</rdfs:comment>
        <rdfs:label>SpatialThing</rdfs:label>
    </owl:Class>
    


    <!-- http://www.w3.org/2006/time#TemporalDuration -->

    <rdf:Description rdf:about="http://www.w3.org/2006/time#TemporalDuration">
        <rdfs:subClassOf>
            <owl:Restriction>
                <owl:onProperty rdf:resource="http://www.w3.org/2006/time#unitType"/>
                <owl:qualifiedCardinality rdf:datatype="http://www.w3.org/2001/XMLSchema#nonNegativeInteger">1</owl:qualifiedCardinality>
                <owl:onClass rdf:resource="http://www.w3.org/2006/time#TemporalUnit"/>
            </owl:Restriction>
        </rdfs:subClassOf>
    </rdf:Description>
    


    <!-- http://www.w3.org/2006/vcard/ns#Address -->

    <rdf:Description rdf:about="http://www.w3.org/2006/vcard/ns#Address">
        <rdfs:subClassOf rdf:resource="http://www.w3.org/2003/01/geo/wgs84_pos#SpatialThing"/>
    </rdf:Description>
    


    <!-- http://www.w3id.org/issi/WorkOrder -->

    <owl:Class rdf:about="http://www.w3id.org/issi/WorkOrder">
        <rdfs:subClassOf>
            <owl:Restriction>
                <owl:onProperty rdf:resource="http://www.w3.org/2006/time#hasDuration"/>
                <owl:minQualifiedCardinality rdf:datatype="http://www.w3.org/2001/XMLSchema#nonNegativeInteger">1</owl:minQualifiedCardinality>
                <owl:onClass rdf:resource="http://www.w3.org/2006/time#TemporalDuration"/>
            </owl:Restriction>
        </rdfs:subClassOf>
        <rdfs:subClassOf>
            <owl:Restriction>
                <owl:onProperty rdf:resource="http://www.w3.org/2006/time#hasTime"/>
                <owl:minQualifiedCardinality rdf:datatype="http://www.w3.org/2001/XMLSchema#nonNegativeInteger">1</owl:minQualifiedCardinality>
                <owl:onClass rdf:resource="http://www.w3.org/2006/time#Instant"/>
            </owl:Restriction>
        </rdfs:subClassOf>
        <rdfs:subClassOf>
            <owl:Restriction>
                <owl:onProperty rdf:resource="http://iirds.tekom.de/iirds#identifier"/>
                <owl:cardinality rdf:datatype="http://www.w3.org/2001/XMLSchema#nonNegativeInteger">1</owl:cardinality>
            </owl:Restriction>
        </rdfs:subClassOf>
        <rdfs:label xml:lang="en">Work Order</rdfs:label>
    </owl:Class>
    


    <!-- 
    ///////////////////////////////////////////////////////////////////////////////////////
    //
    // Individuals
    //
    ///////////////////////////////////////////////////////////////////////////////////////
     -->

    


    <!-- http://iirds.tekom.de/iirds#Acquisition -->

    <owl:NamedIndividual rdf:about="http://iirds.tekom.de/iirds#Acquisition">
        <rdf:type rdf:resource="http://iirds.tekom.de/iirds#DesignAndRealization"/>
        <iirds:description xml:lang="en"></iirds:description>
        <rdfs:comment xml:lang="en">Lifecycle phase of a product during which services, goods, or works are acquired from an external source.</rdfs:comment>
        <rdfs:label xml:lang="en">Acquisition</rdfs:label>
        <rdfs:label xml:lang="de">Beschaffung</rdfs:label>
    </owl:NamedIndividual>
    


    <!-- http://iirds.tekom.de/iirds#AdministrativeMetadata -->

    <owl:NamedIndividual rdf:about="http://iirds.tekom.de/iirds#AdministrativeMetadata"/>
    


    <!-- http://iirds.tekom.de/iirds#AdministratorGuide -->

    <owl:NamedIndividual rdf:about="http://iirds.tekom.de/iirds#AdministratorGuide">
        <rdf:type rdf:resource="http://iirds.tekom.de/iirds#DocumentType"/>
        <iirds:description xml:lang="en"></iirds:description>
        <rdfs:comment xml:lang="en">Type of document. Contains instructions for the administration of a technical system.</rdfs:comment>
        <rdfs:label xml:lang="de">Administrationsanleitung</rdfs:label>
        <rdfs:label xml:lang="en">Administrator guide</rdfs:label>
    </owl:NamedIndividual>
    


    <!-- http://iirds.tekom.de/iirds#AfterUse -->

    <owl:NamedIndividual rdf:about="http://iirds.tekom.de/iirds#AfterUse"/>
    


    <!-- http://iirds.tekom.de/iirds#ApplicableStandards -->

    <owl:NamedIndividual rdf:about="http://iirds.tekom.de/iirds#ApplicableStandards">
        <rdf:type rdf:resource="http://iirds.tekom.de/iirds#Conformity"/>
        <iirds:description xml:lang="en">Examples: machinery directive, ATEX directive</iirds:description>
        <rdfs:comment xml:lang="en">Information subject related to conformity. Describes content related to standards that a product needs to fulfill.</rdfs:comment>
        <rdfs:label xml:lang="en">Applicable standard</rdfs:label>
        <rdfs:label xml:lang="de">Geltende Norm und Richtlinie</rdfs:label>
    </owl:NamedIndividual>
    


    <!-- http://iirds.tekom.de/iirds#Approved -->

    <owl:NamedIndividual rdf:about="http://iirds.tekom.de/iirds#Approved">
        <rdf:type rdf:resource="http://iirds.tekom.de/iirds#ContentLifeCycleStatusValue"/>
        <iirds:description xml:lang="en"></iirds:description>
        <rdfs:comment xml:lang="en">Content lifecycle status value; indicates that the content has been approved.</rdfs:comment>
        <rdfs:label xml:lang="en">Approved</rdfs:label>
        <rdfs:label xml:lang="de">Freigegeben</rdfs:label>
    </owl:NamedIndividual>
    


    <!-- http://iirds.tekom.de/iirds#AssemblyInstructions -->

    <owl:NamedIndividual rdf:about="http://iirds.tekom.de/iirds#AssemblyInstructions">
        <rdf:type rdf:resource="http://iirds.tekom.de/iirds#DocumentType"/>
        <iirds:description xml:lang="en"></iirds:description>
        <rdfs:comment xml:lang="de">Dokumentenart. Enthält Anleitungen, die den Anwender dazu befähigen, ein physisches Produkt so zusammenzubauen, dass es die bestimmungsgemäße Verwendung erfüllt und die Sicherheit und Gesundheit von Personen nicht beeinträchtigt wird.</rdfs:comment>
        <rdfs:comment xml:lang="en">Type of document. Contains instructions enabling the operator to assemble a physical product so that it fulfills its intended use and does not endanger the health and safety of persons.</rdfs:comment>
        <rdfs:label xml:lang="en">Assembly instructions</rdfs:label>
        <rdfs:label xml:lang="de">Montageanleitung</rdfs:label>
    </owl:NamedIndividual>
    


    <!-- http://iirds.tekom.de/iirds#Author -->

    <owl:NamedIndividual rdf:about="http://iirds.tekom.de/iirds#Author">
        <rdf:type rdf:resource="http://iirds.tekom.de/iirds#PartyRole"/>
        <iirds:description xml:lang="en">An author is the individual or the organization from which the referenced iiRDS domain entity originates.</iirds:description>
        <rdfs:comment xml:lang="en">Instance of the PartyRole class describing the role of an actor related to an iiRDS domain entity.</rdfs:comment>
        <rdfs:label xml:lang="en">Author</rdfs:label>
        <rdfs:label xml:lang="de">Autor</rdfs:label>
    </owl:NamedIndividual>
    


    <!-- http://iirds.tekom.de/iirds#BillOfMaterials -->

    <owl:NamedIndividual rdf:about="http://iirds.tekom.de/iirds#BillOfMaterials">
        <rdf:type rdf:resource="http://iirds.tekom.de/iirds#DocumentType"/>
        <iirds:description xml:lang="en">Type of document (VDI 2770). Examples are part list with part number, part description, order number, and references to other documents.</iirds:description>
        <rdfs:comment xml:lang="en">List of sub-components, sub-modules and parts of a product. The materials are listed with their identity and characteristics so that they can be identified within the product and procured.</rdfs:comment>
        <rdfs:label xml:lang="de"></rdfs:label>
        <rdfs:label xml:lang="en">Bill of materials</rdfs:label>
    </owl:NamedIndividual>
    


    <!-- http://iirds.tekom.de/iirds#CEDeclarationOfConformity -->

    <owl:NamedIndividual rdf:about="http://iirds.tekom.de/iirds#CEDeclarationOfConformity">
        <rdf:type rdf:resource="http://iirds.tekom.de/iirds#DocumentType"/>
        <iirds:description xml:lang="en"></iirds:description>
        <rdfs:comment xml:lang="de">Bestätigung des Hersteller (bzw. falls dieser seinen Sitz außerhalb der EU hat, sein Bevollmächtigter mit Sitz in der EU), dass ein von ihm in Verkehr gebrachtes Produkt den grundlegenden Gesundheits- und Sicherheitsanforderungen aller relevanten europäischen Richtlinien entspricht, also mit ihnen konform ist.</rdfs:comment>
        <rdfs:comment xml:lang="en">Type of document. Created as a result of a procedure whereby the manufacture or authorized representative &quot;ensures and declares&quot; that the products concerned satisfy the requirements of the directives that apply to them.</rdfs:comment>
        <rdfs:label xml:lang="en">CE declaration of conformity</rdfs:label>
        <rdfs:label xml:lang="de">CE-Konformitätserklärung</rdfs:label>
    </owl:NamedIndividual>
    


    <!-- http://iirds.tekom.de/iirds#Caution -->

    <owl:NamedIndividual rdf:about="http://iirds.tekom.de/iirds#Caution">
        <rdf:type rdf:resource="http://iirds.tekom.de/iirds#WarningMessage"/>
        <iirds:description xml:lang="en">See ANSI Z535.5</iirds:description>
        <rdfs:comment xml:lang="en">Describes a hazardous situation which, if not avoided, could result in minor or moderate injury.</rdfs:comment>
        <rdfs:label xml:lang="en">Caution</rdfs:label>
        <rdfs:label xml:lang="de">Vorsicht</rdfs:label>
    </owl:NamedIndividual>
    


    <!-- http://iirds.tekom.de/iirds#Certificate -->

    <owl:NamedIndividual rdf:about="http://iirds.tekom.de/iirds#Certificate">
        <rdf:type rdf:resource="http://iirds.tekom.de/iirds#DocumentType"/>
        <iirds:description xml:lang="en">Type of document (VDI 2770). Examples are ATEX certificates, acceptance reports, and material certificates.</iirds:description>
        <rdfs:comment xml:lang="en">Document of legal nature that contains and certifies product information, quality, and characteristics. Usually acknowledged with a signature.</rdfs:comment>
        <rdfs:label xml:lang="en">Certificate</rdfs:label>
        <rdfs:label xml:lang="de">Zertifikat</rdfs:label>
    </owl:NamedIndividual>
    


    <!-- http://iirds.tekom.de/iirds#Collection -->

    <owl:NamedIndividual rdf:about="http://iirds.tekom.de/iirds#Collection"/>
    


    <!-- http://iirds.tekom.de/iirds#Component -->

    <owl:NamedIndividual rdf:about="http://iirds.tekom.de/iirds#Component"/>
    


    <!-- http://iirds.tekom.de/iirds#Concept -->

    <owl:NamedIndividual rdf:about="http://iirds.tekom.de/iirds#Concept"/>
    


    <!-- http://iirds.tekom.de/iirds#Configuration -->

    <owl:NamedIndividual rdf:about="http://iirds.tekom.de/iirds#Configuration">
        <rdf:type rdf:resource="http://iirds.tekom.de/iirds#PuttingToUse"/>
        <iirds:description xml:lang="en"></iirds:description>
        <rdfs:comment xml:lang="en">Lifecycle phase of a product describing activities related to configuring the settings of a technical system before use.</rdfs:comment>
        <rdfs:label xml:lang="en">Configuration</rdfs:label>
        <rdfs:label xml:lang="de">Einrichtung</rdfs:label>
    </owl:NamedIndividual>
    


    <!-- http://iirds.tekom.de/iirds#Conformity -->

    <owl:NamedIndividual rdf:about="http://iirds.tekom.de/iirds#Conformity"/>
    


    <!-- http://iirds.tekom.de/iirds#ContactInformation -->

    <owl:NamedIndividual rdf:about="http://iirds.tekom.de/iirds#ContactInformation">
        <rdf:type rdf:resource="http://iirds.tekom.de/iirds#Formality"/>
        <iirds:description xml:lang="en">Contact information such as addresses, phone numbers, URLs.</iirds:description>
        <rdfs:comment xml:lang="en">Information subject. Contact information of the supplier.</rdfs:comment>
        <rdfs:label xml:lang="en">Contact information</rdfs:label>
        <rdfs:label xml:lang="de">Kontaktdaten</rdfs:label>
    </owl:NamedIndividual>
    


    <!-- http://iirds.tekom.de/iirds#ContentLifeCycleStatus -->

    <owl:NamedIndividual rdf:about="http://iirds.tekom.de/iirds#ContentLifeCycleStatus"/>
    


    <!-- http://iirds.tekom.de/iirds#ContentLifeCycleStatusValue -->

    <owl:NamedIndividual rdf:about="http://iirds.tekom.de/iirds#ContentLifeCycleStatusValue"/>
    


    <!-- http://iirds.tekom.de/iirds#ContractualDocument -->

    <owl:NamedIndividual rdf:about="http://iirds.tekom.de/iirds#ContractualDocument">
        <rdf:type rdf:resource="http://iirds.tekom.de/iirds#DocumentType"/>
        <iirds:description xml:lang="en">Type of document (VDI 2770). Contractual documents include, among others, contracts, acceptance reports, and service conditions.</iirds:description>
        <rdfs:comment xml:lang="en">Document that is part of or accompanies a contract.</rdfs:comment>
        <rdfs:label xml:lang="en">Contractual document</rdfs:label>
        <rdfs:label xml:lang="de">Vertragliches Dokument</rdfs:label>
    </owl:NamedIndividual>
    


    <!-- http://iirds.tekom.de/iirds#Contributor -->

    <owl:NamedIndividual rdf:about="http://iirds.tekom.de/iirds#Contributor">
        <rdf:type rdf:resource="http://iirds.tekom.de/iirds#PartyRole"/>
        <iirds:description xml:lang="en">A contributor is an individual or an organization that participated in the generation/change of the referenced iiRDS domain entity.</iirds:description>
        <rdfs:comment xml:lang="en">Instance of the PartyRole class describing the role of an actor related to an iiRDS domain entity.</rdfs:comment>
        <rdfs:label xml:lang="de">Beteiligter</rdfs:label>
        <rdfs:label xml:lang="en">Contributor</rdfs:label>
    </owl:NamedIndividual>
    


    <!-- http://iirds.tekom.de/iirds#Creator -->

    <owl:NamedIndividual rdf:about="http://iirds.tekom.de/iirds#Creator">
        <rdf:type rdf:resource="http://iirds.tekom.de/iirds#PartyRole"/>
        <iirds:description xml:lang="en">A creator is the individual or the organization that created the referenced iiRDS domain entity.</iirds:description>
        <rdfs:comment xml:lang="en">Instance of the PartyRole class describing the role of an actor related to an iiRDS domain entity.</rdfs:comment>
        <rdfs:label xml:lang="en">Creator</rdfs:label>
        <rdfs:label xml:lang="de">Ersteller</rdfs:label>
    </owl:NamedIndividual>
    


    <!-- http://iirds.tekom.de/iirds#Customer -->

    <owl:NamedIndividual rdf:about="http://iirds.tekom.de/iirds#Customer">
        <rdf:type rdf:resource="http://iirds.tekom.de/iirds#PartyRole"/>
        <iirds:description xml:lang="en">A customer is an individual or an organization that purchased or consumes the referenced iiRDS domain entity.</iirds:description>
        <rdfs:comment xml:lang="en">Instance of the PartyRole class describing the role of an actor related to an iiRDS domain entity.</rdfs:comment>
        <rdfs:label xml:lang="en">Customer</rdfs:label>
        <rdfs:label xml:lang="de">Kunde</rdfs:label>
    </owl:NamedIndividual>
    


    <!-- http://iirds.tekom.de/iirds#Danger -->

    <owl:NamedIndividual rdf:about="http://iirds.tekom.de/iirds#Danger">
        <rdf:type rdf:resource="http://iirds.tekom.de/iirds#WarningMessage"/>
        <iirds:description xml:lang="en">See ANSI Z535.5</iirds:description>
        <rdfs:comment xml:lang="en">Describes a hazardous situation which, if not avoided, will result in death or serious injury.</rdfs:comment>
        <rdfs:label xml:lang="en">Danger</rdfs:label>
        <rdfs:label xml:lang="de">Gefahr</rdfs:label>
    </owl:NamedIndividual>
    


    <!-- http://iirds.tekom.de/iirds#DeclarationOfConformity -->

    <owl:NamedIndividual rdf:about="http://iirds.tekom.de/iirds#DeclarationOfConformity">
        <rdf:type rdf:resource="http://iirds.tekom.de/iirds#Conformity"/>
        <iirds:description xml:lang="en">The Declaration of Conformity states that the product complies with the essential requirements of the relevant standards. </iirds:description>
        <rdfs:comment xml:lang="en">Information subject. Specifies that the information unit deals with the EU Declaration of Conformity for CE marking.</rdfs:comment>
        <rdfs:label xml:lang="en">Declaration of conformity</rdfs:label>
        <rdfs:label xml:lang="de">Konformitätserklärung</rdfs:label>
    </owl:NamedIndividual>
    


    <!-- http://iirds.tekom.de/iirds#Decommissioning -->

    <owl:NamedIndividual rdf:about="http://iirds.tekom.de/iirds#Decommissioning">
        <rdf:type rdf:resource="http://iirds.tekom.de/iirds#Use"/>
        <iirds:description xml:lang="en"></iirds:description>
        <rdfs:comment xml:lang="en">Lifecycle phase of a product describing the shut-down and transfer into a safe state.</rdfs:comment>
        <rdfs:label xml:lang="de">Außerbetriebnahme</rdfs:label>
        <rdfs:label xml:lang="en">Decommissioning</rdfs:label>
    </owl:NamedIndividual>
    


    <!-- http://iirds.tekom.de/iirds#Deleted -->

    <owl:NamedIndividual rdf:about="http://iirds.tekom.de/iirds#Deleted">
        <rdf:type rdf:resource="http://iirds.tekom.de/iirds#ContentLifeCycleStatusValue"/>
        <iirds:description xml:lang="en"></iirds:description>
        <rdfs:comment xml:lang="en">Content lifecycle status value; indicates that the content has been removed.</rdfs:comment>
        <rdfs:label xml:lang="en">Deleted</rdfs:label>
        <rdfs:label xml:lang="de">Gelöscht</rdfs:label>
    </owl:NamedIndividual>
    


    <!-- http://iirds.tekom.de/iirds#Design -->

    <owl:NamedIndividual rdf:about="http://iirds.tekom.de/iirds#Design">
        <rdf:type rdf:resource="http://iirds.tekom.de/iirds#DesignAndRealization"/>
        <iirds:description xml:lang="en"></iirds:description>
        <rdfs:comment xml:lang="en">Lifecycle phase of product design.</rdfs:comment>
        <rdfs:label xml:lang="de">Design</rdfs:label>
        <rdfs:label xml:lang="en">Design</rdfs:label>
    </owl:NamedIndividual>
    


    <!-- http://iirds.tekom.de/iirds#DesignAndRealization -->

    <owl:NamedIndividual rdf:about="http://iirds.tekom.de/iirds#DesignAndRealization"/>
    


    <!-- http://iirds.tekom.de/iirds#Development -->

    <owl:NamedIndividual rdf:about="http://iirds.tekom.de/iirds#Development">
        <rdf:type rdf:resource="http://iirds.tekom.de/iirds#DesignAndRealization"/>
        <iirds:description xml:lang="en"></iirds:description>
        <rdfs:comment xml:lang="en">Lifecycle phase of a product progressing from detailed design to prototyping through pilot release to full product launch.</rdfs:comment>
        <rdfs:label xml:lang="en">Development</rdfs:label>
        <rdfs:label xml:lang="de">Entwicklung</rdfs:label>
    </owl:NamedIndividual>
    


    <!-- http://iirds.tekom.de/iirds#Diagnostics -->

    <owl:NamedIndividual rdf:about="http://iirds.tekom.de/iirds#Diagnostics">
        <rdf:type rdf:resource="http://iirds.tekom.de/iirds#Use"/>
        <iirds:description xml:lang="en"></iirds:description>
        <rdfs:comment xml:lang="en">Lifecycle phase of a product containing procedures for locating errors.</rdfs:comment>
        <rdfs:label xml:lang="en">Diagnostics</rdfs:label>
        <rdfs:label xml:lang="de">Fehlerdiagnose</rdfs:label>
    </owl:NamedIndividual>
    


    <!-- http://iirds.tekom.de/iirds#DirectoryNode -->

    <owl:NamedIndividual rdf:about="http://iirds.tekom.de/iirds#DirectoryNode"/>
    


    <!-- http://iirds.tekom.de/iirds#DirectoryNodeType -->

    <owl:NamedIndividual rdf:about="http://iirds.tekom.de/iirds#DirectoryNodeType"/>
    


    <!-- http://iirds.tekom.de/iirds#Disposal -->

    <owl:NamedIndividual rdf:about="http://iirds.tekom.de/iirds#Disposal">
        <rdf:type rdf:resource="http://iirds.tekom.de/iirds#AfterUse"/>
        <iirds:description xml:lang="en"></iirds:description>
        <rdfs:comment xml:lang="en">Lifecycle phase of a product describing the elimination of components, mounted parts and lubricant considering the country-specific current law.</rdfs:comment>
        <rdfs:label xml:lang="en">Disposal</rdfs:label>
        <rdfs:label xml:lang="de">Entsorgung</rdfs:label>
    </owl:NamedIndividual>
    


    <!-- http://iirds.tekom.de/iirds#Document -->

    <owl:NamedIndividual rdf:about="http://iirds.tekom.de/iirds#Document"/>
    


    <!-- http://iirds.tekom.de/iirds#DocumentType -->

    <owl:NamedIndividual rdf:about="http://iirds.tekom.de/iirds#DocumentType"/>
    


    <!-- http://iirds.tekom.de/iirds#DocumentationMetadata -->

    <owl:NamedIndividual rdf:about="http://iirds.tekom.de/iirds#DocumentationMetadata"/>
    


    <!-- http://iirds.tekom.de/iirds#DownTime -->

    <owl:NamedIndividual rdf:about="http://iirds.tekom.de/iirds#DownTime"/>
    


    <!-- http://iirds.tekom.de/iirds#ElectronicIdentificationPlate -->

    <owl:NamedIndividual rdf:about="http://iirds.tekom.de/iirds#ElectronicIdentificationPlate">
        <rdf:type rdf:resource="http://iirds.tekom.de/iirds#DocumentType"/>
        <iirds:description xml:lang="en">Type of document (VDI 2770)</iirds:description>
        <rdfs:comment xml:lang="en">Electronically readable label on a machine or component that provides information on the identity of the manufacturer and the product, as well as on the technical characteristics of the product.</rdfs:comment>
        <rdfs:label xml:lang="de"></rdfs:label>
        <rdfs:label xml:lang="en">Electronic identification plate</rdfs:label>
    </owl:NamedIndividual>
    


    <!-- http://iirds.tekom.de/iirds#EmergencyOperation -->

    <owl:NamedIndividual rdf:about="http://iirds.tekom.de/iirds#EmergencyOperation">
        <rdf:type rdf:resource="http://iirds.tekom.de/iirds#Use"/>
        <iirds:description xml:lang="en"></iirds:description>
        <rdfs:comment xml:lang="en">Product lifecycle phase of a technical system in which the system&apos;s functionality is reduced to a minimum due to an error or emergency situation.</rdfs:comment>
        <rdfs:label xml:lang="en">Emergency operation</rdfs:label>
        <rdfs:label xml:lang="de">Notbetrieb</rdfs:label>
    </owl:NamedIndividual>
    


    <!-- http://iirds.tekom.de/iirds#Event -->

    <owl:NamedIndividual rdf:about="http://iirds.tekom.de/iirds#Event"/>
    


    <!-- http://iirds.tekom.de/iirds#Fault -->

    <owl:NamedIndividual rdf:about="http://iirds.tekom.de/iirds#Fault">
        <rdf:type rdf:resource="http://iirds.tekom.de/iirds#Use"/>
        <iirds:description xml:lang="en"></iirds:description>
        <rdfs:comment xml:lang="de">Phase im Produktlebenszyklus, in der Störungen des bestimmungsgemäßen Betriebes einer technischen Anlage, einer Software oder eines technischen Systems auftreten.</rdfs:comment>
        <rdfs:comment xml:lang="en">Product lifecycle phase of a technical system in which the intended use and operation of a technical system or software is interrupted due to an error or malfunction.</rdfs:comment>
        <rdfs:label xml:lang="en">Fault</rdfs:label>
        <rdfs:label xml:lang="de">Störung</rdfs:label>
    </owl:NamedIndividual>
    


    <!-- http://iirds.tekom.de/iirds#ForeseeableMisuse -->

    <owl:NamedIndividual rdf:about="http://iirds.tekom.de/iirds#ForeseeableMisuse">
        <rdf:type rdf:resource="http://iirds.tekom.de/iirds#Safety"/>
        <iirds:description xml:lang="en">Use of a product in a manner not intended by the producer or supplier but which may result from foreseeable human behavior. See EN 82079-1</iirds:description>
        <rdfs:comment xml:lang="en">Information subject. Foreseeable misuse of a product.</rdfs:comment>
        <rdfs:label xml:lang="en">Foreseeable misuse</rdfs:label>
        <rdfs:label xml:lang="de">Vorhersehbarer Fehlgebrauch</rdfs:label>
    </owl:NamedIndividual>
    


    <!-- http://iirds.tekom.de/iirds#Form -->

    <owl:NamedIndividual rdf:about="http://iirds.tekom.de/iirds#Form"/>
    


    <!-- http://iirds.tekom.de/iirds#Formality -->

    <owl:NamedIndividual rdf:about="http://iirds.tekom.de/iirds#Formality"/>
    


    <!-- http://iirds.tekom.de/iirds#Fragment -->

    <owl:NamedIndividual rdf:about="http://iirds.tekom.de/iirds#Fragment"/>
    


    <!-- http://iirds.tekom.de/iirds#FragmentSelector -->

    <owl:NamedIndividual rdf:about="http://iirds.tekom.de/iirds#FragmentSelector"/>
    


    <!-- http://iirds.tekom.de/iirds#FunctionalMetadata -->

    <owl:NamedIndividual rdf:about="http://iirds.tekom.de/iirds#FunctionalMetadata"/>
    


    <!-- http://iirds.tekom.de/iirds#Functionality -->

    <owl:NamedIndividual rdf:about="http://iirds.tekom.de/iirds#Functionality"/>
    


    <!-- http://iirds.tekom.de/iirds#GenericAfterUse -->

    <owl:NamedIndividual rdf:about="http://iirds.tekom.de/iirds#GenericAfterUse">
        <rdf:type rdf:resource="http://iirds.tekom.de/iirds#AfterUse"/>
        <iirds:description xml:lang="en">The AfterUse class is a parent class for product lifecycle phases that occur after the active use of the product.</iirds:description>
        <rdfs:comment xml:lang="en">Generic instance of the AfterUse class. </rdfs:comment>
        <rdfs:label xml:lang="en">After use</rdfs:label>
        <rdfs:label xml:lang="de">Nutzungsende</rdfs:label>
    </owl:NamedIndividual>
    


    <!-- http://iirds.tekom.de/iirds#GenericCollection -->

    <owl:NamedIndividual rdf:about="http://iirds.tekom.de/iirds#GenericCollection">
        <rdf:type rdf:resource="http://iirds.tekom.de/iirds#Collection"/>
        <iirds:description xml:lang="en"></iirds:description>
        <rdfs:comment xml:lang="en">Information subject. Indicates that the content represents a collection of information assembled from different information units.</rdfs:comment>
        <rdfs:label xml:lang="en">Collection</rdfs:label>
        <rdfs:label xml:lang="de">Zusammenstellung</rdfs:label>
    </owl:NamedIndividual>
    


    <!-- http://iirds.tekom.de/iirds#GenericConcept -->

    <owl:NamedIndividual rdf:about="http://iirds.tekom.de/iirds#GenericConcept">
        <rdf:type rdf:resource="http://iirds.tekom.de/iirds#Concept"/>
        <iirds:description xml:lang="en">Conceptual information helps users to map their existing knowledge to tasks and other essential information about a product or system.</iirds:description>
        <rdfs:comment xml:lang="en">Topic type that provides background that helps readers understand essential information about a product, interface, or task.</rdfs:comment>
        <rdfs:label xml:lang="de">Beschreibung</rdfs:label>
        <rdfs:label xml:lang="en">Concept</rdfs:label>
    </owl:NamedIndividual>
    


    <!-- http://iirds.tekom.de/iirds#GenericConformity -->

    <owl:NamedIndividual rdf:about="http://iirds.tekom.de/iirds#GenericConformity">
        <rdf:type rdf:resource="http://iirds.tekom.de/iirds#Conformity"/>
        <iirds:description xml:lang="en">The Conformity class is a parent class for information subjects that describe content related to applicable standards or the conformity of the product.</iirds:description>
        <rdfs:comment xml:lang="en">Generic instance of the Conformity class.</rdfs:comment>
        <rdfs:label xml:lang="en">Conformity</rdfs:label>
        <rdfs:label xml:lang="de">Konformität</rdfs:label>
    </owl:NamedIndividual>
    


    <!-- http://iirds.tekom.de/iirds#GenericDesignAndRealization -->

    <owl:NamedIndividual rdf:about="http://iirds.tekom.de/iirds#GenericDesignAndRealization">
        <rdf:type rdf:resource="http://iirds.tekom.de/iirds#DesignAndRealization"/>
        <iirds:description xml:lang="en">The DesignAndRealization class is a parent class for product lifecycle phases related to the design, construction, and realization of a product.</iirds:description>
        <rdfs:comment xml:lang="en">Generic instance of the DesignAndRealization class.</rdfs:comment>
        <rdfs:label xml:lang="en">Design and realization</rdfs:label>
        <rdfs:label xml:lang="de">Produktentstehung</rdfs:label>
    </owl:NamedIndividual>
    


    <!-- http://iirds.tekom.de/iirds#GenericDownTime -->

    <owl:NamedIndividual rdf:about="http://iirds.tekom.de/iirds#GenericDownTime">
        <rdf:type rdf:resource="http://iirds.tekom.de/iirds#DownTime"/>
        <iirds:description xml:lang="en">The DownTime class is a parent class for time periods during which an equipment or machine is not functional or cannot work.</iirds:description>
        <rdfs:comment xml:lang="en">Generic instance of the DownTime class.</rdfs:comment>
        <rdfs:label xml:lang="en">Down time</rdfs:label>
        <rdfs:label xml:lang="de">Stillstandszeit</rdfs:label>
    </owl:NamedIndividual>
    


    <!-- http://iirds.tekom.de/iirds#GenericEvent -->

    <owl:NamedIndividual rdf:about="http://iirds.tekom.de/iirds#GenericEvent">
        <rdf:type rdf:resource="http://iirds.tekom.de/iirds#Event"/>
        <iirds:description xml:lang="en">The Event class describes events that happen in the technical system. Examples are errors, malfunctions, and warnings.</iirds:description>
        <rdfs:comment xml:lang="en">Generic instance of the Event class.</rdfs:comment>
        <rdfs:label xml:lang="de">Ereignis</rdfs:label>
        <rdfs:label xml:lang="en">Event</rdfs:label>
    </owl:NamedIndividual>
    


    <!-- http://iirds.tekom.de/iirds#GenericForm -->

    <owl:NamedIndividual rdf:about="http://iirds.tekom.de/iirds#GenericForm">
        <rdf:type rdf:resource="http://iirds.tekom.de/iirds#Form"/>
        <iirds:description xml:lang="en">The Form class describes topics that contain information in pre-defined form fields. Examples of forms are service reports, field reports, and user feedback.</iirds:description>
        <rdfs:comment xml:lang="en">Generic instance of the Form class.</rdfs:comment>
        <rdfs:label xml:lang="en">Form</rdfs:label>
        <rdfs:label xml:lang="de">Formular</rdfs:label>
    </owl:NamedIndividual>
    


    <!-- http://iirds.tekom.de/iirds#GenericFormality -->

    <owl:NamedIndividual rdf:about="http://iirds.tekom.de/iirds#GenericFormality">
        <rdf:type rdf:resource="http://iirds.tekom.de/iirds#Formality"/>
        <iirds:description xml:lang="en">The Formality class is the parent class for information subjects that describe content related to official or legal documents.</iirds:description>
        <rdfs:comment xml:lang="en">Generic instance of the Formality class.</rdfs:comment>
        <rdfs:label xml:lang="de">Formalie</rdfs:label>
        <rdfs:label xml:lang="en">Formality</rdfs:label>
    </owl:NamedIndividual>
    


    <!-- http://iirds.tekom.de/iirds#GenericFunctionality -->

    <owl:NamedIndividual rdf:about="http://iirds.tekom.de/iirds#GenericFunctionality">
        <rdf:type rdf:resource="http://iirds.tekom.de/iirds#Functionality"/>
        <iirds:description xml:lang="en">The Functionality class is the parent class for information subjects that describe content related to specific functionalities of the product.</iirds:description>
        <rdfs:comment xml:lang="en">Generic instance of the Functionality class.</rdfs:comment>
        <rdfs:label xml:lang="en">Functionality</rdfs:label>
        <rdfs:label xml:lang="de">Funktionalität</rdfs:label>
    </owl:NamedIndividual>
    


    <!-- http://iirds.tekom.de/iirds#GenericLearning -->

    <owl:NamedIndividual rdf:about="http://iirds.tekom.de/iirds#GenericLearning">
        <rdf:type rdf:resource="http://iirds.tekom.de/iirds#Learning"/>
        <iirds:description xml:lang="en">Learning content may comprise learning plans, learning objectives, learning content details, summaries, and assessments.</iirds:description>
        <rdfs:comment xml:lang="en">Topic type that provides learning content.</rdfs:comment>
        <rdfs:label xml:lang="en">Learning</rdfs:label>
        <rdfs:label xml:lang="de">Lernen</rdfs:label>
    </owl:NamedIndividual>
    


    <!-- http://iirds.tekom.de/iirds#GenericMaintenanceInterval -->

    <owl:NamedIndividual rdf:about="http://iirds.tekom.de/iirds#GenericMaintenanceInterval">
        <rdf:type rdf:resource="http://iirds.tekom.de/iirds#MaintenanceInterval"/>
        <iirds:description xml:lang="en">The MaintenanceInterval class describes time intervals and durations for the scheduled maintenance of a technical system or its parts.</iirds:description>
        <rdfs:comment xml:lang="en">Generic instance of the MaintenanceInterval class.</rdfs:comment>
        <rdfs:label xml:lang="en">Maintenance interval</rdfs:label>
        <rdfs:label xml:lang="de">Wartungsintervall</rdfs:label>
    </owl:NamedIndividual>
    


    <!-- http://iirds.tekom.de/iirds#GenericPlanningTime -->

    <owl:NamedIndividual rdf:about="http://iirds.tekom.de/iirds#GenericPlanningTime">
        <rdf:type rdf:resource="http://iirds.tekom.de/iirds#PlanningTime"/>
        <iirds:description xml:lang="en">The PlanningTime class describes different types of planning times that may be referenced in technical documentation, for example time required for or resulting from specific working tasks.</iirds:description>
        <rdfs:comment xml:lang="en">Generic instance of the PlanningTime class.</rdfs:comment>
        <rdfs:label xml:lang="en">Planning time</rdfs:label>
        <rdfs:label xml:lang="de">Planungszeit</rdfs:label>
    </owl:NamedIndividual>
    


    <!-- http://iirds.tekom.de/iirds#GenericProcess -->

    <owl:NamedIndividual rdf:about="http://iirds.tekom.de/iirds#GenericProcess">
        <rdf:type rdf:resource="http://iirds.tekom.de/iirds#Process"/>
        <iirds:description xml:lang="en">The Process class contains information subject for process-related information.</iirds:description>
        <rdfs:comment xml:lang="en">Generic instance of the Process class.</rdfs:comment>
        <rdfs:label xml:lang="en">Process</rdfs:label>
        <rdfs:label xml:lang="de">Prozess</rdfs:label>
    </owl:NamedIndividual>
    


    <!-- http://iirds.tekom.de/iirds#GenericProductFeature -->

    <owl:NamedIndividual rdf:about="http://iirds.tekom.de/iirds#GenericProductFeature">
        <rdf:type rdf:resource="http://iirds.tekom.de/iirds#ProductFeature"/>
        <iirds:description xml:lang="en">The ProductFeature class is a parent class for characteristics and functions of a product or component.</iirds:description>
        <rdfs:comment xml:lang="en">Generic instance of the ProductFeature class.</rdfs:comment>
        <rdfs:label xml:lang="en">Product feature</rdfs:label>
        <rdfs:label xml:lang="de">Produktmerkmal</rdfs:label>
    </owl:NamedIndividual>
    


    <!-- http://iirds.tekom.de/iirds#GenericProductFunction -->

    <owl:NamedIndividual rdf:about="http://iirds.tekom.de/iirds#GenericProductFunction">
        <rdf:type rdf:resource="http://iirds.tekom.de/iirds#ProductFunction"/>
        <iirds:description xml:lang="en">The ProductFunction class describes a function that a product or component provides or implements.</iirds:description>
        <rdfs:comment xml:lang="en">Generic instance of the ProductFunction class.</rdfs:comment>
        <rdfs:label xml:lang="en">Product function</rdfs:label>
        <rdfs:label xml:lang="de">Produktfunktion</rdfs:label>
    </owl:NamedIndividual>
    


    <!-- http://iirds.tekom.de/iirds#GenericProductProperty -->

    <owl:NamedIndividual rdf:about="http://iirds.tekom.de/iirds#GenericProductProperty">
        <rdf:type rdf:resource="http://iirds.tekom.de/iirds#ProductProperty"/>
        <iirds:description xml:lang="en">The ProductProperty class describes a characteristic of a product or component.</iirds:description>
        <rdfs:comment xml:lang="en">Generic instance of the ProductProperty class.</rdfs:comment>
        <rdfs:label xml:lang="en">Product property</rdfs:label>
        <rdfs:label xml:lang="de">Produkteigenschaft</rdfs:label>
    </owl:NamedIndividual>
    


    <!-- http://iirds.tekom.de/iirds#GenericPuttingToUse -->

    <owl:NamedIndividual rdf:about="http://iirds.tekom.de/iirds#GenericPuttingToUse">
        <rdf:type rdf:resource="http://iirds.tekom.de/iirds#PuttingToUse"/>
        <iirds:description xml:lang="en">The PuttingToUse class is a parent class for the product lifecycle phases related to putting a product or technical system to use.</iirds:description>
        <rdfs:comment xml:lang="en">Generic instance of the GenericPuttingToUse class.</rdfs:comment>
        <rdfs:label xml:lang="de">In Nutzung nehmen</rdfs:label>
        <rdfs:label xml:lang="en">Putting to use</rdfs:label>
    </owl:NamedIndividual>
    


    <!-- http://iirds.tekom.de/iirds#GenericReference -->

    <owl:NamedIndividual rdf:about="http://iirds.tekom.de/iirds#GenericReference">
        <rdf:type rdf:resource="http://iirds.tekom.de/iirds#Reference"/>
        <iirds:description xml:lang="en">The Reference class describes a topic type containing information that supports users as they perform a task, meaning data that is looked up rather than memorized. Examples are parameter lists, tables with technical data, UI control overviews, and parts lists. </iirds:description>
        <rdfs:comment xml:lang="en">Generic instance of the Reference class. </rdfs:comment>
        <rdfs:label xml:lang="en">Reference</rdfs:label>
        <rdfs:label xml:lang="de">Referenz</rdfs:label>
    </owl:NamedIndividual>
    


    <!-- http://iirds.tekom.de/iirds#GenericRole -->

    <owl:NamedIndividual rdf:about="http://iirds.tekom.de/iirds#GenericRole">
        <rdf:type rdf:resource="http://iirds.tekom.de/iirds#Role"/>
        <iirds:description xml:lang="en">The Role class describes roles for users of the technical system and the associated technical information.</iirds:description>
        <rdfs:comment xml:lang="en">Generic instance of the Role class.</rdfs:comment>
        <rdfs:label xml:lang="en">Role</rdfs:label>
        <rdfs:label xml:lang="de">Rolle</rdfs:label>
    </owl:NamedIndividual>
    


    <!-- http://iirds.tekom.de/iirds#GenericSafety -->

    <owl:NamedIndividual rdf:about="http://iirds.tekom.de/iirds#GenericSafety">
        <rdf:type rdf:resource="http://iirds.tekom.de/iirds#Safety"/>
        <iirds:description xml:lang="en">The Safety class contains information subjects related to safety.</iirds:description>
        <rdfs:comment xml:lang="en">Generic instance of the Safety class.</rdfs:comment>
        <rdfs:label xml:lang="en">Safety</rdfs:label>
        <rdfs:label xml:lang="de">Sicherheit</rdfs:label>
    </owl:NamedIndividual>
    


    <!-- http://iirds.tekom.de/iirds#GenericSkillLevel -->

    <owl:NamedIndividual rdf:about="http://iirds.tekom.de/iirds#GenericSkillLevel">
        <rdf:type rdf:resource="http://iirds.tekom.de/iirds#SkillLevel"/>
        <iirds:description xml:lang="en">The SkillLevel class describes custom skill levels that the users of the technical system and the associated technical information require.</iirds:description>
        <rdfs:comment xml:lang="en">Generic instance of the SkillLevel class.</rdfs:comment>
        <rdfs:label xml:lang="de">Kenntnisstufe</rdfs:label>
        <rdfs:label xml:lang="en">Skill level</rdfs:label>
    </owl:NamedIndividual>
    


    <!-- http://iirds.tekom.de/iirds#GenericSupply -->

    <owl:NamedIndividual rdf:about="http://iirds.tekom.de/iirds#GenericSupply">
        <rdf:type rdf:resource="http://iirds.tekom.de/iirds#Supply"/>
        <iirds:description xml:lang="en">The Supply class is a parent class for supplies that are required for working tasks described in technical documentation.</iirds:description>
        <rdfs:comment xml:lang="en">Generic instance of the Supply class.</rdfs:comment>
        <rdfs:label xml:lang="en">Generic supply</rdfs:label>
        <rdfs:label xml:lang="de">Hilfsmittel</rdfs:label>
    </owl:NamedIndividual>
    


    <!-- http://iirds.tekom.de/iirds#GenericTask -->

    <owl:NamedIndividual rdf:about="http://iirds.tekom.de/iirds#GenericTask">
        <rdf:type rdf:resource="http://iirds.tekom.de/iirds#Task"/>
        <iirds:description xml:lang="en">Tasks provide instructions and may contain information on other aspects, such as requirements that must be fulfilled or safety instructions.</iirds:description>
        <rdfs:comment xml:lang="en">Topic type that contains procedural information for work activities.</rdfs:comment>
        <rdfs:label xml:lang="de">Aufgabe</rdfs:label>
        <rdfs:label xml:lang="en">Task</rdfs:label>
    </owl:NamedIndividual>
    


    <!-- http://iirds.tekom.de/iirds#GenericTechnicalData -->

    <owl:NamedIndividual rdf:about="http://iirds.tekom.de/iirds#GenericTechnicalData">
        <rdf:type rdf:resource="http://iirds.tekom.de/iirds#TechnicalData"/>
        <iirds:description xml:lang="en">Information that describes the technical characteristics of a product or component.</iirds:description>
        <rdfs:comment xml:lang="en">Generic instance of the TechnicalData class.</rdfs:comment>
        <rdfs:label xml:lang="en">Technical data</rdfs:label>
        <rdfs:label xml:lang="de">Technische Daten</rdfs:label>
    </owl:NamedIndividual>
    


    <!-- http://iirds.tekom.de/iirds#GenericTechnicalOverview -->

    <owl:NamedIndividual rdf:about="http://iirds.tekom.de/iirds#GenericTechnicalOverview">
        <rdf:type rdf:resource="http://iirds.tekom.de/iirds#TechnicalOverview"/>
        <iirds:description xml:lang="en">The TechnicalOverview class is a parent class for information subjects describing contents related to technical plans, diagrams, or the technical architecture of the product.</iirds:description>
        <rdfs:comment xml:lang="en">Generic instance of the TechnicalOverview class.</rdfs:comment>
        <rdfs:label xml:lang="en">Technical overview</rdfs:label>
        <rdfs:label xml:lang="de">Technische Übersicht</rdfs:label>
    </owl:NamedIndividual>
    


    <!-- http://iirds.tekom.de/iirds#GenericTroubleshooting -->

    <owl:NamedIndividual rdf:about="http://iirds.tekom.de/iirds#GenericTroubleshooting">
        <rdf:type rdf:resource="http://iirds.tekom.de/iirds#Troubleshooting"/>
        <iirds:description xml:lang="en">Troubleshooting information may comprise a description of the symptoms, the cause of the error, and a remedy for the error.</iirds:description>
        <rdfs:comment xml:lang="en">Topic type that contains corrective action information that helps to fix an error or remove a malfunction.</rdfs:comment>
        <rdfs:label xml:lang="de">Störungsbeseitigung</rdfs:label>
        <rdfs:label xml:lang="en">Troubleshooting</rdfs:label>
    </owl:NamedIndividual>
    


    <!-- http://iirds.tekom.de/iirds#GenericUse -->

    <owl:NamedIndividual rdf:about="http://iirds.tekom.de/iirds#GenericUse">
        <rdf:type rdf:resource="http://iirds.tekom.de/iirds#Use"/>
        <iirds:description xml:lang="en">The Use class is a parent class for product lifecycle phases related to using a product or technical system.</iirds:description>
        <rdfs:comment xml:lang="en">Generic instance of the Use class.</rdfs:comment>
        <rdfs:label xml:lang="de">Nutzung</rdfs:label>
        <rdfs:label xml:lang="en">Use</rdfs:label>
    </owl:NamedIndividual>
    


    <!-- http://iirds.tekom.de/iirds#GenericWarningMessage -->

    <owl:NamedIndividual rdf:about="http://iirds.tekom.de/iirds#GenericWarningMessage">
        <rdf:type rdf:resource="http://iirds.tekom.de/iirds#WarningMessage"/>
        <iirds:description xml:lang="en">If possible, use Danger, Warning, Caution, or Notice instead.</iirds:description>
        <rdfs:comment xml:lang="en">Warning or notice with unknown severity.</rdfs:comment>
        <rdfs:label xml:lang="de">Warnhinweis</rdfs:label>
        <rdfs:label xml:lang="en">Warning message</rdfs:label>
    </owl:NamedIndividual>
    


    <!-- http://iirds.tekom.de/iirds#GenericWorkingTime -->

    <owl:NamedIndividual rdf:about="http://iirds.tekom.de/iirds#GenericWorkingTime">
        <rdf:type rdf:resource="http://iirds.tekom.de/iirds#WorkingTime"/>
        <iirds:description xml:lang="en">The WorkingTime class is a parent class for periods of time required for a specific working task.</iirds:description>
        <rdfs:comment xml:lang="en">Generic instance of the WorkingTime class. </rdfs:comment>
        <rdfs:label xml:lang="de">Arbeitszeit</rdfs:label>
        <rdfs:label xml:lang="en">Generic working time</rdfs:label>
    </owl:NamedIndividual>
    


    <!-- http://iirds.tekom.de/iirds#IdentificationDocument -->

    <owl:NamedIndividual rdf:about="http://iirds.tekom.de/iirds#IdentificationDocument">
        <rdf:type rdf:resource="http://iirds.tekom.de/iirds#DocumentType"/>
        <iirds:description xml:lang="en">Identifies an object and provides descriptive or classifying information.</iirds:description>
        <rdfs:comment xml:lang="en">Type of document. </rdfs:comment>
        <rdfs:label xml:lang="en">Identification document</rdfs:label>
        <rdfs:label xml:lang="de">Identifikationsdokument</rdfs:label>
    </owl:NamedIndividual>
    


    <!-- http://iirds.tekom.de/iirds#Identity -->

    <owl:NamedIndividual rdf:about="http://iirds.tekom.de/iirds#Identity"/>
    


    <!-- http://iirds.tekom.de/iirds#IdentityDomain -->

    <owl:NamedIndividual rdf:about="http://iirds.tekom.de/iirds#IdentityDomain"/>
    


    <!-- http://iirds.tekom.de/iirds#InPreparation -->

    <owl:NamedIndividual rdf:about="http://iirds.tekom.de/iirds#InPreparation">
        <rdf:type rdf:resource="http://iirds.tekom.de/iirds#ContentLifeCycleStatusValue"/>
        <iirds:description xml:lang="en"></iirds:description>
        <rdfs:comment xml:lang="en">Content lifecycle status value; indicates that the content is not finished yet and is still being edited.</rdfs:comment>
        <rdfs:label xml:lang="de">In Arbeit</rdfs:label>
        <rdfs:label xml:lang="en">In preparation</rdfs:label>
    </owl:NamedIndividual>
    


    <!-- http://iirds.tekom.de/iirds#InReview -->

    <owl:NamedIndividual rdf:about="http://iirds.tekom.de/iirds#InReview">
        <rdf:type rdf:resource="http://iirds.tekom.de/iirds#ContentLifeCycleStatusValue"/>
        <iirds:description xml:lang="en"></iirds:description>
        <rdfs:comment xml:lang="en">Content lifecycle status value; indicates that the content is being reviewed.</rdfs:comment>
        <rdfs:label xml:lang="de">In Review</rdfs:label>
        <rdfs:label xml:lang="en">In review</rdfs:label>
    </owl:NamedIndividual>
    


    <!-- http://iirds.tekom.de/iirds#Index -->

    <owl:NamedIndividual rdf:about="http://iirds.tekom.de/iirds#Index">
        <rdf:type rdf:resource="http://iirds.tekom.de/iirds#DirectoryNodeType"/>
        <iirds:description xml:lang="en"></iirds:description>
        <rdfs:comment xml:lang="en">Index directory type</rdfs:comment>
        <rdfs:comment xml:lang="de">Verzeichnistyp Index</rdfs:comment>
        <rdfs:label xml:lang="de">Index</rdfs:label>
        <rdfs:label xml:lang="en">Index</rdfs:label>
    </owl:NamedIndividual>
    


    <!-- http://iirds.tekom.de/iirds#InformationObject -->

    <owl:NamedIndividual rdf:about="http://iirds.tekom.de/iirds#InformationObject"/>
    


    <!-- http://iirds.tekom.de/iirds#InformationSubject -->

    <owl:NamedIndividual rdf:about="http://iirds.tekom.de/iirds#InformationSubject"/>
    


    <!-- http://iirds.tekom.de/iirds#InformationType -->

    <owl:NamedIndividual rdf:about="http://iirds.tekom.de/iirds#InformationType"/>
    


    <!-- http://iirds.tekom.de/iirds#InformationUnit -->

    <owl:NamedIndividual rdf:about="http://iirds.tekom.de/iirds#InformationUnit"/>
    


    <!-- http://iirds.tekom.de/iirds#Inspector -->

    <owl:NamedIndividual rdf:about="http://iirds.tekom.de/iirds#Inspector">
        <rdf:type rdf:resource="http://iirds.tekom.de/iirds#PartyRole"/>
        <iirds:description xml:lang="en">An inspector is an individual or an organization that supervises or checks the referenced iiRDS domain entity and makes reports.</iirds:description>
        <rdfs:comment xml:lang="en">Instance of the PartyRole class describing the role of an actor related to an iiRDS domain entity.</rdfs:comment>
        <rdfs:label xml:lang="en">Inspector</rdfs:label>
        <rdfs:label xml:lang="de">Prüfer</rdfs:label>
    </owl:NamedIndividual>
    


    <!-- http://iirds.tekom.de/iirds#Installation -->

    <owl:NamedIndividual rdf:about="http://iirds.tekom.de/iirds#Installation">
        <rdf:type rdf:resource="http://iirds.tekom.de/iirds#PuttingToUse"/>
        <iirds:description xml:lang="en"></iirds:description>
        <rdfs:comment xml:lang="en">Lifecycle phase of a product containing procedures for installing and setting up a software or IT system.</rdfs:comment>
        <rdfs:label xml:lang="de">Installation</rdfs:label>
        <rdfs:label xml:lang="en">Installation</rdfs:label>
    </owl:NamedIndividual>
    


    <!-- http://iirds.tekom.de/iirds#InstallationInstructions -->

    <owl:NamedIndividual rdf:about="http://iirds.tekom.de/iirds#InstallationInstructions">
        <rdf:type rdf:resource="http://iirds.tekom.de/iirds#DocumentType"/>
        <iirds:description xml:lang="en">For physical products: instructions enabling the operator to assemble and electrically connect a physical product so that it fulfills its intended use and does not endanger the health and safety of persons. For IT products: Instructions enabling the administrator to set up and potentially configure a program or new version on a computer so that does not endanger data security. </iirds:description>
        <rdfs:comment xml:lang="en">Type of document. Contains instructions enabling the operator or administrator to assemble or install a physical product or software so that it fulfills its intended use.</rdfs:comment>
        <rdfs:label xml:lang="en">Installation instructions</rdfs:label>
        <rdfs:label xml:lang="de">Installationsanleitung</rdfs:label>
    </owl:NamedIndividual>
    


    <!-- http://iirds.tekom.de/iirds#IntendedUse -->

    <owl:NamedIndividual rdf:about="http://iirds.tekom.de/iirds#IntendedUse">
        <rdf:type rdf:resource="http://iirds.tekom.de/iirds#Safety"/>
        <iirds:description xml:lang="en"></iirds:description>
        <rdfs:comment xml:lang="en">Information subject: Legal concept outlining the field of application specified in matters of design and construction of the machinery which is described in the operating instructions/technical documentation, including considerations of the reasonable foreseeable use and potential misuse.</rdfs:comment>
        <rdfs:comment xml:lang="de">Informationsthema: Rechtlicher Begriff für den bei der Konzeption und Konstruktion einer Maschine festgelegten Einsatzbereich, der in der Betriebsanleitung/Technischen Dokumentation beschrieben wird und auch Überlegungen zur vernünftigerweise vorhersehbaren Verwendung bzw. zu möglicher Fehlverwendung beinhaltet.</rdfs:comment>
        <rdfs:label xml:lang="de">Bestimmungsgemäße Verwendung</rdfs:label>
        <rdfs:label xml:lang="en">Intended use</rdfs:label>
    </owl:NamedIndividual>
    


    <!-- http://iirds.tekom.de/iirds#Learning -->

    <owl:NamedIndividual rdf:about="http://iirds.tekom.de/iirds#Learning"/>
    


    <!-- http://iirds.tekom.de/iirds#LegalInformation -->

    <owl:NamedIndividual rdf:about="http://iirds.tekom.de/iirds#LegalInformation">
        <rdf:type rdf:resource="http://iirds.tekom.de/iirds#Formality"/>
        <iirds:description xml:lang="en"></iirds:description>
        <rdfs:comment xml:lang="en">Information subject for legal information.</rdfs:comment>
        <rdfs:label xml:lang="en">Legal information</rdfs:label>
        <rdfs:label xml:lang="de">Rechtlicher Hinweis</rdfs:label>
    </owl:NamedIndividual>
    


    <!-- http://iirds.tekom.de/iirds#LicenceTerm -->

    <owl:NamedIndividual rdf:about="http://iirds.tekom.de/iirds#LicenceTerm">
        <rdf:type rdf:resource="http://iirds.tekom.de/iirds#Formality"/>
        <iirds:description xml:lang="en"></iirds:description>
        <rdfs:comment xml:lang="en">Information subject describing licensing conditions.</rdfs:comment>
        <rdfs:label xml:lang="en">License terms</rdfs:label>
        <rdfs:label xml:lang="de">Lizenzbedingung</rdfs:label>
    </owl:NamedIndividual>
    


    <!-- http://iirds.tekom.de/iirds#ListOfFigures -->

    <owl:NamedIndividual rdf:about="http://iirds.tekom.de/iirds#ListOfFigures">
        <rdf:type rdf:resource="http://iirds.tekom.de/iirds#DirectoryNodeType"/>
        <iirds:synonym>LOF</iirds:synonym>
        <iirds:description xml:lang="en">Type of directory</iirds:description>
        <rdfs:comment xml:lang="de">Abbildungsverzeichnis</rdfs:comment>
        <rdfs:comment xml:lang="en">List of figures</rdfs:comment>
        <rdfs:label xml:lang="de">Abbildungsverzeichnis</rdfs:label>
        <rdfs:label xml:lang="en">List of figures</rdfs:label>
    </owl:NamedIndividual>
    


    <!-- http://iirds.tekom.de/iirds#ListOfListings -->

    <owl:NamedIndividual rdf:about="http://iirds.tekom.de/iirds#ListOfListings">
        <rdf:type rdf:resource="http://iirds.tekom.de/iirds#DirectoryNodeType"/>
        <iirds:synonym>LOL</iirds:synonym>
        <iirds:description xml:lang="en">Type of directory</iirds:description>
        <rdfs:comment xml:lang="en">Code listing</rdfs:comment>
        <rdfs:comment xml:lang="de">Verzeichnistyp für Programmcode</rdfs:comment>
        <rdfs:label xml:lang="de">Codeverzeichnis</rdfs:label>
        <rdfs:label xml:lang="en">List of listings</rdfs:label>
    </owl:NamedIndividual>
    


    <!-- http://iirds.tekom.de/iirds#ListOfTables -->

    <owl:NamedIndividual rdf:about="http://iirds.tekom.de/iirds#ListOfTables">
        <rdf:type rdf:resource="http://iirds.tekom.de/iirds#DirectoryNodeType"/>
        <iirds:synonym>LOT</iirds:synonym>
        <iirds:description xml:lang="en">Type of directory</iirds:description>
        <rdfs:comment xml:lang="en">List of tables</rdfs:comment>
        <rdfs:comment xml:lang="de">Tabellenverzeichnis</rdfs:comment>
        <rdfs:label xml:lang="en">List of tables</rdfs:label>
        <rdfs:label xml:lang="de">Tabellenverzeichnis</rdfs:label>
    </owl:NamedIndividual>
    


    <!-- http://iirds.tekom.de/iirds#Maintenance -->

    <owl:NamedIndividual rdf:about="http://iirds.tekom.de/iirds#Maintenance">
        <rdf:type rdf:resource="http://iirds.tekom.de/iirds#Use"/>
        <iirds:description xml:lang="en"></iirds:description>
        <rdfs:comment xml:lang="en">Lifecycle phase of a product that describes activities for moving or conveying the product from one place to another.</rdfs:comment>
        <rdfs:label xml:lang="en">Maintenance</rdfs:label>
        <rdfs:label xml:lang="de">Wartung</rdfs:label>
    </owl:NamedIndividual>
    


    <!-- http://iirds.tekom.de/iirds#MaintenanceInstructions -->

    <owl:NamedIndividual rdf:about="http://iirds.tekom.de/iirds#MaintenanceInstructions">
        <rdf:type rdf:resource="http://iirds.tekom.de/iirds#DocumentType"/>
        <iirds:description xml:lang="en"></iirds:description>
        <rdfs:comment xml:lang="en">Type of document. Contains instructions for retaining or restoring a piece of equipment, machine, or system to the specified operable condition.</rdfs:comment>
        <rdfs:label xml:lang="en">Maintenance instructions</rdfs:label>
        <rdfs:label xml:lang="de">Wartungsanleitung</rdfs:label>
    </owl:NamedIndividual>
    


    <!-- http://iirds.tekom.de/iirds#MaintenanceInterval -->

    <owl:NamedIndividual rdf:about="http://iirds.tekom.de/iirds#MaintenanceInterval"/>
    


    <!-- http://iirds.tekom.de/iirds#Manufacturer -->

    <owl:NamedIndividual rdf:about="http://iirds.tekom.de/iirds#Manufacturer">
        <rdf:type rdf:resource="http://iirds.tekom.de/iirds#PartyRole"/>
        <iirds:description xml:lang="en">The manufacturer is the individual or the organization that produces the referenced iiRDS domain entity.</iirds:description>
        <rdfs:comment xml:lang="en">Instance of the PartyRole class describing the role of an actor related to an iiRDS domain entity.</rdfs:comment>
        <rdfs:label xml:lang="de">Hersteller</rdfs:label>
        <rdfs:label xml:lang="en">Manufacturer</rdfs:label>
    </owl:NamedIndividual>
    


    <!-- http://iirds.tekom.de/iirds#ManufacturerInformation -->

    <owl:NamedIndividual rdf:about="http://iirds.tekom.de/iirds#ManufacturerInformation">
        <rdf:type rdf:resource="http://iirds.tekom.de/iirds#Formality"/>
        <iirds:description xml:lang="en"></iirds:description>
        <rdfs:comment xml:lang="en">Information subject. Information about the manufacturer of a product like name and address.</rdfs:comment>
        <rdfs:label xml:lang="de">Herstellerinformation</rdfs:label>
        <rdfs:label xml:lang="en">Manufacturer information</rdfs:label>
    </owl:NamedIndividual>
    


    <!-- http://iirds.tekom.de/iirds#Notice -->

    <owl:NamedIndividual rdf:about="http://iirds.tekom.de/iirds#Notice">
        <rdf:type rdf:resource="http://iirds.tekom.de/iirds#WarningMessage"/>
        <iirds:description xml:lang="en">See ANSI Z535.5</iirds:description>
        <rdfs:comment xml:lang="en">Information considered important but not related to personal injury.</rdfs:comment>
        <rdfs:label xml:lang="de">Hinweis</rdfs:label>
        <rdfs:label xml:lang="en">Notice</rdfs:label>
    </owl:NamedIndividual>
    


    <!-- http://iirds.tekom.de/iirds#OperatingElement -->

    <owl:NamedIndividual rdf:about="http://iirds.tekom.de/iirds#OperatingElement">
        <rdf:type rdf:resource="http://iirds.tekom.de/iirds#TechnicalOverview"/>
        <iirds:description xml:lang="en"></iirds:description>
        <rdfs:comment xml:lang="en">Information subject. Describes a device that a person can use to influence a machine or plant.</rdfs:comment>
        <rdfs:label xml:lang="de">Bedienelement</rdfs:label>
        <rdfs:label xml:lang="en">Control element</rdfs:label>
    </owl:NamedIndividual>
    


    <!-- http://iirds.tekom.de/iirds#OperatingInstructions -->

    <owl:NamedIndividual rdf:about="http://iirds.tekom.de/iirds#OperatingInstructions">
        <rdf:type rdf:resource="http://iirds.tekom.de/iirds#DocumentType"/>
        <iirds:description xml:lang="de">Anleitung, die den Anwender dazu befähigt, ein Gerät, eine Maschine oder eine Software so zu betreiben, dass das Gerät oder die Maschine die bestimmungsgemäße Verwendung erfüllt und die Sicherheit und Gesundheit von Personen nicht beeinträchtigt wird.</iirds:description>
        <iirds:description xml:lang="en">The instructions in this document type enable the user to operate a device, machine, or software considering the reference use as well as the safety and health regulations for the product.</iirds:description>
        <rdfs:comment xml:lang="en">Type of document. Contains instructions for operation and use of a technical system.</rdfs:comment>
        <rdfs:label xml:lang="de">Betriebsanleitung</rdfs:label>
        <rdfs:label xml:lang="en">Operating instructions</rdfs:label>
    </owl:NamedIndividual>
    


    <!-- http://iirds.tekom.de/iirds#Operation -->

    <owl:NamedIndividual rdf:about="http://iirds.tekom.de/iirds#Operation">
        <rdf:type rdf:resource="http://iirds.tekom.de/iirds#Use"/>
        <iirds:description xml:lang="en"></iirds:description>
        <rdfs:comment xml:lang="en">Lifecycle phase of a product in which a technical product or system is actively used and operated.</rdfs:comment>
        <rdfs:label xml:lang="de">Betrieb</rdfs:label>
        <rdfs:label xml:lang="en">Operation</rdfs:label>
    </owl:NamedIndividual>
    


    <!-- http://iirds.tekom.de/iirds#Package -->

    <owl:NamedIndividual rdf:about="http://iirds.tekom.de/iirds#Package"/>
    


    <!-- http://iirds.tekom.de/iirds#PartsCatalog -->

    <owl:NamedIndividual rdf:about="http://iirds.tekom.de/iirds#PartsCatalog">
        <rdf:type rdf:resource="http://iirds.tekom.de/iirds#DocumentType"/>
        <iirds:description xml:lang="en"></iirds:description>
        <rdfs:comment xml:lang="en">Type of document. Contains listings of product names and their part numbers and graphics which are necessary for the aftersales service, but do not include prices or availabilities.</rdfs:comment>
        <rdfs:label xml:lang="en">Parts catalog</rdfs:label>
        <rdfs:label xml:lang="de">Teilekatalog</rdfs:label>
    </owl:NamedIndividual>
    


    <!-- http://iirds.tekom.de/iirds#Party -->

    <owl:NamedIndividual rdf:about="http://iirds.tekom.de/iirds#Party"/>
    


    <!-- http://iirds.tekom.de/iirds#PartyRole -->

    <owl:NamedIndividual rdf:about="http://iirds.tekom.de/iirds#PartyRole"/>
    


    <!-- http://iirds.tekom.de/iirds#PerformedBy -->

    <owl:NamedIndividual rdf:about="http://iirds.tekom.de/iirds#PerformedBy">
        <rdf:type rdf:resource="http://iirds.tekom.de/iirds#PartyRole"/>
        <iirds:description xml:lang="en">Describes the actor that is involved in changing the content lifecycle status.</iirds:description>
        <rdfs:comment xml:lang="en">Instance of the PartyRole class describing the role of an actor related to an iiRDS domain entity.</rdfs:comment>
        <rdfs:label xml:lang="de">Durchgeführt von</rdfs:label>
        <rdfs:label xml:lang="en">Performed by</rdfs:label>
    </owl:NamedIndividual>
    


    <!-- http://iirds.tekom.de/iirds#Plan -->

    <owl:NamedIndividual rdf:about="http://iirds.tekom.de/iirds#Plan">
        <rdf:type rdf:resource="http://iirds.tekom.de/iirds#DocumentType"/>
        <iirds:description xml:lang="en">Type of document (VDI 2770).</iirds:description>
        <rdfs:comment xml:lang="en">Describes documents containing technical plans for a component or machine.</rdfs:comment>
        <rdfs:label xml:lang="de"></rdfs:label>
        <rdfs:label xml:lang="en">Plan</rdfs:label>
    </owl:NamedIndividual>
    


    <!-- http://iirds.tekom.de/iirds#PlanningTime -->

    <owl:NamedIndividual rdf:about="http://iirds.tekom.de/iirds#PlanningTime"/>
    


    <!-- http://iirds.tekom.de/iirds#Process -->

    <owl:NamedIndividual rdf:about="http://iirds.tekom.de/iirds#Process"/>
    


    <!-- http://iirds.tekom.de/iirds#ProductFeature -->

    <owl:NamedIndividual rdf:about="http://iirds.tekom.de/iirds#ProductFeature"/>
    


    <!-- http://iirds.tekom.de/iirds#ProductFunction -->

    <owl:NamedIndividual rdf:about="http://iirds.tekom.de/iirds#ProductFunction"/>
    


    <!-- http://iirds.tekom.de/iirds#ProductIdentification -->

    <owl:NamedIndividual rdf:about="http://iirds.tekom.de/iirds#ProductIdentification">
        <rdf:type rdf:resource="http://iirds.tekom.de/iirds#Formality"/>
        <iirds:description xml:lang="en"></iirds:description>
        <rdfs:comment xml:lang="en">Information subject: Describes a name plate or similar that identifies the product.</rdfs:comment>
        <rdfs:label xml:lang="en">Product identification</rdfs:label>
        <rdfs:label xml:lang="de">Produktidentifikation</rdfs:label>
    </owl:NamedIndividual>
    


    <!-- http://iirds.tekom.de/iirds#ProductLifeCyclePhase -->

    <owl:NamedIndividual rdf:about="http://iirds.tekom.de/iirds#ProductLifeCyclePhase"/>
    


    <!-- http://iirds.tekom.de/iirds#ProductMetadata -->

    <owl:NamedIndividual rdf:about="http://iirds.tekom.de/iirds#ProductMetadata"/>
    


    <!-- http://iirds.tekom.de/iirds#ProductName -->

    <owl:NamedIndividual rdf:about="http://iirds.tekom.de/iirds#ProductName">
        <rdf:type rdf:resource="http://iirds.tekom.de/iirds#Formality"/>
        <iirds:description xml:lang="en"></iirds:description>
        <rdfs:comment xml:lang="en">Information subject. Contains the name of the product.</rdfs:comment>
        <rdfs:label xml:lang="en">Product name</rdfs:label>
        <rdfs:label xml:lang="de">Produktbezeichnung</rdfs:label>
    </owl:NamedIndividual>
    


    <!-- http://iirds.tekom.de/iirds#ProductProperty -->

    <owl:NamedIndividual rdf:about="http://iirds.tekom.de/iirds#ProductProperty"/>
    


    <!-- http://iirds.tekom.de/iirds#ProductVariant -->

    <owl:NamedIndividual rdf:about="http://iirds.tekom.de/iirds#ProductVariant"/>
    


    <!-- http://iirds.tekom.de/iirds#Production -->

    <owl:NamedIndividual rdf:about="http://iirds.tekom.de/iirds#Production">
        <rdf:type rdf:resource="http://iirds.tekom.de/iirds#DesignAndRealization"/>
        <iirds:description xml:lang="en"></iirds:description>
        <rdfs:comment xml:lang="en">Lifecycle phase of a product in which the product is manufactured.</rdfs:comment>
        <rdfs:label xml:lang="de">Herstellung</rdfs:label>
        <rdfs:label xml:lang="en">Production</rdfs:label>
    </owl:NamedIndividual>
    


    <!-- http://iirds.tekom.de/iirds#PuttingToUse -->

    <owl:NamedIndividual rdf:about="http://iirds.tekom.de/iirds#PuttingToUse"/>
    


    <!-- http://iirds.tekom.de/iirds#Qualification -->

    <owl:NamedIndividual rdf:about="http://iirds.tekom.de/iirds#Qualification"/>
    


    <!-- http://iirds.tekom.de/iirds#QuickGuide -->

    <owl:NamedIndividual rdf:about="http://iirds.tekom.de/iirds#QuickGuide">
        <rdf:type rdf:resource="http://iirds.tekom.de/iirds#DocumentType"/>
        <iirds:description xml:lang="en"></iirds:description>
        <rdfs:comment xml:lang="en">Type of document. Describes a short document that contains selected instructions for a specific user group or purpose.</rdfs:comment>
        <rdfs:label xml:lang="de">Kurzanleitung</rdfs:label>
        <rdfs:label xml:lang="en">Quick reference guide</rdfs:label>
    </owl:NamedIndividual>
    


    <!-- http://iirds.tekom.de/iirds#RangeSelector -->

    <owl:NamedIndividual rdf:about="http://iirds.tekom.de/iirds#RangeSelector"/>
    


    <!-- http://iirds.tekom.de/iirds#Reference -->

    <owl:NamedIndividual rdf:about="http://iirds.tekom.de/iirds#Reference"/>
    


    <!-- http://iirds.tekom.de/iirds#Released -->

    <owl:NamedIndividual rdf:about="http://iirds.tekom.de/iirds#Released">
        <rdf:type rdf:resource="http://iirds.tekom.de/iirds#ContentLifeCycleStatusValue"/>
        <iirds:description xml:lang="en"></iirds:description>
        <rdfs:comment xml:lang="en">Content lifecycle status value; indicates that the content has been released.</rdfs:comment>
        <rdfs:label xml:lang="en">Released</rdfs:label>
        <rdfs:label xml:lang="de">Veröffentlicht</rdfs:label>
    </owl:NamedIndividual>
    


    <!-- http://iirds.tekom.de/iirds#Rendition -->

    <owl:NamedIndividual rdf:about="http://iirds.tekom.de/iirds#Rendition"/>
    


    <!-- http://iirds.tekom.de/iirds#Repair -->

    <owl:NamedIndividual rdf:about="http://iirds.tekom.de/iirds#Repair">
        <rdf:type rdf:resource="http://iirds.tekom.de/iirds#Use"/>
        <iirds:description xml:lang="en"></iirds:description>
        <rdfs:comment xml:lang="en">Lifecycle phase of a product that describes activities for restoring the product to a working and sound condition after damage or wear and tear.</rdfs:comment>
        <rdfs:label xml:lang="en">Repair</rdfs:label>
        <rdfs:label xml:lang="de">Reparatur</rdfs:label>
    </owl:NamedIndividual>
    


    <!-- http://iirds.tekom.de/iirds#RepairInstructions -->

    <owl:NamedIndividual rdf:about="http://iirds.tekom.de/iirds#RepairInstructions">
        <rdf:type rdf:resource="http://iirds.tekom.de/iirds#DocumentType"/>
        <iirds:description xml:lang="de">Anleitung, die den Anwender dazu befähigt, ein Gerät oder eine Maschine so instandzusetzen, dass das Gerät oder die Maschine die bestimmungsgemäße Verwendung erfüllt und die Sicherheit und Gesundheit von Personen nicht beeinträchtigt wird.</iirds:description>
        <iirds:description xml:lang="en">The instructions in this document type enable the user to repair a device, machine, or system considering the reference use as well as the safety and health regulations for the product.</iirds:description>
        <rdfs:comment xml:lang="en">Type of document. Contains instructions for restoring a product to a working condition.</rdfs:comment>
        <rdfs:label xml:lang="en">Repair instructions</rdfs:label>
        <rdfs:label xml:lang="de">Reparaturanleitung</rdfs:label>
    </owl:NamedIndividual>
    


    <!-- http://iirds.tekom.de/iirds#RequirementsAnalysis -->

    <owl:NamedIndividual rdf:about="http://iirds.tekom.de/iirds#RequirementsAnalysis">
        <rdf:type rdf:resource="http://iirds.tekom.de/iirds#DesignAndRealization"/>
        <iirds:description xml:lang="en"></iirds:description>
        <rdfs:comment xml:lang="en">Lifecycle phase of a product belonging to the product design; comprises the analysis and definition of requirements for the future product.</rdfs:comment>
        <rdfs:label xml:lang="de">Anforderungsanalyse</rdfs:label>
        <rdfs:label xml:lang="en">Requirement analysis</rdfs:label>
    </owl:NamedIndividual>
    


    <!-- http://iirds.tekom.de/iirds#RestrictionOnUse -->

    <owl:NamedIndividual rdf:about="http://iirds.tekom.de/iirds#RestrictionOnUse">
        <rdf:type rdf:resource="http://iirds.tekom.de/iirds#Safety"/>
        <iirds:description xml:lang="en"></iirds:description>
        <rdfs:comment xml:lang="en">Information subjects. Specifies that there are restrictions regarding the use of the product.</rdfs:comment>
        <rdfs:label xml:lang="de">Einsatzbeschränkungen</rdfs:label>
        <rdfs:label xml:lang="en">Restriction on use</rdfs:label>
    </owl:NamedIndividual>
    


    <!-- http://iirds.tekom.de/iirds#Reviewed -->

    <owl:NamedIndividual rdf:about="http://iirds.tekom.de/iirds#Reviewed">
        <rdf:type rdf:resource="http://iirds.tekom.de/iirds#ContentLifeCycleStatusValue"/>
        <iirds:description xml:lang="en"></iirds:description>
        <rdfs:comment xml:lang="en">Content lifecycle status value; indicates that the content has been reviewed.</rdfs:comment>
        <rdfs:label xml:lang="de">Review durchgeführt</rdfs:label>
        <rdfs:label xml:lang="en">Reviewed</rdfs:label>
    </owl:NamedIndividual>
    


    <!-- http://iirds.tekom.de/iirds#RiskAssessment -->

    <owl:NamedIndividual rdf:about="http://iirds.tekom.de/iirds#RiskAssessment">
        <rdf:type rdf:resource="http://iirds.tekom.de/iirds#Conformity"/>
        <iirds:description xml:lang="en">A risk assessment determines the risks and hazards to life, environment, or machine functioning including a quantitative and qualitative estimate.</iirds:description>
        <rdfs:comment xml:lang="en">Information subject related to conformity. Specifies that the information unit contains information on the risk assessment made within the safety engineering of the product.</rdfs:comment>
        <rdfs:label xml:lang="de">Risikobewertung</rdfs:label>
        <rdfs:label xml:lang="en">Risk assessment</rdfs:label>
    </owl:NamedIndividual>
    


    <!-- http://iirds.tekom.de/iirds#Role -->

    <owl:NamedIndividual rdf:about="http://iirds.tekom.de/iirds#Role"/>
    


    <!-- http://iirds.tekom.de/iirds#Safety -->

    <owl:NamedIndividual rdf:about="http://iirds.tekom.de/iirds#Safety"/>
    


    <!-- http://iirds.tekom.de/iirds#SafetyInstruction -->

    <owl:NamedIndividual rdf:about="http://iirds.tekom.de/iirds#SafetyInstruction">
        <rdf:type rdf:resource="http://iirds.tekom.de/iirds#Safety"/>
        <iirds:description xml:lang="en"></iirds:description>
        <rdfs:comment xml:lang="en">Information subject. Safety instructions explain to the user how to handle a product in a safe way.</rdfs:comment>
        <rdfs:label xml:lang="en">Safety instruction</rdfs:label>
        <rdfs:label xml:lang="de">Sicherheitshinweis</rdfs:label>
    </owl:NamedIndividual>
    


    <!-- http://iirds.tekom.de/iirds#SafetyInstructions -->

    <owl:NamedIndividual rdf:about="http://iirds.tekom.de/iirds#SafetyInstructions">
        <rdf:type rdf:resource="http://iirds.tekom.de/iirds#DocumentType"/>
        <iirds:description xml:lang="en">Type of document (VDI 2770). Examples are documents about the intended use of the product, protection/safety measures, safety equipment, and explosion prevention. </iirds:description>
        <rdfs:comment xml:lang="en">Contains general safety-related information provided by the manufacturer that must be considered during assembly, operation, maintenance, repair, and disassembly of the product. Safety information related to individual tasks is provided in the tasks.</rdfs:comment>
        <rdfs:label xml:lang="en">Safety instructions</rdfs:label>
        <rdfs:label xml:lang="de">Sicherheitsanleitung</rdfs:label>
    </owl:NamedIndividual>
    


    <!-- http://iirds.tekom.de/iirds#SalesCatalog -->

    <owl:NamedIndividual rdf:about="http://iirds.tekom.de/iirds#SalesCatalog">
        <rdf:type rdf:resource="http://iirds.tekom.de/iirds#DocumentType"/>
        <iirds:description xml:lang="en"></iirds:description>
        <rdfs:comment xml:lang="en">Type of document. Contains listings of available products of a producing company with consumers as the target group.</rdfs:comment>
        <rdfs:label xml:lang="en">Sales catalog</rdfs:label>
        <rdfs:label xml:lang="de">Verkaufskatalog</rdfs:label>
    </owl:NamedIndividual>
    


    <!-- http://iirds.tekom.de/iirds#ScopeOfDelivery -->

    <owl:NamedIndividual rdf:about="http://iirds.tekom.de/iirds#ScopeOfDelivery">
        <rdf:type rdf:resource="http://iirds.tekom.de/iirds#Formality"/>
        <iirds:description xml:lang="en"></iirds:description>
        <rdfs:comment xml:lang="en">Information subject. Specifies the scope of the delivery.</rdfs:comment>
        <rdfs:label xml:lang="de">Lieferumfang</rdfs:label>
        <rdfs:label xml:lang="en">Scope of delivery</rdfs:label>
    </owl:NamedIndividual>
    


    <!-- http://iirds.tekom.de/iirds#Selector -->

    <owl:NamedIndividual rdf:about="http://iirds.tekom.de/iirds#Selector"/>
    


    <!-- http://iirds.tekom.de/iirds#SkillLevel -->

    <owl:NamedIndividual rdf:about="http://iirds.tekom.de/iirds#SkillLevel"/>
    


    <!-- http://iirds.tekom.de/iirds#Specification -->

    <owl:NamedIndividual rdf:about="http://iirds.tekom.de/iirds#Specification">
        <rdf:type rdf:resource="http://iirds.tekom.de/iirds#DocumentType"/>
        <iirds:description xml:lang="en"></iirds:description>
        <rdfs:comment xml:lang="en">Type of document. Contains requirements and/or statements describing properties and qualities of a product to be built or manufactured.</rdfs:comment>
        <rdfs:label xml:lang="en">Specification</rdfs:label>
        <rdfs:label xml:lang="de">Spezifikation</rdfs:label>
    </owl:NamedIndividual>
    


    <!-- http://iirds.tekom.de/iirds#Supplier -->

    <owl:NamedIndividual rdf:about="http://iirds.tekom.de/iirds#Supplier">
        <rdf:type rdf:resource="http://iirds.tekom.de/iirds#PartyRole"/>
        <iirds:description xml:lang="en">Describes the individual or the organization that provides the referenced iiRDS domain entity, e.g. a component.</iirds:description>
        <rdfs:comment xml:lang="en">Instance of the PartyRole class describing the role of an actor related to an iiRDS domain entity.</rdfs:comment>
        <rdfs:label xml:lang="en">Supplier</rdfs:label>
        <rdfs:label xml:lang="de">Zulieferer</rdfs:label>
    </owl:NamedIndividual>
    


    <!-- http://iirds.tekom.de/iirds#Supply -->

    <owl:NamedIndividual rdf:about="http://iirds.tekom.de/iirds#Supply"/>
    


    <!-- http://iirds.tekom.de/iirds#Symbol -->

    <owl:NamedIndividual rdf:about="http://iirds.tekom.de/iirds#Symbol">
        <rdf:type rdf:resource="http://iirds.tekom.de/iirds#TechnicalOverview"/>
        <iirds:description xml:lang="en"></iirds:description>
        <rdfs:comment xml:lang="en">Information subject. Contains a list and explanation of symbols used in the documentation.</rdfs:comment>
        <rdfs:label xml:lang="de">Symbol</rdfs:label>
        <rdfs:label xml:lang="en">Symbol</rdfs:label>
    </owl:NamedIndividual>
    


    <!-- http://iirds.tekom.de/iirds#TableOfContents -->

    <owl:NamedIndividual rdf:about="http://iirds.tekom.de/iirds#TableOfContents">
        <rdf:type rdf:resource="http://iirds.tekom.de/iirds#DirectoryNodeType"/>
        <iirds:synonym>TOC</iirds:synonym>
        <iirds:description xml:lang="en">Directory type</iirds:description>
        <rdfs:comment xml:lang="de">Inhaltsverzeichnis</rdfs:comment>
        <rdfs:comment xml:lang="en">Table of contents</rdfs:comment>
        <rdfs:label xml:lang="de">Inhaltsverzeichnis</rdfs:label>
        <rdfs:label xml:lang="en">Table of contents</rdfs:label>
    </owl:NamedIndividual>
    


    <!-- http://iirds.tekom.de/iirds#Task -->

    <owl:NamedIndividual rdf:about="http://iirds.tekom.de/iirds#Task"/>
    


    <!-- http://iirds.tekom.de/iirds#TechnicalData -->

    <owl:NamedIndividual rdf:about="http://iirds.tekom.de/iirds#TechnicalData"/>
    


    <!-- http://iirds.tekom.de/iirds#TechnicalDrawingDiagram -->

    <owl:NamedIndividual rdf:about="http://iirds.tekom.de/iirds#TechnicalDrawingDiagram">
        <rdf:type rdf:resource="http://iirds.tekom.de/iirds#DocumentType"/>
        <iirds:description xml:lang="en">A technical drawing or diagram.</iirds:description>
        <rdfs:comment xml:lang="en">Type of document. Examples are flow diagrams and circuit diagrams.</rdfs:comment>
        <rdfs:label xml:lang="en">Technical drawing/diagram</rdfs:label>
        <rdfs:label xml:lang="de">Technische Zeichnung/Diagramm</rdfs:label>
    </owl:NamedIndividual>
    


    <!-- http://iirds.tekom.de/iirds#TechnicalOverview -->

    <owl:NamedIndividual rdf:about="http://iirds.tekom.de/iirds#TechnicalOverview"/>
    


    <!-- http://iirds.tekom.de/iirds#TechnicalReport -->

    <owl:NamedIndividual rdf:about="http://iirds.tekom.de/iirds#TechnicalReport">
        <rdf:type rdf:resource="http://iirds.tekom.de/iirds#Conformity"/>
        <iirds:description xml:lang="en"></iirds:description>
        <rdfs:comment xml:lang="en">Information subject related to conformity. Specifies that the information unit represents a report regarding the activities or working tasks related to the product. </rdfs:comment>
        <rdfs:label xml:lang="en">Technical report</rdfs:label>
        <rdfs:label xml:lang="de">Technischer Bericht</rdfs:label>
    </owl:NamedIndividual>
    


    <!-- http://iirds.tekom.de/iirds#Topic -->

    <owl:NamedIndividual rdf:about="http://iirds.tekom.de/iirds#Topic"/>
    


    <!-- http://iirds.tekom.de/iirds#TopicType -->

    <owl:NamedIndividual rdf:about="http://iirds.tekom.de/iirds#TopicType"/>
    


    <!-- http://iirds.tekom.de/iirds#TransportInstructions -->

    <owl:NamedIndividual rdf:about="http://iirds.tekom.de/iirds#TransportInstructions">
        <rdf:type rdf:resource="http://iirds.tekom.de/iirds#DocumentType"/>
        <iirds:description xml:lang="en"></iirds:description>
        <rdfs:comment xml:lang="en">Type of document. Contains instructions for transporting the product or its components from one place to another.</rdfs:comment>
        <rdfs:label xml:lang="en">Transport instructions</rdfs:label>
        <rdfs:label xml:lang="de">Transportanleitung</rdfs:label>
    </owl:NamedIndividual>
    


    <!-- http://iirds.tekom.de/iirds#Troubleshooting -->

    <owl:NamedIndividual rdf:about="http://iirds.tekom.de/iirds#Troubleshooting"/>
    


    <!-- http://iirds.tekom.de/iirds#Use -->

    <owl:NamedIndividual rdf:about="http://iirds.tekom.de/iirds#Use"/>
    


    <!-- http://iirds.tekom.de/iirds#Warning -->

    <owl:NamedIndividual rdf:about="http://iirds.tekom.de/iirds#Warning">
        <rdf:type rdf:resource="http://iirds.tekom.de/iirds#WarningMessage"/>
        <iirds:description xml:lang="en">See ANSI Z535.5</iirds:description>
        <rdfs:comment xml:lang="en">Describes a hazardous situation which, if not avoided, could result in death or serious injury.</rdfs:comment>
        <rdfs:label xml:lang="en">Warning</rdfs:label>
        <rdfs:label xml:lang="de">Warnung</rdfs:label>
    </owl:NamedIndividual>
    


    <!-- http://iirds.tekom.de/iirds#WarningMessage -->

    <owl:NamedIndividual rdf:about="http://iirds.tekom.de/iirds#WarningMessage"/>
    


    <!-- http://iirds.tekom.de/iirds#WarrantyConditions -->

    <owl:NamedIndividual rdf:about="http://iirds.tekom.de/iirds#WarrantyConditions">
        <rdf:type rdf:resource="http://iirds.tekom.de/iirds#Formality"/>
        <iirds:description xml:lang="en"></iirds:description>
        <rdfs:comment xml:lang="en">Information subject. Contains the warranty conditions.</rdfs:comment>
        <rdfs:label xml:lang="de"></rdfs:label>
        <rdfs:label xml:lang="en">Warranty conditions</rdfs:label>
    </owl:NamedIndividual>
    


    <!-- http://iirds.tekom.de/iirds#Withdrawn -->

    <owl:NamedIndividual rdf:about="http://iirds.tekom.de/iirds#Withdrawn">
        <rdf:type rdf:resource="http://iirds.tekom.de/iirds#ContentLifeCycleStatusValue"/>
        <iirds:description xml:lang="en"></iirds:description>
        <rdfs:comment xml:lang="en">Content lifecycle status value; indicates that the content has been withdrawn and is no longer valid.</rdfs:comment>
        <rdfs:label xml:lang="de">Widerrufen</rdfs:label>
        <rdfs:label xml:lang="en">Withdrawn</rdfs:label>
    </owl:NamedIndividual>
    


    <!-- http://iirds.tekom.de/iirds#WorkingTime -->

    <owl:NamedIndividual rdf:about="http://iirds.tekom.de/iirds#WorkingTime"/>
    


    <!-- http://iirds.tekom.de/iirds#dateOfCreation -->

    <owl:NamedIndividual rdf:about="http://iirds.tekom.de/iirds#dateOfCreation"/>
    


    <!-- http://iirds.tekom.de/iirds#dateOfEffect -->

    <owl:NamedIndividual rdf:about="http://iirds.tekom.de/iirds#dateOfEffect"/>
    


    <!-- http://iirds.tekom.de/iirds#dateOfExpiry -->

    <owl:NamedIndividual rdf:about="http://iirds.tekom.de/iirds#dateOfExpiry"/>
    


    <!-- http://iirds.tekom.de/iirds#dateOfLastModification -->

    <owl:NamedIndividual rdf:about="http://iirds.tekom.de/iirds#dateOfLastModification"/>
    


    <!-- http://iirds.tekom.de/iirds#dateOfStatus -->

    <owl:NamedIndividual rdf:about="http://iirds.tekom.de/iirds#dateOfStatus"/>
    


    <!-- http://iirds.tekom.de/iirds#description -->

    <owl:NamedIndividual rdf:about="http://iirds.tekom.de/iirds#description"/>
    


    <!-- http://iirds.tekom.de/iirds#duration -->

    <owl:NamedIndividual rdf:about="http://iirds.tekom.de/iirds#duration"/>
    


    <!-- http://iirds.tekom.de/iirds#format -->

    <owl:NamedIndividual rdf:about="http://iirds.tekom.de/iirds#format"/>
    


    <!-- http://iirds.tekom.de/iirds#formatRestriction -->

    <owl:NamedIndividual rdf:about="http://iirds.tekom.de/iirds#formatRestriction"/>
    


    <!-- http://iirds.tekom.de/iirds#frequency -->

    <owl:NamedIndividual rdf:about="http://iirds.tekom.de/iirds#frequency"/>
    


    <!-- http://iirds.tekom.de/iirds#has-abstract -->

    <owl:NamedIndividual rdf:about="http://iirds.tekom.de/iirds#has-abstract"/>
    


    <!-- http://iirds.tekom.de/iirds#has-component -->

    <owl:NamedIndividual rdf:about="http://iirds.tekom.de/iirds#has-component"/>
    


    <!-- http://iirds.tekom.de/iirds#has-content-lifecycle-status -->

    <owl:NamedIndividual rdf:about="http://iirds.tekom.de/iirds#has-content-lifecycle-status"/>
    


    <!-- http://iirds.tekom.de/iirds#has-content-lifecycle-status-value -->

    <owl:NamedIndividual rdf:about="http://iirds.tekom.de/iirds#has-content-lifecycle-status-value"/>
    


    <!-- http://iirds.tekom.de/iirds#has-directory-structure-type -->

    <owl:NamedIndividual rdf:about="http://iirds.tekom.de/iirds#has-directory-structure-type"/>
    


    <!-- http://iirds.tekom.de/iirds#has-document-type -->

    <owl:NamedIndividual rdf:about="http://iirds.tekom.de/iirds#has-document-type"/>
    


    <!-- http://iirds.tekom.de/iirds#has-end-selector -->

    <owl:NamedIndividual rdf:about="http://iirds.tekom.de/iirds#has-end-selector"/>
    


    <!-- http://iirds.tekom.de/iirds#has-event-code -->

    <owl:NamedIndividual rdf:about="http://iirds.tekom.de/iirds#has-event-code"/>
    


    <!-- http://iirds.tekom.de/iirds#has-event-type -->

    <owl:NamedIndividual rdf:about="http://iirds.tekom.de/iirds#has-event-type"/>
    


    <!-- http://iirds.tekom.de/iirds#has-first-child -->

    <owl:NamedIndividual rdf:about="http://iirds.tekom.de/iirds#has-first-child"/>
    


    <!-- http://iirds.tekom.de/iirds#has-identity -->

    <owl:NamedIndividual rdf:about="http://iirds.tekom.de/iirds#has-identity"/>
    


    <!-- http://iirds.tekom.de/iirds#has-identity-domain -->

    <owl:NamedIndividual rdf:about="http://iirds.tekom.de/iirds#has-identity-domain"/>
    


    <!-- http://iirds.tekom.de/iirds#has-information-type -->

    <owl:NamedIndividual rdf:about="http://iirds.tekom.de/iirds#has-information-type"/>
    


    <!-- http://iirds.tekom.de/iirds#has-next-sibling -->

    <owl:NamedIndividual rdf:about="http://iirds.tekom.de/iirds#has-next-sibling"/>
    


    <!-- http://iirds.tekom.de/iirds#has-party-role -->

    <owl:NamedIndividual rdf:about="http://iirds.tekom.de/iirds#has-party-role"/>
    


    <!-- http://iirds.tekom.de/iirds#has-planning-time -->

    <owl:NamedIndividual rdf:about="http://iirds.tekom.de/iirds#has-planning-time"/>
    


    <!-- http://iirds.tekom.de/iirds#has-rendition -->

    <owl:NamedIndividual rdf:about="http://iirds.tekom.de/iirds#has-rendition"/>
    


    <!-- http://iirds.tekom.de/iirds#has-selector -->

    <owl:NamedIndividual rdf:about="http://iirds.tekom.de/iirds#has-selector"/>
    


    <!-- http://iirds.tekom.de/iirds#has-start-selector -->

    <owl:NamedIndividual rdf:about="http://iirds.tekom.de/iirds#has-start-selector"/>
    


    <!-- http://iirds.tekom.de/iirds#has-subject -->

    <owl:NamedIndividual rdf:about="http://iirds.tekom.de/iirds#has-subject"/>
    


    <!-- http://iirds.tekom.de/iirds#has-topic-type -->

    <owl:NamedIndividual rdf:about="http://iirds.tekom.de/iirds#has-topic-type"/>
    


    <!-- http://iirds.tekom.de/iirds#identifier -->

    <owl:NamedIndividual rdf:about="http://iirds.tekom.de/iirds#identifier"/>
    


    <!-- http://iirds.tekom.de/iirds#iiRDSVersion -->

    <owl:NamedIndividual rdf:about="http://iirds.tekom.de/iirds#iiRDSVersion"/>
    


    <!-- http://iirds.tekom.de/iirds#iirdsAttribute -->

    <owl:NamedIndividual rdf:about="http://iirds.tekom.de/iirds#iirdsAttribute"/>
    


    <!-- http://iirds.tekom.de/iirds#iirdsDomainEntity -->

    <owl:NamedIndividual rdf:about="http://iirds.tekom.de/iirds#iirdsDomainEntity"/>
    


    <!-- http://iirds.tekom.de/iirds#iirdsRelationConcept -->

    <owl:NamedIndividual rdf:about="http://iirds.tekom.de/iirds#iirdsRelationConcept"/>
    


    <!-- http://iirds.tekom.de/iirds#is-applicable-for-document-type -->

    <owl:NamedIndividual rdf:about="http://iirds.tekom.de/iirds#is-applicable-for-document-type"/>
    


    <!-- http://iirds.tekom.de/iirds#is-part-of-package -->

    <owl:NamedIndividual rdf:about="http://iirds.tekom.de/iirds#is-part-of-package"/>
    


    <!-- http://iirds.tekom.de/iirds#is-replacement-of -->

    <owl:NamedIndividual rdf:about="http://iirds.tekom.de/iirds#is-replacement-of"/>
    


    <!-- http://iirds.tekom.de/iirds#is-version-of -->

    <owl:NamedIndividual rdf:about="http://iirds.tekom.de/iirds#is-version-of"/>
    


    <!-- http://iirds.tekom.de/iirds#language -->

    <owl:NamedIndividual rdf:about="http://iirds.tekom.de/iirds#language"/>
    


    <!-- http://iirds.tekom.de/iirds#nil -->

    <owl:NamedIndividual rdf:about="http://iirds.tekom.de/iirds#nil"/>
    


    <!-- http://iirds.tekom.de/iirds#purpose -->

    <owl:NamedIndividual rdf:about="http://iirds.tekom.de/iirds#purpose"/>
    


    <!-- http://iirds.tekom.de/iirds#relates-to-administrative-metadata -->

    <owl:NamedIndividual rdf:about="http://iirds.tekom.de/iirds#relates-to-administrative-metadata"/>
    


    <!-- http://iirds.tekom.de/iirds#relates-to-component -->

    <owl:NamedIndividual rdf:about="http://iirds.tekom.de/iirds#relates-to-component"/>
    


    <!-- http://iirds.tekom.de/iirds#relates-to-event -->

    <owl:NamedIndividual rdf:about="http://iirds.tekom.de/iirds#relates-to-event"/>
    


    <!-- http://iirds.tekom.de/iirds#relates-to-functional-metadata -->

    <owl:NamedIndividual rdf:about="http://iirds.tekom.de/iirds#relates-to-functional-metadata"/>
    


    <!-- http://iirds.tekom.de/iirds#relates-to-information-unit -->

    <owl:NamedIndividual rdf:about="http://iirds.tekom.de/iirds#relates-to-information-unit"/>
    


    <!-- http://iirds.tekom.de/iirds#relates-to-party -->

    <owl:NamedIndividual rdf:about="http://iirds.tekom.de/iirds#relates-to-party"/>
    


    <!-- http://iirds.tekom.de/iirds#relates-to-product-feature -->

    <owl:NamedIndividual rdf:about="http://iirds.tekom.de/iirds#relates-to-product-feature"/>
    


    <!-- http://iirds.tekom.de/iirds#relates-to-product-lifecycle-phase -->

    <owl:NamedIndividual rdf:about="http://iirds.tekom.de/iirds#relates-to-product-lifecycle-phase"/>
    


    <!-- http://iirds.tekom.de/iirds#relates-to-product-metadata -->

    <owl:NamedIndividual rdf:about="http://iirds.tekom.de/iirds#relates-to-product-metadata"/>
    


    <!-- http://iirds.tekom.de/iirds#relates-to-product-variant -->

    <owl:NamedIndividual rdf:about="http://iirds.tekom.de/iirds#relates-to-product-variant"/>
    


    <!-- http://iirds.tekom.de/iirds#relates-to-qualification -->

    <owl:NamedIndividual rdf:about="http://iirds.tekom.de/iirds#relates-to-qualification"/>
    


    <!-- http://iirds.tekom.de/iirds#relates-to-supply -->

    <owl:NamedIndividual rdf:about="http://iirds.tekom.de/iirds#relates-to-supply"/>
    


    <!-- http://iirds.tekom.de/iirds#relates-to-vcard -->

    <owl:NamedIndividual rdf:about="http://iirds.tekom.de/iirds#relates-to-vcard"/>
    


    <!-- http://iirds.tekom.de/iirds#revision -->

    <owl:NamedIndividual rdf:about="http://iirds.tekom.de/iirds#revision"/>
    


    <!-- http://iirds.tekom.de/iirds#rights -->

    <owl:NamedIndividual rdf:about="http://iirds.tekom.de/iirds#rights"/>
    


    <!-- http://iirds.tekom.de/iirds#source -->

    <owl:NamedIndividual rdf:about="http://iirds.tekom.de/iirds#source"/>
    


    <!-- http://iirds.tekom.de/iirds#statusComment -->

    <owl:NamedIndividual rdf:about="http://iirds.tekom.de/iirds#statusComment"/>
    


    <!-- http://iirds.tekom.de/iirds#synonym -->

    <owl:NamedIndividual rdf:about="http://iirds.tekom.de/iirds#synonym"/>
    


    <!-- http://iirds.tekom.de/iirds#title -->

    <owl:NamedIndividual rdf:about="http://iirds.tekom.de/iirds#title"/>
    


    <!-- 
    ///////////////////////////////////////////////////////////////////////////////////////
    //
    // Annotations
    //
    ///////////////////////////////////////////////////////////////////////////////////////
     -->

    <rdf:Description rdf:about="http://iirds.tekom.de/iirds#AdministrativeMetadata">
        <rdfs:label xml:lang="en">Administrative metadata</rdfs:label>
        <rdfs:label xml:lang="de">Verwaltungsmetadaten</rdfs:label>
        <iirds:description xml:lang="en">Not intended to be used directly. Use the subclasses instead.</iirds:description>
        <rdfs:comment xml:lang="en">Parent class for administrative metadata, such as status and identifier. </rdfs:comment>
    </rdf:Description>
    <rdf:Description rdf:about="http://iirds.tekom.de/iirds#AfterUse">
        <rdfs:label xml:lang="en">After use</rdfs:label>
        <iirds:description xml:lang="en">IRI: required</iirds:description>
        <rdfs:label xml:lang="de">Nutzungsende</rdfs:label>
        <rdfs:comment xml:lang="en">Parent class for iiRDS standard definitions of product lifecycle phases that occur after the active use of the product. </rdfs:comment>
        <iirds:description xml:lang="en">Not intended to be used directly. Use the subclasses instead. For lifecycle phases not covered by the iiRDS standard subclasses, define custom subclasses.</iirds:description>
    </rdf:Description>
    <rdf:Description rdf:about="http://iirds.tekom.de/iirds#Collection">
        <iirds:description xml:lang="en">IRI: required</iirds:description>
        <rdfs:label xml:lang="de">Zusammenstellung</rdfs:label>
        <rdfs:label xml:lang="en">Collection</rdfs:label>
        <iirds:description xml:lang="en">Not intented to be used directly. Use the subclasses instead. For collection subjects not covered by the iiRDS standard subclasses, define custom subclasses.</iirds:description>
        <rdfs:comment xml:lang="en">Parent class for information subjects representing collections of specific information, such as list of spare parts or maintenance plan.</rdfs:comment>
    </rdf:Description>
    <rdf:Description rdf:about="http://iirds.tekom.de/iirds#Component">
        <rdfs:comment xml:lang="en">Describes a component of the technical system that the documentation refers to.</rdfs:comment>
        <iirds:description xml:lang="en">Components may have relations to other components so that iiRDS Generators can build up a simple component hierarchy with iiRDS structures. 

The iirds#Component may also be used as a docking point for external component definitions.</iirds:description>
        <iirds:description xml:lang="en">IRI: required</iirds:description>
        <rdfs:label xml:lang="de">Komponente</rdfs:label>
        <rdfs:label xml:lang="en">Component</rdfs:label>
    </rdf:Description>
    <rdf:Description rdf:about="http://iirds.tekom.de/iirds#Concept">
        <iirds:description xml:lang="en">Conceptual information helps users to map their existing knowledge to tasks and other essential information about a product or system.
		</iirds:description>
        <rdfs:label xml:lang="en">Concept</rdfs:label>
        <rdfs:label xml:lang="de">Beschreibung</rdfs:label>
        <rdfs:comment xml:lang="en">Class of topic types that provide background that helps readers understand essential information about a product, interface, or task.</rdfs:comment>
        <iirds:description xml:lang="en">IRI: required</iirds:description>
    </rdf:Description>
    <rdf:Description rdf:about="http://iirds.tekom.de/iirds#Conformity">
        <iirds:description xml:lang="en">Not intended to be used directly. Use the subclasses instead. For information subjects not covered by the iiRDS standard subclasses, define custom subclasses.</iirds:description>
        <rdfs:comment xml:lang="en">Parent class for information subjects that describe content related to applicable standards or the conformity of the product.</rdfs:comment>
        <rdfs:label xml:lang="en">Conformity</rdfs:label>
        <rdfs:label xml:lang="de">Konformität</rdfs:label>
        <iirds:description xml:lang="en">IRI: required</iirds:description>
    </rdf:Description>
    <rdf:Description rdf:about="http://iirds.tekom.de/iirds#ContentLifeCycleStatus">
        <rdfs:comment xml:lang="en">Content lifecycle status of an information unit.</rdfs:comment>
        <rdfs:label xml:lang="en">Information unit lifecycle status</rdfs:label>
        <rdfs:label xml:lang="de">Lebenszyklus-Status einer Informationseinheit</rdfs:label>
        <iirds:description xml:lang="en">The status value is referenced using has-content-lifecycle-status-value. </iirds:description>
        <iirds:description xml:lang="en">IRI: optional</iirds:description>
    </rdf:Description>
    <rdf:Description rdf:about="http://iirds.tekom.de/iirds#ContentLifeCycleStatusValue">
        <iirds:description xml:lang="en">IRI: required</iirds:description>
        <rdfs:label xml:lang="de">Wert des Lebenszyklus-Status einer Informationseinheit</rdfs:label>
        <iirds:description xml:lang="en">The value refers to the content status, for example whether it is approved or withdrawn.</iirds:description>
        <rdfs:label xml:lang="en">Value of the information unit lifecycle status</rdfs:label>
        <rdfs:comment xml:lang="en">Value of an information unit&apos;s lifecycle status. The value is set by involved parties, such as the manufacturer or supplier.</rdfs:comment>
    </rdf:Description>
    <rdf:Description rdf:about="http://iirds.tekom.de/iirds#DesignAndRealization">
        <rdfs:label xml:lang="de">Produktentstehung</rdfs:label>
        <rdfs:comment xml:lang="en">Parent class for subclasses that describe product lifecycle phases related to the design, construction, and realization of a product.</rdfs:comment>
        <iirds:description xml:lang="en">IRI: required</iirds:description>
        <rdfs:label xml:lang="en">Design and realization</rdfs:label>
        <iirds:description xml:lang="en">Not intended to be used directly. Use the subclasses instead. For lifecycle phases not covered by the iiRDS standard subclasses, define custom subclasses.</iirds:description>
    </rdf:Description>
    <rdf:Description rdf:about="http://iirds.tekom.de/iirds#DirectoryNode">
        <iirds:description xml:lang="de">Ein Verzeichnis ist eine baumartig organisierte und geordnete Zusammenstellung von Informationseinheiten. Verzeichnisknoten sind die Einträge in dem Baum. Verzeichnisse dienen dem Benutzer als Navigationshilfe über die Informationseinheiten. Ein Inhaltsverzeichnis eines Dokuments ist ein typisches Beispiel eines Verzeichnisses.</iirds:description>
        <rdfs:label xml:lang="de">Verzeichnisknoten</rdfs:label>
        <iirds:description xml:lang="en">A directory is a tree-like, ordered collection of information units. Directory nodes are the entries in the directory. Directories help the user to navigate through the information units. A table of contents is a typical example of a directory. </iirds:description>
        <rdfs:comment xml:lang="en">A node in a directory</rdfs:comment>
        <rdfs:label xml:lang="en">Directory node</rdfs:label>
        <rdfs:comment xml:lang="de">Ein Eintrag in einem Verzeichnis</rdfs:comment>
        <iirds:description xml:lang="en">IRI: optional</iirds:description>
    </rdf:Description>
    <rdf:Description rdf:about="http://iirds.tekom.de/iirds#DirectoryNodeType">
        <rdfs:label xml:lang="de">Verzeichnistyp</rdfs:label>
        <iirds:description xml:lang="en">IRI: required</iirds:description>
        <iirds:description xml:lang="de">Ein Verzeichnis, das durch einen Wurzelknoten und seine untergeordneten Knoten aufgespannt wird, hat einen Typ wie &apos;Inhaltsverzeichnis&apos; oder &apos;Abbildungsverzeichnis&apos;.</iirds:description>
        <rdfs:comment xml:lang="de">Verzeichnistyp</rdfs:comment>
        <rdfs:comment xml:lang="en">Directory type</rdfs:comment>
        <iirds:description xml:lang="en">A directory represented by a directory root node and its sub nodes has a type such as &apos;table of contens&apos; or &apos;list of figures&apos;.</iirds:description>
        <rdfs:label xml:lang="en">Directory node type</rdfs:label>
    </rdf:Description>
    <rdf:Description rdf:about="http://iirds.tekom.de/iirds#Document">
        <rdfs:label xml:lang="de">Dokument</rdfs:label>
        <rdfs:label xml:lang="en">Document</rdfs:label>
        <iirds:description xml:lang="en">A document consists of one or more files. It can consist of topics. The resource is either a blank node (when there is no file representing the document) or a file in the iiRDS package.</iirds:description>
        <rdfs:comment xml:lang="en">A unit of information in an iiRDS package that represents a complete document.</rdfs:comment>
        <iirds:description xml:lang="en">IRI: required</iirds:description>
    </rdf:Description>
    <rdf:Description rdf:about="http://iirds.tekom.de/iirds#DocumentType">
        <rdfs:label xml:lang="de">Dokumentart</rdfs:label>
        <rdfs:comment xml:lang="en">The type of a document.</rdfs:comment>
        <rdfs:label xml:lang="en">Document type</rdfs:label>
        <iirds:description xml:lang="en">Document types define the intended purpose of a document.</iirds:description>
        <iirds:description xml:lang="en">IRI: required</iirds:description>
    </rdf:Description>
    <rdf:Description rdf:about="http://iirds.tekom.de/iirds#DocumentationMetadata">
        <rdfs:label xml:lang="de">Metadaten der Dokumentation</rdfs:label>
        <rdfs:comment xml:lang="en">Parent class for functional metadata and product metadata.</rdfs:comment>
        <iirds:description xml:lang="en">Not intended to be used directly. Use the subclasses instead.</iirds:description>
        <rdfs:label xml:lang="en">Documentation metadata</rdfs:label>
    </rdf:Description>
    <rdf:Description rdf:about="http://iirds.tekom.de/iirds#DownTime">
        <rdfs:label xml:lang="de">Stillstandzeit</rdfs:label>
        <iirds:description xml:lang="en"></iirds:description>
        <rdfs:label xml:lang="en">Down time</rdfs:label>
        <iirds:description xml:lang="en">IRI: optional</iirds:description>
        <rdfs:comment xml:lang="en">Type of planning time: Period of time during which a technical system is stopped, especially during setup for an operation or when making repairs.</rdfs:comment>
    </rdf:Description>
    <rdf:Description rdf:about="http://iirds.tekom.de/iirds#Event">
        <iirds:description xml:lang="en">Examples are errors, malfunctions, and warnings. 
Use the relates-to-event property to create a reference from an information unit to an event.</iirds:description>
        <iirds:description xml:lang="en">IRI: required</iirds:description>
        <rdfs:label xml:lang="en">Event</rdfs:label>
        <rdfs:label xml:lang="de">Ereignis</rdfs:label>
        <rdfs:comment xml:lang="en">Describes events that happen in the technical system</rdfs:comment>
    </rdf:Description>
    <rdf:Description rdf:about="http://iirds.tekom.de/iirds#Form">
        <iirds:description xml:lang="en">IRI: required</iirds:description>
        <iirds:description xml:lang="en">Examples of forms are service reports, field reports, and user feedback.</iirds:description>
        <rdfs:comment xml:lang="en">Class of topic types that contain information in pre-defined form fields.</rdfs:comment>
        <rdfs:label xml:lang="en">Form</rdfs:label>
        <rdfs:label xml:lang="de">Formular</rdfs:label>
    </rdf:Description>
    <rdf:Description rdf:about="http://iirds.tekom.de/iirds#Formality">
        <rdfs:comment xml:lang="en">Parent class for information subjects that describe content related to official or legal documents.</rdfs:comment>
        <rdfs:label xml:lang="en">Formality</rdfs:label>
        <iirds:description xml:lang="en">Examples of formality subjects are license terms and warranty conditions.</iirds:description>
        <iirds:description xml:lang="en">IRI: required</iirds:description>
        <rdfs:label xml:lang="de">Formalität</rdfs:label>
    </rdf:Description>
    <rdf:Description rdf:about="http://iirds.tekom.de/iirds#Fragment">
        <rdfs:label xml:lang="de">Fragment</rdfs:label>
        <iirds:description xml:lang="en">Sections, tables, lists, paragraphs, and hazard statements are examples of fragments. Fragments assign metadata to parts of topic or document files in an iiRDS package. The parts are identified by a fragment selector.</iirds:description>
        <iirds:description xml:lang="en">IRI: required</iirds:description>
        <rdfs:comment xml:lang="en">A piece of information within a document or topic.</rdfs:comment>
        <rdfs:label xml:lang="en">Fragment</rdfs:label>
    </rdf:Description>
    <rdf:Description rdf:about="http://iirds.tekom.de/iirds#FragmentSelector">
        <rdfs:comment xml:lang="de">Verweist auf Fragment in einer physikalischen Ressource.</rdfs:comment>
        <rdfs:label xml:lang="en">Fragment selector</rdfs:label>
        <rdfs:label xml:lang="de">Fragmentselektor</rdfs:label>
        <iirds:description xml:lang="en">IRI: optional</iirds:description>
        <rdfs:comment xml:lang="en">Points to a fragment in a physical resource.</rdfs:comment>
    </rdf:Description>
    <rdf:Description rdf:about="http://iirds.tekom.de/iirds#FunctionalMetadata">
        <rdfs:label xml:lang="en">Functional metadata</rdfs:label>
        <rdfs:label xml:lang="de">Funktionale Metadaten</rdfs:label>
        <iirds:description xml:lang="en">Not intended to be used directly. Use the subclasses instead.</iirds:description>
        <rdfs:comment xml:lang="en">Parent class for metadata supporting advanced content delivery scenarios and content assemblies for specific purposes.</rdfs:comment>
    </rdf:Description>
    <rdf:Description rdf:about="http://iirds.tekom.de/iirds#Functionality">
        <iirds:description xml:lang="en"></iirds:description>
        <rdfs:comment xml:lang="en">Parent class for information subjects that describe content related to specific functionalities of the product.</rdfs:comment>
        <rdfs:label xml:lang="de">Funktionalität</rdfs:label>
        <rdfs:label xml:lang="en">Functionality</rdfs:label>
        <iirds:description xml:lang="en">IRI: required</iirds:description>
    </rdf:Description>
    <rdf:Description rdf:about="http://iirds.tekom.de/iirds#Identity">
        <iirds:description xml:lang="en">IRI: optional</iirds:description>
        <rdfs:label xml:lang="de">Identität</rdfs:label>
        <iirds:description xml:lang="en">Complex identifiers may be assigned to information objects, information units, product variants, and components. Typically, identities are used to provide IDs from other systems. Examples: serial numbers for components and module IDs from content management systems for topics.</iirds:description>
        <rdfs:comment xml:lang="en">Complex identifier of an iiRDS domain entity. Each identifier must be related to the identity domain within which it is unambiguous.</rdfs:comment>
        <rdfs:label xml:lang="en">Identity</rdfs:label>
    </rdf:Description>
    <rdf:Description rdf:about="http://iirds.tekom.de/iirds#IdentityDomain">
        <rdfs:comment xml:lang="en">Domain of an identifier that is assigned to an iiRDS domain entity.</rdfs:comment>
        <rdfs:label xml:lang="en">Identity domain</rdfs:label>
        <iirds:description xml:lang="en">An identity domain relates to a party, meaning a company or organization. The party is the owner or custodian of the domain.</iirds:description>
        <rdfs:label xml:lang="de">Identitäts-Domäne</rdfs:label>
        <iirds:description xml:lang="en">IRI: required</iirds:description>
    </rdf:Description>
    <rdf:Description rdf:about="http://iirds.tekom.de/iirds#InformationObject">
        <iirds:description xml:lang="en">Only used if a version/language-independent equivalent to an information unit is required. The versioned information unit references the information object.</iirds:description>
        <iirds:description xml:lang="en">IRI: required</iirds:description>
        <rdfs:label xml:lang="en">Information object</rdfs:label>
        <rdfs:label xml:lang="de">Informationsobjekt</rdfs:label>
        <rdfs:comment xml:lang="en">A version-independent and language-independent equivalent to an information unit.</rdfs:comment>
    </rdf:Description>
    <rdf:Description rdf:about="http://iirds.tekom.de/iirds#InformationSubject">
        <rdfs:comment xml:lang="en">Type of information. Abstract base class of subjects that an information unit covers.</rdfs:comment>
        <iirds:description xml:lang="en">IRI: required</iirds:description>
        <rdfs:label xml:lang="de">Informationsthema</rdfs:label>
        <rdfs:label xml:lang="en">Information subject</rdfs:label>
        <iirds:description xml:lang="en">Not intented to be used directly. Use the subclasses instead.</iirds:description>
    </rdf:Description>
    <rdf:Description rdf:about="http://iirds.tekom.de/iirds#InformationType">
        <rdfs:label xml:lang="en">Information type</rdfs:label>
        <rdfs:comment xml:lang="en">Type of information. Abstract base class of document and topic type.</rdfs:comment>
        <iirds:description xml:lang="en">Not intented to be used directly.</iirds:description>
        <iirds:description xml:lang="en">IRI: required</iirds:description>
        <rdfs:label xml:lang="de">Informationsart</rdfs:label>
    </rdf:Description>
    <rdf:Description rdf:about="http://iirds.tekom.de/iirds#InformationUnit">
        <iirds:description xml:lang="en">IRI: required</iirds:description>
        <rdfs:label xml:lang="de">Informationseinheit</rdfs:label>
        <iirds:description xml:lang="en">Not intended to be used directly. Use the subclasses Package, Document, Topic, and Fragment instead.</iirds:description>
        <rdfs:comment xml:lang="en">A unit of information. Abstract base class for specific information units.</rdfs:comment>
        <rdfs:label xml:lang="en">Information unit</rdfs:label>
    </rdf:Description>
    <rdf:Description rdf:about="http://iirds.tekom.de/iirds#Learning">
        <rdfs:comment xml:lang="en">Class of topic types for learning. Learning content may comprise learning plans, learning objectives, learning content details, summaries, and assessments.</rdfs:comment>
        <iirds:description xml:lang="en">IRI: required</iirds:description>
        <rdfs:label xml:lang="en">Learning</rdfs:label>
        <iirds:description xml:lang="de">Learning content may comprise learning plans, learning objectives, learning content details, summaries, and assessments.</iirds:description>
        <rdfs:label xml:lang="de">Lernen</rdfs:label>
    </rdf:Description>
    <rdf:Description rdf:about="http://iirds.tekom.de/iirds#MaintenanceInterval">
        <rdfs:comment xml:lang="en">Type of planning time: Fixed time interval for the scheduled maintenance of a technical system or its parts.</rdfs:comment>
        <iirds:description xml:lang="en">Instances have a maintenance frequency and an optional maintenance duration.</iirds:description>
        <rdfs:label xml:lang="en">Maintenance interval</rdfs:label>
        <iirds:description xml:lang="en">IRI: optional</iirds:description>
        <rdfs:label xml:lang="de">Wartungsintervall</rdfs:label>
    </rdf:Description>
    <rdf:Description rdf:about="http://iirds.tekom.de/iirds#Package">
        <rdfs:label xml:lang="de">Paket</rdfs:label>
        <iirds:description xml:lang="en">IRI: required</iirds:description>
        <rdfs:comment xml:lang="en">A set of information in terms of documents and topics with their metadata.</rdfs:comment>
        <rdfs:label xml:lang="en">Package</rdfs:label>
        <iirds:description xml:lang="en">There is exactly one Package instance within an iiRDS package. It holds general metadata on the overall iiRDS package.</iirds:description>
    </rdf:Description>
    <rdf:Description rdf:about="http://iirds.tekom.de/iirds#Party">
        <iirds:description xml:lang="en">Detailed information about a party may be specified in a vCard.</iirds:description>
        <rdfs:label xml:lang="en">Party</rdfs:label>
        <rdfs:label xml:lang="de">Akteur</rdfs:label>
        <iirds:description xml:lang="en">IRI: required</iirds:description>
        <rdfs:comment xml:lang="en">Party related to an iiRDS domain entity. </rdfs:comment>
    </rdf:Description>
    <rdf:Description rdf:about="http://iirds.tekom.de/iirds#PartyRole">
        <rdfs:comment xml:lang="en">Role of a party related to an iiRDS domain entity.</rdfs:comment>
        <rdfs:label xml:lang="de">Akteursrolle</rdfs:label>
        <iirds:description xml:lang="en">Examples of party roles: manufacturer, author, inspector.</iirds:description>
        <iirds:description xml:lang="en">IRI: required</iirds:description>
        <rdfs:label xml:lang="en">Party role</rdfs:label>
    </rdf:Description>
    <rdf:Description rdf:about="http://iirds.tekom.de/iirds#PlanningTime">
        <iirds:description xml:lang="en">IRI: optional</iirds:description>
        <iirds:description xml:lang="en">Not intended to be used directly.  Use the subclasses instead.</iirds:description>
        <rdfs:label xml:lang="de">Planungszeit</rdfs:label>
        <rdfs:comment xml:lang="en">Parent class for different types of planning time that may be referenced in technical documentation. Planning times describe periods of time required for or resulting from specific working tasks.</rdfs:comment>
        <rdfs:label xml:lang="en">Planning time</rdfs:label>
    </rdf:Description>
    <rdf:Description rdf:about="http://iirds.tekom.de/iirds#Process">
        <iirds:description xml:lang="en">IRI: required</iirds:description>
        <iirds:description xml:lang="en"></iirds:description>
        <rdfs:label xml:lang="de">Prozess</rdfs:label>
        <rdfs:comment xml:lang="en">Information subject for process-related information</rdfs:comment>
        <rdfs:label xml:lang="en">Process</rdfs:label>
    </rdf:Description>
    <rdf:Description rdf:about="http://iirds.tekom.de/iirds#ProductFeature">
        <iirds:description xml:lang="en">Not intended to be used directly. Use the subclasses instead.</iirds:description>
        <rdfs:comment xml:lang="en">Parent class for characteristics and functions of a product or component.</rdfs:comment>
        <rdfs:label xml:lang="en">Product feature</rdfs:label>
        <rdfs:label xml:lang="de">Produktmerkmal</rdfs:label>
        <iirds:description xml:lang="en">IRI: required</iirds:description>
    </rdf:Description>
    <rdf:Description rdf:about="http://iirds.tekom.de/iirds#ProductFunction">
        <rdfs:label xml:lang="en">Product function</rdfs:label>
        <iirds:description xml:lang="en">Examples: starting a phone call, ending a phone call, ringing.</iirds:description>
        <iirds:description xml:lang="en">IRI: required</iirds:description>
        <rdfs:label xml:lang="de">Produktfunktion</rdfs:label>
        <rdfs:comment xml:lang="en">A function that a product or component provides or implements.</rdfs:comment>
    </rdf:Description>
    <rdf:Description rdf:about="http://iirds.tekom.de/iirds#ProductLifeCyclePhase">
        <iirds:description xml:lang="en">Not intended to be used directly. Use the subclasses instead. </iirds:description>
        <rdfs:label xml:lang="en">Phase of product lifecycle</rdfs:label>
        <rdfs:comment xml:lang="en">Parent class for standardized product lifecycle phases that technical documentation may refer to.</rdfs:comment>
        <iirds:description xml:lang="en">IRI: required</iirds:description>
        <rdfs:label xml:lang="de">Produktlebenszyklusphase</rdfs:label>
    </rdf:Description>
    <rdf:Description rdf:about="http://iirds.tekom.de/iirds#ProductMetadata">
        <iirds:description xml:lang="en">Not intended to be used directly. Use the subclasses instead.</iirds:description>
        <rdfs:label xml:lang="de">Produktmetadaten</rdfs:label>
        <rdfs:comment xml:lang="en">Parent class for product-related metadata.</rdfs:comment>
        <iirds:description xml:lang="en">IRI: required</iirds:description>
        <rdfs:label xml:lang="en">ProductMetadata</rdfs:label>
    </rdf:Description>
    <rdf:Description rdf:about="http://iirds.tekom.de/iirds#ProductProperty">
        <rdfs:label xml:lang="en">Product property</rdfs:label>
        <iirds:description xml:lang="en">Examples: dimensions, voltage, power, weight.</iirds:description>
        <rdfs:comment xml:lang="en">A characteristic of a product or component.</rdfs:comment>
        <iirds:description xml:lang="en">IRI: required</iirds:description>
        <rdfs:label xml:lang="de">Produkteigenschaft</rdfs:label>
    </rdf:Description>
    <rdf:Description rdf:about="http://iirds.tekom.de/iirds#ProductVariant">
        <rdfs:label xml:lang="en">Product variant</rdfs:label>
        <iirds:description xml:lang="en">Examples: a specific model in a series or an individually manufactured good.</iirds:description>
        <iirds:description xml:lang="en">IRI: required</iirds:description>
        <rdfs:label xml:lang="de">Produktvariante</rdfs:label>
        <rdfs:comment xml:lang="en">A variation of a product with some specific characteristics or features. </rdfs:comment>
    </rdf:Description>
    <rdf:Description rdf:about="http://iirds.tekom.de/iirds#PuttingToUse">
        <rdfs:label xml:lang="de">In Nutzung nehmen</rdfs:label>
        <iirds:description xml:lang="en">IRI: required</iirds:description>
        <rdfs:comment xml:lang="en">Parent class for subclasses that describe product lifecycle phases related to putting a product or technical system to use.</rdfs:comment>
        <iirds:description xml:lang="en">Not intended to be used directly. Use the subclasses instead. For lifecycle phases not covered by the iiRDS standard subclasses, define custom subclasses.</iirds:description>
        <rdfs:label xml:lang="en">Putting to use</rdfs:label>
    </rdf:Description>
    <rdf:Description rdf:about="http://iirds.tekom.de/iirds#Qualification">
        <rdfs:label xml:lang="en">Qualification</rdfs:label>
        <rdfs:label xml:lang="de">Qualifikation</rdfs:label>
        <iirds:description xml:lang="en">Not intended to be used directly. Use the subclasses instead. </iirds:description>
        <rdfs:comment xml:lang="en">Parent class for different types of skills and roles required for working tasks described in technical documentation. </rdfs:comment>
        <iirds:description xml:lang="en">IRI: required</iirds:description>
    </rdf:Description>
    <rdf:Description rdf:about="http://iirds.tekom.de/iirds#RangeSelector">
        <rdfs:label xml:lang="de">Bereichsselektor</rdfs:label>
        <iirds:description xml:lang="en"></iirds:description>
        <iirds:description xml:lang="en">IRI: optional</iirds:description>
        <rdfs:comment xml:lang="en">Points to a range in a physical resource. Has a start and end point.</rdfs:comment>
        <rdfs:comment xml:lang="de">Verweist auf einen Bereich in einer physikalischen Ressource. Hat einen Start- und einen Endpunkt.</rdfs:comment>
        <rdfs:label xml:lang="en">Range selector</rdfs:label>
    </rdf:Description>
    <rdf:Description rdf:about="http://iirds.tekom.de/iirds#Reference">
        <iirds:description xml:lang="en">IRI: required</iirds:description>
        <iirds:description xml:lang="de">Examples are parameter lists, tables with technical data, UI control overviews, and parts lists. 
		</iirds:description>
        <rdfs:label xml:lang="en">Reference</rdfs:label>
        <rdfs:comment xml:lang="de">Class of topic types that contain information that supports users as they perform a task, meaning data that is looked up rather than memorized.</rdfs:comment>
        <rdfs:label xml:lang="de">Referenz</rdfs:label>
    </rdf:Description>
    <rdf:Description rdf:about="http://iirds.tekom.de/iirds#Rendition">
        <rdfs:label xml:lang="de">Inhaltsausprägung</rdfs:label>
        <iirds:description xml:lang="en"></iirds:description>
        <rdfs:comment xml:lang="de">Inhalt einer Informationseinheit in einem bestimmten Format</rdfs:comment>
        <iirds:description xml:lang="en">IRI: optional</iirds:description>
        <rdfs:comment xml:lang="en">Content of an information unit in a specific format</rdfs:comment>
        <rdfs:label xml:lang="en">Rendition</rdfs:label>
    </rdf:Description>
    <rdf:Description rdf:about="http://iirds.tekom.de/iirds#Role">
        <rdfs:comment xml:lang="de">Andockpunkt für unternehmensspezifische Rollen für Anwender des technischen Systems und der dazugehörigen Informationen.</rdfs:comment>
        <rdfs:label xml:lang="en">Role</rdfs:label>
        <rdfs:label xml:lang="de">Rolle</rdfs:label>
        <iirds:description xml:lang="de">Menge von zusammenhängenden Verhaltensweisen, Berechtigungen und Verpflichtungen, die Nutzern (Menschen, Softwareprozesse oder Geräte) eines Systems zugeordnet sind.</iirds:description>
        <iirds:description xml:lang="en">IRI: required</iirds:description>
        <iirds:description xml:lang="en">Describes a set of connected behaviors, privileges and obligations associated with users (humans, software processes or devices) of a system.</iirds:description>
        <rdfs:comment xml:lang="en">Docking point for custom roles for users of the technical system and the associated technical information.</rdfs:comment>
    </rdf:Description>
    <rdf:Description rdf:about="http://iirds.tekom.de/iirds#Safety">
        <rdfs:comment xml:lang="en">Information subject. Abstract base class for safety subjects.</rdfs:comment>
        <iirds:description xml:lang="en">Not intended to be used directly. Use the subclasses instead.</iirds:description>
        <rdfs:label xml:lang="de">Sicherheit</rdfs:label>
        <iirds:description xml:lang="en">IRI: required</iirds:description>
        <rdfs:label xml:lang="en">Safety</rdfs:label>
    </rdf:Description>
    <rdf:Description rdf:about="http://iirds.tekom.de/iirds#Selector">
        <iirds:description xml:lang="en">IRI: optional</iirds:description>
        <iirds:description xml:lang="en"></iirds:description>
        <rdfs:label xml:lang="de">Selektor</rdfs:label>
        <rdfs:label xml:lang="en">Selector</rdfs:label>
        <rdfs:comment xml:lang="de">Verweis auf eine physikalische Ressource.</rdfs:comment>
        <rdfs:comment xml:lang="en">Pointer to a physical resource.</rdfs:comment>
        <iirds:description xml:lang="de"></iirds:description>
    </rdf:Description>
    <rdf:Description rdf:about="http://iirds.tekom.de/iirds#SkillLevel">
        <rdfs:label xml:lang="de">Kenntnisstufe</rdfs:label>
        <iirds:description xml:lang="en">IRI: required</iirds:description>
        <iirds:description xml:lang="en">Describe the levels of ability required to carry out a specific task described in the technical documentation.</iirds:description>
        <rdfs:comment xml:lang="en">Docking point for custom skill levels that the users of the technical system and the associated technical information require.</rdfs:comment>
        <rdfs:label xml:lang="en">Skill level</rdfs:label>
    </rdf:Description>
    <rdf:Description rdf:about="http://iirds.tekom.de/iirds#Supply">
        <iirds:description xml:lang="en">IRI: required</iirds:description>
        <rdfs:comment xml:lang="en">Parent class for different types of supplies required for working tasks described in technical documentation.
</rdfs:comment>
        <rdfs:label xml:lang="en">Supply</rdfs:label>
        <iirds:description xml:lang="en">Not intended to be used directly. Use the subclasses instead. </iirds:description>
        <rdfs:label xml:lang="de">Hilfsmittel</rdfs:label>
    </rdf:Description>
    <rdf:Description rdf:about="http://iirds.tekom.de/iirds#Task">
        <rdfs:label xml:lang="en">Task</rdfs:label>
        <rdfs:comment xml:lang="en">Class of topic types that contains procedural information for work activities.</rdfs:comment>
        <iirds:description xml:lang="en">Tasks provide instructions and may contain information on other aspects, such as requirements that must be fulfilled or safety instructions.
		</iirds:description>
        <iirds:description xml:lang="en">IRI: required</iirds:description>
        <rdfs:label xml:lang="de">Aufgabe</rdfs:label>
    </rdf:Description>
    <rdf:Description rdf:about="http://iirds.tekom.de/iirds#TechnicalData">
        <rdfs:comment xml:lang="en">Information subject class. Information that describes the technical characteristics of a product or component in sufficient detail for assembly, integration, operation, and maintenance.</rdfs:comment>
        <iirds:description xml:lang="en">IRI: required</iirds:description>
        <rdfs:label xml:lang="en">Technical data</rdfs:label>
        <rdfs:label xml:lang="de">Technische Daten</rdfs:label>
        <iirds:description xml:lang="en">Not intended to be used directly. Use instances of this class instead.</iirds:description>
    </rdf:Description>
    <rdf:Description rdf:about="http://iirds.tekom.de/iirds#TechnicalOverview">
        <iirds:description xml:lang="en">Examples are circuit diagrams, flow diagrams, software interface overviews, and pneumatic diagrams.</iirds:description>
        <iirds:description xml:lang="en">IRI: required</iirds:description>
        <rdfs:comment xml:lang="en">Parent class for information subjects describing content related to technical plans, diagrams, or the technical architecture of the product.</rdfs:comment>
        <rdfs:label xml:lang="en">Technical overview</rdfs:label>
        <rdfs:label xml:lang="de">Technische Übersicht</rdfs:label>
    </rdf:Description>
    <rdf:Description rdf:about="http://iirds.tekom.de/iirds#Topic">
        <rdfs:label xml:lang="de">Topic</rdfs:label>
        <iirds:description xml:lang="en">The resource of a topic is a file in the iiRDS package.</iirds:description>
        <iirds:description xml:lang="en">IRI: required</iirds:description>
        <rdfs:comment xml:lang="en">A topic is a unit of information covering a single subject.</rdfs:comment>
        <rdfs:label xml:lang="en">Topic</rdfs:label>
    </rdf:Description>
    <rdf:Description rdf:about="http://iirds.tekom.de/iirds#TopicType">
        <rdfs:comment xml:lang="en">Defines the information type of an iiRDS topic.</rdfs:comment>
        <iirds:description xml:lang="en">IRI: required</iirds:description>
        <rdfs:label xml:lang="en">Topic type</rdfs:label>
        <iirds:description xml:lang="en">Possible types include task, learning, and concept. Information units that represent topics may have one or more has-topic-type properties that define the topic&apos;s information type. Topics without a has-topic-type property are generic topics, with no specific type.</iirds:description>
        <rdfs:label xml:lang="de">Topictyp</rdfs:label>
    </rdf:Description>
    <rdf:Description rdf:about="http://iirds.tekom.de/iirds#Troubleshooting">
        <rdfs:comment xml:lang="en">Class of topic types. Troubleshooting topics contain corrective action information that helps to fix an error or remove a malfunction.</rdfs:comment>
        <rdfs:label xml:lang="de">Störungsbeseitigung</rdfs:label>
        <rdfs:label xml:lang="en">Troubleshooting </rdfs:label>
        <iirds:description xml:lang="en">Typical troubleshooting topics contain sections with a description of the system&apos;s behavior or symptom, the cause for the error, and a remedy for the error.</iirds:description>
        <iirds:description xml:lang="en">IRI: required</iirds:description>
    </rdf:Description>
    <rdf:Description rdf:about="http://iirds.tekom.de/iirds#Use">
        <rdfs:label xml:lang="en">Use</rdfs:label>
        <rdfs:comment xml:lang="de">Produktlebenszyklusphase: Oberklasse für den Gebrauch eines Produkts.</rdfs:comment>
        <iirds:description xml:lang="en">IRI: required</iirds:description>
        <rdfs:comment xml:lang="en">Parent class for subclasses that describe product lifecycle phases related to using a product or technical system.</rdfs:comment>
        <rdfs:label xml:lang="de">Nutzung</rdfs:label>
        <iirds:description xml:lang="en">Not intended to be used directly. Use the subclasses instead. For lifecycle phases not covered by the iiRDS standard subclasses, define custom subclasses.</iirds:description>
    </rdf:Description>
    <rdf:Description rdf:about="http://iirds.tekom.de/iirds#WarningMessage">
        <iirds:description xml:lang="en">Warning messages usually consist of a hazard alert symbol, a signal word (such as &quot;Danger&quot;, &quot;Warning&quot;, &quot;Caution&quot;, &quot;Notice&quot;),  
a description of the potential hazard, and hints how to avoid the hazard.</iirds:description>
        <rdfs:label xml:lang="en">Warning message</rdfs:label>
        <iirds:description xml:lang="en">IRI: required</iirds:description>
        <rdfs:label xml:lang="de">Warnhinweis</rdfs:label>
        <rdfs:comment xml:lang="en">Information subject. Description of situations where a potential hazard can occur.</rdfs:comment>
    </rdf:Description>
    <rdf:Description rdf:about="http://iirds.tekom.de/iirds#WorkingTime">
        <iirds:description xml:lang="en">IRI: optional</iirds:description>
        <iirds:description xml:lang="en"></iirds:description>
        <rdfs:label xml:lang="de">Arbeitszeit</rdfs:label>
        <rdfs:comment xml:lang="en">Type of planning time: Period of time that is required for a specific working task.</rdfs:comment>
        <rdfs:label xml:lang="en">Working time</rdfs:label>
    </rdf:Description>
    <rdf:Description rdf:about="http://iirds.tekom.de/iirds#dateOfCreation">
        <schema:domainIncludes rdf:resource="http://iirds.tekom.de/iirds#InformationUnit"/>
        <schema:rangeIncludes rdf:resource="http://www.w3.org/2001/XMLSchema#dateTimeStamp"/>
        <rdfs:comment xml:lang="en">Date of creation of the information unit</rdfs:comment>
        <iirds:description xml:lang="en">Cardinality: http://iirds.tekom.de/iirds#InformationUnit [0..1]</iirds:description>
        <iirds:description xml:lang="en"></iirds:description>
        <rdfs:label xml:lang="de">Erstellungsdatum</rdfs:label>
        <rdfs:label xml:lang="en">Date of Creation</rdfs:label>
    </rdf:Description>
    <rdf:Description rdf:about="http://iirds.tekom.de/iirds#dateOfEffect">
        <rdfs:label xml:lang="en">Effective date</rdfs:label>
        <iirds:description xml:lang="en">Cardinality: http://iirds.tekom.de/iirds#ContentLifeCycleStatus [0..1]</iirds:description>
        <schema:domainIncludes rdf:resource="http://iirds.tekom.de/iirds#ContentLifeCycleStatus"/>
        <rdfs:comment xml:lang="en">Date and time on which the given content lifecycle status becomes valid.</rdfs:comment>
        <rdfs:label xml:lang="de">Gültigkeitsbeginn</rdfs:label>
        <rdfs:comment xml:lang="de">Datum und Uhrzeit, an dem der vergebene Status gültig wird.</rdfs:comment>
        <schema:rangeIncludes rdf:resource="http://www.w3.org/2001/XMLSchema#dateTimeStamp"/>
        <iirds:description xml:lang="en"></iirds:description>
    </rdf:Description>
    <rdf:Description rdf:about="http://iirds.tekom.de/iirds#dateOfExpiry">
        <schema:rangeIncludes rdf:resource="http://www.w3.org/2001/XMLSchema#dateTimeStamp"/>
        <iirds:description xml:lang="en">Cardinality: http://iirds.tekom.de/iirds#ContentLifeCycleStatus [0..1]</iirds:description>
        <rdfs:label xml:lang="de">Auslaufdatum</rdfs:label>
        <rdfs:comment xml:lang="en">Date and time on which the given content lifecycle status becomes invalid.</rdfs:comment>
        <schema:domainIncludes rdf:resource="http://iirds.tekom.de/iirds#ContentLifeCycleStatus"/>
        <iirds:description xml:lang="en"></iirds:description>
        <rdfs:comment xml:lang="de">Datum und Uhrzeit, an dem der vergebene Status ungültig wird.</rdfs:comment>
        <rdfs:label xml:lang="en">Expiry date</rdfs:label>
    </rdf:Description>
    <rdf:Description rdf:about="http://iirds.tekom.de/iirds#dateOfLastModification">
        <rdfs:comment xml:lang="en">Specifies the date and time on which the information unit was last changed.</rdfs:comment>
        <schema:rangeIncludes rdf:resource="http://www.w3.org/2001/XMLSchema#dateTimeStamp"/>
        <rdfs:label xml:lang="en">Date of last modification</rdfs:label>
        <schema:domainIncludes rdf:resource="http://iirds.tekom.de/iirds#InformationUnit"/>
        <iirds:description xml:lang="en"></iirds:description>
        <iirds:description xml:lang="en">Cardinality: http://iirds.tekom.de/iirds#InformationUnit [0..1]</iirds:description>
        <rdfs:label xml:lang="de">Letztes Änderungsdatum</rdfs:label>
    </rdf:Description>
    <rdf:Description rdf:about="http://iirds.tekom.de/iirds#dateOfStatus">
        <rdfs:label xml:lang="en">Status date</rdfs:label>
        <iirds:description xml:lang="en">Cardinality: http://iirds.tekom.de/iirds#ContentLifeCycleStatus [0..1]</iirds:description>
        <schema:domainIncludes rdf:resource="http://iirds.tekom.de/iirds#ContentLifeCycleStatus"/>
        <iirds:description xml:lang="en"></iirds:description>
        <rdfs:comment xml:lang="en">Specifies the date and time on which content lifecycle status was changed.</rdfs:comment>
        <rdfs:label xml:lang="de">Vergabedatum</rdfs:label>
        <schema:rangeIncludes rdf:resource="http://www.w3.org/2001/XMLSchema#dateTimeStamp"/>
    </rdf:Description>
    <rdf:Description rdf:about="http://iirds.tekom.de/iirds#description">
        <schema:domainIncludes rdf:resource="http://iirds.tekom.de/iirds#iirdsDomainEntity"/>
        <rdfs:label xml:lang="de">Beschreibung</rdfs:label>
        <iirds:description xml:lang="en">Cardinality: http://iirds.tekom.de/iirds#iirdsDomainEntity [0..*]</iirds:description>
        <rdfs:label xml:lang="en">Description</rdfs:label>
        <rdfs:comment xml:lang="en">An account of the resource.</rdfs:comment>
        <schema:rangeIncludes rdf:resource="http://www.w3.org/2000/01/rdf-schema#Literal"/>
        <iirds:description xml:lang="en">Typically a free-text acount of the resource</iirds:description>
    </rdf:Description>
    <rdf:Description rdf:about="http://iirds.tekom.de/iirds#duration">
        <rdfs:label xml:lang="en">Duration</rdfs:label>
        <iirds:description xml:lang="en"></iirds:description>
        <iirds:description xml:lang="en">Cardinality: http://iirds.tekom.de/iirds#PlanningTime [1]</iirds:description>
        <rdfs:label xml:lang="de">Dauer</rdfs:label>
        <schema:rangeIncludes rdf:resource="http://www.w3.org/2001/XMLSchema#duration"/>
        <rdfs:comment xml:lang="en">A span of time.</rdfs:comment>
        <schema:domainIncludes rdf:resource="http://iirds.tekom.de/iirds#PlanningTime"/>
        <rdfs:comment xml:lang="de">Dauer</rdfs:comment>
    </rdf:Description>
    <rdf:Description rdf:about="http://iirds.tekom.de/iirds#format">
        <iirds:description xml:lang="en">Cardinality: http://iirds.tekom.de/iirds#Rendition [1]</iirds:description>
        <rdfs:label xml:lang="de">Format</rdfs:label>
        <schema:domainIncludes rdf:resource="http://iirds.tekom.de/iirds#Rendition"/>
        <iirds:description xml:lang="en"></iirds:description>
        <rdfs:comment xml:lang="de">Medientyp (MIME-Type) der Inhaltsausprägung</rdfs:comment>
        <schema:rangeIncludes rdf:resource="http://www.w3.org/2000/01/rdf-schema#Literal"/>
        <rdfs:label xml:lang="en">Format</rdfs:label>
        <rdfs:comment xml:lang="en">Media type (MIME type) of the rendition</rdfs:comment>
    </rdf:Description>
    <rdf:Description rdf:about="http://iirds.tekom.de/iirds#formatRestriction">
        <rdfs:comment xml:lang="en">Restriction to the media formats used in the package.</rdfs:comment>
        <iirds:description xml:lang="en">Value &quot;A&quot; means that the package uses a restricted set of media formats (&quot;iiRDS/A&quot;).</iirds:description>
        <schema:domainIncludes rdf:resource="http://iirds.tekom.de/iirds#Package"/>
        <rdfs:label xml:lang="de">Formateinschränkung</rdfs:label>
        <iirds:description xml:lang="en">Cardinality: http://iirds.tekom.de/iirds#Package [0..1]</iirds:description>
        <rdfs:label xml:lang="en">Format Restriction</rdfs:label>
        <schema:rangeIncludes rdf:resource="http://www.w3.org/2000/01/rdf-schema#Literal"/>
    </rdf:Description>
    <rdf:Description rdf:about="http://iirds.tekom.de/iirds#frequency">
        <rdfs:comment xml:lang="de">Wartungsfrequenz</rdfs:comment>
        <rdfs:label xml:lang="en">Maintenance frequency</rdfs:label>
        <iirds:description xml:lang="en">Cardinality: http://iirds.tekom.de/iirds#MaintenanceInterval [1]</iirds:description>
        <iirds:description xml:lang="en"></iirds:description>
        <rdfs:comment xml:lang="en">Maintenance frequency</rdfs:comment>
        <rdfs:label xml:lang="de">Wartungsfrequenz</rdfs:label>
    </rdf:Description>
    <rdf:Description rdf:about="http://iirds.tekom.de/iirds#has-abstract">
        <schema:domainIncludes rdf:resource="http://iirds.tekom.de/iirds#InformationUnit"/>
        <rdfs:label xml:lang="de">hat Zusammenfassung</rdfs:label>
        <rdfs:label xml:lang="en">has abstract</rdfs:label>
        <iirds:description xml:lang="en"></iirds:description>
        <iirds:description xml:lang="en">Cardinality: http://iirds.tekom.de/iirds#InformationUnit [0..1]</iirds:description>
        <rdfs:comment xml:lang="en">Relates to a literal or information unit that provides an abstract/summary for the information unit.</rdfs:comment>
    </rdf:Description>
    <rdf:Description rdf:about="http://iirds.tekom.de/iirds#has-component">
        <schema:rangeIncludes rdf:resource="http://iirds.tekom.de/iirds#Component"/>
        <rdfs:comment xml:lang="de">Verweist auf eine Kompoente, die Teil einer anderen Komponente ist.</rdfs:comment>
        <iirds:description xml:lang="en">Cardinality: http://iirds.tekom.de/iirds#Component [0..*]</iirds:description>
        <iirds:description xml:lang="en"></iirds:description>
        <rdfs:label xml:lang="de">hat Komponente</rdfs:label>
        <schema:domainIncludes rdf:resource="http://iirds.tekom.de/iirds#Component"/>
        <rdfs:label xml:lang="en">has component</rdfs:label>
        <rdfs:comment xml:lang="en">Relates to a component that is part of another component.</rdfs:comment>
    </rdf:Description>
    <rdf:Description rdf:about="http://iirds.tekom.de/iirds#has-content-lifecycle-status">
        <schema:domainIncludes rdf:resource="http://iirds.tekom.de/iirds#InformationUnit"/>
        <iirds:description xml:lang="en">Cardinality: http://iirds.tekom.de/iirds#InformationUnit [0..*]</iirds:description>
        <rdfs:label xml:lang="de">hat Beziehung zu Bearbeitungsstatus</rdfs:label>
        <iirds:description xml:lang="en"></iirds:description>
        <rdfs:label xml:lang="en">relates to content lifecycle status</rdfs:label>
        <schema:rangeIncludes rdf:resource="http://iirds.tekom.de/iirds#ContentLifeCycleStatus"/>
        <rdfs:comment xml:lang="en">References the content lifecycle status of the information unit.</rdfs:comment>
    </rdf:Description>
    <rdf:Description rdf:about="http://iirds.tekom.de/iirds#has-content-lifecycle-status-value">
        <rdfs:label xml:lang="en">has status value</rdfs:label>
        <iirds:description xml:lang="en">Cardinality: http://iirds.tekom.de/iirds#ContentLifeCycleStatus [1]</iirds:description>
        <rdfs:label xml:lang="de">hat Statuswert</rdfs:label>
        <schema:domainIncludes rdf:resource="http://iirds.tekom.de/iirds#ContentLifeCycleStatus"/>
        <iirds:description xml:lang="en"></iirds:description>
        <rdfs:comment xml:lang="en">References the content lifecycle status value.</rdfs:comment>
        <schema:rangeIncludes rdf:resource="http://iirds.tekom.de/iirds#ContentLifeCycleStatusValue"/>
    </rdf:Description>
    <rdf:Description rdf:about="http://iirds.tekom.de/iirds#has-directory-structure-type">
        <rdfs:comment xml:lang="de">Die Natur des Verzeichnisses</rdfs:comment>
        <rdfs:label xml:lang="de">hat Verzeichnisstrukturtyp</rdfs:label>
        <iirds:description xml:lang="en">Cardinality: http://iirds.tekom.de/iirds#DirectoryNode [0..1]</iirds:description>
        <rdfs:label xml:lang="en">has directory structure type</rdfs:label>
        <schema:rangeIncludes rdf:resource="http://iirds.tekom.de/iirds#DirectoryNodeType"/>
        <iirds:description xml:lang="en"></iirds:description>
        <rdfs:comment xml:lang="en">The nature of the directory.</rdfs:comment>
        <schema:domainIncludes rdf:resource="http://iirds.tekom.de/iirds#DirectoryNode"/>
    </rdf:Description>
    <rdf:Description rdf:about="http://iirds.tekom.de/iirds#has-document-type">
        <iirds:description xml:lang="en">Cardinality: http://iirds.tekom.de/iirds#Document [1..*]</iirds:description>
        <iirds:description xml:lang="en">Documents have one or more document types. Documents without document types are unspecific documents.</iirds:description>
        <rdfs:label xml:lang="de">hat Dokumentart</rdfs:label>
        <schema:domainIncludes rdf:resource="http://iirds.tekom.de/iirds#Document"/>
        <rdfs:label xml:lang="en">has document type</rdfs:label>
        <rdfs:comment xml:lang="en">The type of a document.</rdfs:comment>
        <schema:rangeIncludes rdf:resource="http://iirds.tekom.de/iirds#DocumentType"/>
    </rdf:Description>
    <rdf:Description rdf:about="http://iirds.tekom.de/iirds#has-end-selector">
        <schema:domainIncludes rdf:resource="http://iirds.tekom.de/iirds#RangeSelector"/>
        <iirds:description xml:lang="en">A range selector must reference one start and one end selector.</iirds:description>
        <rdfs:label xml:lang="en">has end selector</rdfs:label>
        <rdfs:label xml:lang="de">hat Endselektor</rdfs:label>
        <rdfs:comment xml:lang="en">References the end of a range in a file.</rdfs:comment>
        <iirds:description xml:lang="en">Cardinality: http://iirds.tekom.de/iirds#RangeSelector [1]</iirds:description>
        <schema:rangeIncludes rdf:resource="http://iirds.tekom.de/iirds#FragmentSelector"/>
    </rdf:Description>
    <rdf:Description rdf:about="http://iirds.tekom.de/iirds#has-event-code">
        <rdfs:label xml:lang="de">hat Ereigniscode</rdfs:label>
        <rdfs:label xml:lang="en">has event code</rdfs:label>
        <schema:domainIncludes rdf:resource="http://iirds.tekom.de/iirds#Event"/>
        <rdfs:comment xml:lang="en">References the code of the event.</rdfs:comment>
        <iirds:description xml:lang="en"></iirds:description>
        <iirds:description xml:lang="en">Cardinality: http://iirds.tekom.de/iirds#Event [0..1]</iirds:description>
    </rdf:Description>
    <rdf:Description rdf:about="http://iirds.tekom.de/iirds#has-event-type">
        <rdfs:label xml:lang="en">has event type</rdfs:label>
        <rdfs:label xml:lang="de">hat Ereignistyp</rdfs:label>
        <iirds:description xml:lang="en"></iirds:description>
        <iirds:description xml:lang="en">Cardinality: http://iirds.tekom.de/iirds#Event [0..1]</iirds:description>
        <rdfs:comment xml:lang="en">References the type of the event.</rdfs:comment>
        <schema:domainIncludes rdf:resource="http://iirds.tekom.de/iirds#Event"/>
    </rdf:Description>
    <rdf:Description rdf:about="http://iirds.tekom.de/iirds#has-first-child">
        <rdfs:label xml:lang="de">hat als erstes Kindelement</rdfs:label>
        <rdfs:label xml:lang="en">has first child</rdfs:label>
        <rdfs:comment xml:lang="de">Verweist auf den ersten Verzeichniseintrag in der nächsten Unterebene.</rdfs:comment>
        <rdfs:comment xml:lang="en">References the first directory node on the next sub level.</rdfs:comment>
        <schema:rangeIncludes rdf:resource="http://iirds.tekom.de/iirds#DirectoryNode"/>
        <iirds:description xml:lang="en">Cardinality: http://iirds.tekom.de/iirds#DirectoryNode [0..1]</iirds:description>
        <schema:domainIncludes rdf:resource="http://iirds.tekom.de/iirds#DirectoryNode"/>
        <iirds:description xml:lang="en"></iirds:description>
    </rdf:Description>
    <rdf:Description rdf:about="http://iirds.tekom.de/iirds#has-identity">
        <rdfs:label xml:lang="de">hat komplexen Identifier</rdfs:label>
        <iirds:description xml:lang="en">Cardinality: http://iirds.tekom.de/iirds#InformationObject [0..*]</iirds:description>
        <schema:domainIncludes rdf:resource="http://iirds.tekom.de/iirds#InformationObject"/>
        <schema:domainIncludes rdf:resource="http://iirds.tekom.de/iirds#Rendition"/>
        <schema:domainIncludes rdf:resource="http://iirds.tekom.de/iirds#ProductVariant"/>
        <iirds:description xml:lang="en">Cardinality: http://iirds.tekom.de/iirds#Rendition [0..*]</iirds:description>
        <iirds:description xml:lang="en">Cardinality: http://iirds.tekom.de/iirds#ProductVariant [0..*]</iirds:description>
        <schema:domainIncludes rdf:resource="http://iirds.tekom.de/iirds#Component"/>
        <schema:rangeIncludes rdf:resource="http://iirds.tekom.de/iirds#Identity"/>
        <rdfs:comment xml:lang="en">References a complex identifier.</rdfs:comment>
        <iirds:description xml:lang="en">Cardinality: http://iirds.tekom.de/iirds#Component [0..*]</iirds:description>
        <iirds:description xml:lang="en">Cardinality: http://iirds.tekom.de/iirds#InformationUnit [0..*]</iirds:description>
        <iirds:description xml:lang="en"></iirds:description>
        <rdfs:label xml:lang="en">has complex identifier</rdfs:label>
        <schema:domainIncludes rdf:resource="http://iirds.tekom.de/iirds#InformationUnit"/>
    </rdf:Description>
    <rdf:Description rdf:about="http://iirds.tekom.de/iirds#has-identity-domain">
        <iirds:description xml:lang="en">Cardinality: http://iirds.tekom.de/iirds#Identity [1]</iirds:description>
        <rdfs:comment xml:lang="en">References the domain that an identifier is valid for.</rdfs:comment>
        <schema:rangeIncludes rdf:resource="http://iirds.tekom.de/iirds#IdentityDomain"/>
        <rdfs:label xml:lang="en">has identifier domain</rdfs:label>
        <iirds:description xml:lang="en"></iirds:description>
        <rdfs:label xml:lang="de">hat Identifier-Domain</rdfs:label>
        <schema:domainIncludes rdf:resource="http://iirds.tekom.de/iirds#Identity"/>
    </rdf:Description>
    <rdf:Description rdf:about="http://iirds.tekom.de/iirds#has-information-type">
        <schema:domainIncludes rdf:resource="http://iirds.tekom.de/iirds#InformationUnit"/>
        <iirds:description xml:lang="en">Not intended to be used directly. Use the child properties instead, such as has-document-type for documents and has-topic-type for topics.</iirds:description>
        <rdfs:label xml:lang="en">has information type</rdfs:label>
        <schema:rangeIncludes rdf:resource="http://iirds.tekom.de/iirds#InformationType"/>
        <rdfs:comment xml:lang="en">The nature and subject of an information unit.</rdfs:comment>
        <rdfs:label xml:lang="de">hat Informationsart</rdfs:label>
        <iirds:description xml:lang="en">Cardinality: http://iirds.tekom.de/iirds#InformationUnit [0..*]</iirds:description>
    </rdf:Description>
    <rdf:Description rdf:about="http://iirds.tekom.de/iirds#has-next-sibling">
        <rdfs:comment xml:lang="de">Verweist auf den folgenden Verzeichniseintrag einer Verzeichnisstruktur auf gleicher Ebene.</rdfs:comment>
        <rdfs:comment xml:lang="en">References the following directory node at the same hierarchy level in a directory structure.</rdfs:comment>
        <schema:rangeIncludes rdf:resource="http://iirds.tekom.de/iirds#DirectoryNode"/>
        <schema:domainIncludes rdf:resource="http://iirds.tekom.de/iirds#DirectoryNode"/>
        <iirds:description xml:lang="en">Cardinality: http://iirds.tekom.de/iirds#DirectoryNode [0..1]</iirds:description>
        <rdfs:label xml:lang="en">has next sibling</rdfs:label>
        <rdfs:label xml:lang="de">hat als nächstes Element</rdfs:label>
        <iirds:description xml:lang="en"></iirds:description>
    </rdf:Description>
    <rdf:Description rdf:about="http://iirds.tekom.de/iirds#has-party-role">
        <iirds:description xml:lang="en">Cardinality: http://iirds.tekom.de/iirds#Party [0..1]</iirds:description>
        <schema:rangeIncludes rdf:resource="http://iirds.tekom.de/iirds#PartyRole"/>
        <iirds:description xml:lang="en"></iirds:description>
        <rdfs:label xml:lang="de">hat administrative Rolle</rdfs:label>
        <rdfs:label xml:lang="en">has administrative role</rdfs:label>
        <rdfs:comment xml:lang="en">References the role that the party has with respect to an entity referencing the party.</rdfs:comment>
        <schema:domainIncludes rdf:resource="http://iirds.tekom.de/iirds#Party"/>
        <rdfs:comment xml:lang="de"></rdfs:comment>
    </rdf:Description>
    <rdf:Description rdf:about="http://iirds.tekom.de/iirds#has-planning-time">
        <iirds:description xml:lang="en"></iirds:description>
        <schema:rangeIncludes rdf:resource="http://iirds.tekom.de/iirds#PlanningTime"/>
        <schema:domainIncludes rdf:resource="http://iirds.tekom.de/iirds#InformationUnit"/>
        <iirds:description xml:lang="en">Cardinality: http://iirds.tekom.de/iirds#InformationUnit [0..*]</iirds:description>
        <rdfs:label xml:lang="en">has time</rdfs:label>
        <rdfs:label xml:lang="de">hat Zeit</rdfs:label>
        <rdfs:comment xml:lang="en">References the planning time that is related to specific tasks or information described in an information unit.</rdfs:comment>
    </rdf:Description>
    <rdf:Description rdf:about="http://iirds.tekom.de/iirds#has-rendition">
        <schema:domainIncludes rdf:resource="http://iirds.tekom.de/iirds#InformationUnit"/>
        <rdfs:label xml:lang="en">has rendition</rdfs:label>
        <rdfs:comment xml:lang="de">Verweist auf eine Inhaltsausprägung einer Informationseinheit.</rdfs:comment>
        <rdfs:label xml:lang="de">hat Inhaltsausprägung</rdfs:label>
        <iirds:description xml:lang="en"></iirds:description>
        <iirds:description xml:lang="en">Cardinality: http://iirds.tekom.de/iirds#InformationUnit [0..*]</iirds:description>
        <rdfs:comment xml:lang="en">Relates to a rendition of an information unit, meaning a physical file with content.</rdfs:comment>
        <schema:rangeIncludes rdf:resource="http://iirds.tekom.de/iirds#Rendition"/>
    </rdf:Description>
    <rdf:Description rdf:about="http://iirds.tekom.de/iirds#has-selector">
        <rdfs:comment xml:lang="en">References the selector that is used to relate the information unit to a physical file with content.</rdfs:comment>
        <iirds:description xml:lang="en">Cardinality: http://iirds.tekom.de/iirds#Rendition [0..1]</iirds:description>
        <schema:rangeIncludes rdf:resource="http://iirds.tekom.de/iirds#Selector"/>
        <schema:domainIncludes rdf:resource="http://iirds.tekom.de/iirds#Rendition"/>
        <rdfs:label xml:lang="de">hat Selektor</rdfs:label>
        <iirds:description xml:lang="en"></iirds:description>
        <rdfs:label xml:lang="en">has selector</rdfs:label>
    </rdf:Description>
    <rdf:Description rdf:about="http://iirds.tekom.de/iirds#has-start-selector">
        <schema:rangeIncludes rdf:resource="http://iirds.tekom.de/iirds#FragmentSelector"/>
        <rdfs:label xml:lang="de">hat Startselektor</rdfs:label>
        <schema:domainIncludes rdf:resource="http://iirds.tekom.de/iirds#RangeSelector"/>
        <iirds:description xml:lang="en">Cardinality: http://iirds.tekom.de/iirds#RangeSelector [1]</iirds:description>
        <rdfs:label xml:lang="en">has start selector</rdfs:label>
        <rdfs:comment xml:lang="en">References the start of a range in a file.</rdfs:comment>
        <iirds:description xml:lang="en">A range selector must reference one start and one end selector.</iirds:description>
    </rdf:Description>
    <rdf:Description rdf:about="http://iirds.tekom.de/iirds#has-subject">
        <schema:domainIncludes rdf:resource="http://iirds.tekom.de/iirds#InformationUnit"/>
        <schema:rangeIncludes rdf:resource="http://iirds.tekom.de/iirds#InformationSubject"/>
        <rdfs:comment xml:lang="en">References the subject of an information unit.</rdfs:comment>
        <rdfs:comment xml:lang="de">Verweist auf das Thema einer Informationseinheit.</rdfs:comment>
        <iirds:description xml:lang="en">Cardinality: http://iirds.tekom.de/iirds#InformationUnit [0..*]</iirds:description>
        <rdfs:label xml:lang="en">has subject</rdfs:label>
        <iirds:description xml:lang="en"></iirds:description>
        <rdfs:label xml:lang="de">hat Thema</rdfs:label>
    </rdf:Description>
    <rdf:Description rdf:about="http://iirds.tekom.de/iirds#has-topic-type">
        <iirds:description xml:lang="en">Cardinality: http://iirds.tekom.de/iirds#InformationUnit [0..*]</iirds:description>
        <schema:rangeIncludes rdf:resource="http://iirds.tekom.de/iirds#TopicType"/>
        <rdfs:label xml:lang="en">has topic type</rdfs:label>
        <rdfs:comment xml:lang="en">The nature of an information unit.</rdfs:comment>
        <rdfs:label xml:lang="de">hat Topictyp</rdfs:label>
        <schema:domainIncludes rdf:resource="http://iirds.tekom.de/iirds#InformationUnit"/>
        <iirds:description xml:lang="en">Defines the information type of a topic, e.g. task or learning.</iirds:description>
    </rdf:Description>
    <rdf:Description rdf:about="http://iirds.tekom.de/iirds#identifier">
        <iirds:description xml:lang="en">Recommended best practice is to identify the resource by means of a string conforming to a formal identification system.</iirds:description>
        <schema:domainIncludes rdf:resource="http://iirds.tekom.de/iirds#Identity"/>
        <iirds:description xml:lang="en">Cardinality: http://iirds.tekom.de/iirds#Identity [1]</iirds:description>
        <schema:rangeIncludes rdf:resource="http://www.w3.org/2000/01/rdf-schema#Literal"/>
        <rdfs:comment xml:lang="en">An unambiguous reference to the resource within a given context.</rdfs:comment>
        <rdfs:label xml:lang="de">Bezeichner</rdfs:label>
        <rdfs:comment xml:lang="de">Eine eindeutige Referenz auf die Resource in einem gegebenen Kontext.</rdfs:comment>
        <rdfs:label xml:lang="en">Identifier</rdfs:label>
    </rdf:Description>
    <rdf:Description rdf:about="http://iirds.tekom.de/iirds#iiRDSVersion">
        <rdfs:label xml:lang="de">iiRDS Version</rdfs:label>
        <schema:rangeIncludes rdf:resource="http://www.w3.org/2000/01/rdf-schema#Literal"/>
        <iirds:description xml:lang="en">Cardinality: http://iirds.tekom.de/iirds#Package [1]</iirds:description>
        <schema:domainIncludes rdf:resource="http://iirds.tekom.de/iirds#Package"/>
        <rdfs:comment xml:lang="de">iiRDS-Version, die das iiRDS-Paket erfüllt.</rdfs:comment>
        <rdfs:label xml:lang="en">iiRDS version</rdfs:label>
        <rdfs:comment xml:lang="en">iiRDS version to which the iiRDS package complies.</rdfs:comment>
        <iirds:description xml:lang="en">Current version is 1.0.</iirds:description>
    </rdf:Description>
    <rdf:Description rdf:about="http://iirds.tekom.de/iirds#iirdsAttribute">
        <rdfs:label xml:lang="de">iirdsAttribute</rdfs:label>
        <rdfs:comment xml:lang="en">Property type. Abstract base class of all properties with literal values.</rdfs:comment>
        <iirds:description xml:lang="en">Not intended to be used directly. Use the subclasses instead.</iirds:description>
        <schema:rangeIncludes rdf:resource="http://www.w3.org/2000/01/rdf-schema#Literal"/>
        <rdfs:label xml:lang="en">iirdsAttribute</rdfs:label>
        <schema:domainIncludes rdf:resource="http://iirds.tekom.de/iirds#iirdsDomainEntity"/>
    </rdf:Description>
    <rdf:Description rdf:about="http://iirds.tekom.de/iirds#iirdsDomainEntity">
        <rdfs:comment xml:lang="de">Eine Entität der iiRDS-Domäne</rdfs:comment>
        <rdfs:label xml:lang="de">iirdsDomainEntity</rdfs:label>
        <rdfs:comment xml:lang="en">An entity of the iiRDS domain</rdfs:comment>
        <rdfs:label xml:lang="en">iirdsDomainEntity</rdfs:label>
        <iirds:description xml:lang="en">Not intended to be used directly. Use the subclasses instead.</iirds:description>
    </rdf:Description>
    <rdf:Description rdf:about="http://iirds.tekom.de/iirds#iirdsRelationConcept">
        <schema:domainIncludes rdf:resource="http://iirds.tekom.de/iirds#iirdsDomainEntity"/>
        <rdfs:label xml:lang="en">iirdsRelationConcept</rdfs:label>
        <rdfs:label xml:lang="de">iirdsRelationConcept</rdfs:label>
        <rdfs:comment xml:lang="en">Base class for all relations in iiRDS.</rdfs:comment>
        <schema:rangeIncludes rdf:resource="http://iirds.tekom.de/iirds#iirdsDomainEntity"/>
        <iirds:description xml:lang="en">Cardinality: http://iirds.tekom.de/iirds#iirdsDomainEntity [0..*]</iirds:description>
        <iirds:description xml:lang="en">Not indented to be used directly.</iirds:description>
    </rdf:Description>
    <rdf:Description rdf:about="http://iirds.tekom.de/iirds#is-applicable-for-document-type">
        <iirds:description xml:lang="en">Example: topics that are suitable for the installation instructions.</iirds:description>
        <rdfs:label xml:lang="de">geeignet für Dokumentart</rdfs:label>
        <schema:rangeIncludes rdf:resource="http://iirds.tekom.de/iirds#DocumentType"/>
        <schema:domainIncludes rdf:resource="http://iirds.tekom.de/iirds#InformationUnit"/>
        <iirds:description xml:lang="en">Cardinality: http://iirds.tekom.de/iirds#InformationUnit [0..*]</iirds:description>
        <rdfs:comment xml:lang="en">Specifies that the information unit is suitable and can be used for specific types of documents.</rdfs:comment>
        <rdfs:label xml:lang="en">applicable for document type</rdfs:label>
    </rdf:Description>
    <rdf:Description rdf:about="http://iirds.tekom.de/iirds#is-part-of-package">
        <rdfs:label xml:lang="de">ist Teil von Paket</rdfs:label>
        <iirds:description xml:lang="en"></iirds:description>
        <iirds:description xml:lang="en">Cardinality: http://iirds.tekom.de/iirds#InformationUnit [0..*]</iirds:description>
        <rdfs:comment xml:lang="en">References the package in which the information unit was delivered.</rdfs:comment>
        <schema:domainIncludes rdf:resource="http://iirds.tekom.de/iirds#InformationUnit"/>
        <schema:rangeIncludes rdf:resource="http://iirds.tekom.de/iirds#Package"/>
        <rdfs:label xml:lang="en">is part of package</rdfs:label>
    </rdf:Description>
    <rdf:Description rdf:about="http://iirds.tekom.de/iirds#is-replacement-of">
        <schema:rangeIncludes rdf:resource="http://iirds.tekom.de/iirds#InformationUnit"/>
        <rdfs:label xml:lang="de">ersetzt</rdfs:label>
        <rdfs:comment xml:lang="en">References the information unit that is replaced by this information unit.</rdfs:comment>
        <rdfs:label xml:lang="en">replaces</rdfs:label>
        <iirds:description xml:lang="en"></iirds:description>
        <iirds:description xml:lang="en">Cardinality: http://iirds.tekom.de/iirds#InformationUnit [0..1]</iirds:description>
        <schema:domainIncludes rdf:resource="http://iirds.tekom.de/iirds#InformationUnit"/>
    </rdf:Description>
    <rdf:Description rdf:about="http://iirds.tekom.de/iirds#is-version-of">
        <iirds:description xml:lang="en">Specifies that the information unit is a version or language variant of the information object.</iirds:description>
        <schema:rangeIncludes rdf:resource="http://iirds.tekom.de/iirds#InformationObject"/>
        <rdfs:comment xml:lang="en">Relates an information unit to an information object.</rdfs:comment>
        <rdfs:label xml:lang="en">is version of</rdfs:label>
        <schema:domainIncludes rdf:resource="http://iirds.tekom.de/iirds#InformationUnit"/>
        <rdfs:label xml:lang="de">ist Version von</rdfs:label>
        <iirds:description xml:lang="en">Cardinality: http://iirds.tekom.de/iirds#InformationUnit [0..1]</iirds:description>
    </rdf:Description>
    <rdf:Description rdf:about="http://iirds.tekom.de/iirds#language">
        <iirds:description xml:lang="en">Cardinality: http://iirds.tekom.de/iirds#InformationUnit [0..*]</iirds:description>
        <rdfs:label xml:lang="de">Sprache</rdfs:label>
        <iirds:description xml:lang="en">Controlled vocabulary according to RFC 4646.</iirds:description>
        <schema:domainIncludes rdf:resource="http://iirds.tekom.de/iirds#InformationUnit"/>
        <schema:rangeIncludes rdf:resource="http://www.w3.org/2000/01/rdf-schema#Literal"/>
        <rdfs:label xml:lang="en">Language</rdfs:label>
        <rdfs:comment xml:lang="en">A language of the resource.</rdfs:comment>
    </rdf:Description>
    <rdf:Description rdf:about="http://iirds.tekom.de/iirds#nil">
        <rdfs:label xml:lang="en">End of Directory node</rdfs:label>
        <rdfs:comment xml:lang="de">Das Ende in einer verketteten Liste von Verzeichnisknoten </rdfs:comment>
        <iirds:description xml:lang="en"></iirds:description>
        <rdfs:label xml:lang="de">Ende einer Verzeichnisstruktur</rdfs:label>
        <rdfs:comment xml:lang="en">The end in a chain of directory nodes</rdfs:comment>
    </rdf:Description>
    <rdf:Description rdf:about="http://iirds.tekom.de/iirds#purpose">
        <iirds:description xml:lang="en"></iirds:description>
        <schema:domainIncludes rdf:resource="http://iirds.tekom.de/iirds#ContentLifeCycleStatus"/>
        <rdfs:comment xml:lang="en">Specifies the reason for changing the content lifecycle status.</rdfs:comment>
        <schema:rangeIncludes rdf:resource="http://www.w3.org/2000/01/rdf-schema#Literal"/>
        <iirds:description xml:lang="en">Cardinality: http://iirds.tekom.de/iirds#ContentLifeCycleStatus [0..1]</iirds:description>
        <rdfs:comment xml:lang="de">Begründung zum Ausüben der Statusänderung.</rdfs:comment>
        <rdfs:label xml:lang="en">Purpose</rdfs:label>
        <rdfs:label xml:lang="de">Zweck</rdfs:label>
    </rdf:Description>
    <rdf:Description rdf:about="http://iirds.tekom.de/iirds#relates-to-administrative-metadata">
        <rdfs:comment xml:lang="en">Relates an iiRDS entity to administrative metadata.</rdfs:comment>
        <rdfs:label xml:lang="en">relates to administrative metadata</rdfs:label>
        <schema:domainIncludes rdf:resource="http://iirds.tekom.de/iirds#iirdsDomainEntity"/>
        <rdfs:comment xml:lang="de">Setzt eine iiRDS Entität in Beziehung mit administrativen Metadaten.</rdfs:comment>
        <iirds:description xml:lang="en">Cardinality: http://iirds.tekom.de/iirds#iirdsDomainEntity [0..*]</iirds:description>
        <rdfs:comment xml:lang="de">Erzeugt Beziehung von einer iiRDS-Entität zu administrativen Metadaten.</rdfs:comment>
        <rdfs:label xml:lang="de">bezieht sich auf administrative Metadaten</rdfs:label>
        <iirds:description xml:lang="en">Not intended to be used directly. Use the subclasses instead.</iirds:description>
        <schema:rangeIncludes rdf:resource="http://iirds.tekom.de/iirds#AdministrativeMetadata"/>
    </rdf:Description>
    <rdf:Description rdf:about="http://iirds.tekom.de/iirds#relates-to-component">
        <rdfs:label xml:lang="de">bezieht sich auf Komponente</rdfs:label>
        <iirds:description xml:lang="en">Cardinality: http://iirds.tekom.de/iirds#InformationUnit [0..*]</iirds:description>
        <schema:rangeIncludes rdf:resource="http://iirds.tekom.de/iirds#Component"/>
        <iirds:description xml:lang="en">That means that the content of the information unit relates to a specific component of the documented product or component.</iirds:description>
        <schema:domainIncludes rdf:resource="http://iirds.tekom.de/iirds#InformationUnit"/>
        <rdfs:comment xml:lang="en">Relates to a component.</rdfs:comment>
        <rdfs:label xml:lang="en">relates to component</rdfs:label>
    </rdf:Description>
    <rdf:Description rdf:about="http://iirds.tekom.de/iirds#relates-to-event">
        <rdfs:label xml:lang="de">bezieht sich auf Ereignis</rdfs:label>
        <rdfs:comment xml:lang="en">Relates to an event.</rdfs:comment>
        <iirds:description xml:lang="en">That means that the content of the information unit refers to a specific event that occured in the product/system, e.g. an error.</iirds:description>
        <iirds:description xml:lang="en">Cardinality: http://iirds.tekom.de/iirds#InformationUnit [0..*]</iirds:description>
        <schema:rangeIncludes rdf:resource="http://iirds.tekom.de/iirds#Event"/>
        <schema:domainIncludes rdf:resource="http://iirds.tekom.de/iirds#InformationUnit"/>
        <rdfs:label xml:lang="en">relates to event</rdfs:label>
    </rdf:Description>
    <rdf:Description rdf:about="http://iirds.tekom.de/iirds#relates-to-functional-metadata">
        <schema:rangeIncludes rdf:resource="http://iirds.tekom.de/iirds#FunctionalMetadata"/>
        <rdfs:comment xml:lang="en">Relates an iiRDS entity to functional metadata.</rdfs:comment>
        <rdfs:label xml:lang="en">relates to functional metadata</rdfs:label>
        <rdfs:comment xml:lang="de">Erzeugt Beziehung von einer iiRDS-Entität zu funktionalen Metadaten.</rdfs:comment>
        <rdfs:label xml:lang="de">bezieht sich auf funktionale Metadaten</rdfs:label>
        <iirds:description xml:lang="en">No intended to be used directly. Use the subclasses instead.</iirds:description>
        <schema:domainIncludes rdf:resource="http://iirds.tekom.de/iirds#InformationUnit"/>
        <iirds:description xml:lang="en">Cardinality: http://iirds.tekom.de/iirds#InformationUnit [0..*]</iirds:description>
    </rdf:Description>
    <rdf:Description rdf:about="http://iirds.tekom.de/iirds#relates-to-information-unit">
        <rdfs:comment xml:lang="en">References an information unit from a directory node.</rdfs:comment>
        <schema:domainIncludes rdf:resource="http://iirds.tekom.de/iirds#DirectoryNode"/>
        <schema:rangeIncludes rdf:resource="http://iirds.tekom.de/iirds#InformationUnit"/>
        <iirds:description xml:lang="en">Cardinality: http://iirds.tekom.de/iirds#InformationUnit [0..1]</iirds:description>
        <rdfs:label xml:lang="de">referenziert Informationseinheit</rdfs:label>
        <rdfs:label xml:lang="en">references information unit</rdfs:label>
        <iirds:description xml:lang="en">The referenced information unit is part of the directory.</iirds:description>
    </rdf:Description>
    <rdf:Description rdf:about="http://iirds.tekom.de/iirds#relates-to-party">
        <schema:domainIncludes rdf:resource="http://iirds.tekom.de/iirds#InformationUnit"/>
        <rdfs:label xml:lang="en">relates to party</rdfs:label>
        <schema:domainIncludes rdf:resource="http://iirds.tekom.de/iirds#ContentLifeCycleStatus"/>
        <iirds:description xml:lang="en">Cardinality: http://iirds.tekom.de/iirds#Component [0..1]</iirds:description>
        <iirds:description xml:lang="en">Cardinality: http://iirds.tekom.de/iirds#InformationUnit [0..1]</iirds:description>
        <iirds:description xml:lang="en"></iirds:description>
        <rdfs:comment xml:lang="en">Relates to a party, e.g. a company or an organization.</rdfs:comment>
        <schema:domainIncludes rdf:resource="http://iirds.tekom.de/iirds#Component"/>
        <schema:rangeIncludes rdf:resource="http://iirds.tekom.de/iirds#Party"/>
        <iirds:description xml:lang="en">Cardinality: http://iirds.tekom.de/iirds#ContentLifeCycleStatus [0..1]</iirds:description>
        <iirds:description xml:lang="en">Cardinality: http://iirds.tekom.de/iirds#ProductVariant [0..1]</iirds:description>
        <schema:domainIncludes rdf:resource="http://iirds.tekom.de/iirds#IdentityDomain"/>
        <schema:domainIncludes rdf:resource="http://iirds.tekom.de/iirds#ProductVariant"/>
        <iirds:description xml:lang="en">Cardinality: http://iirds.tekom.de/iirds#IdentityDomain [0..1]</iirds:description>
        <rdfs:label xml:lang="de">hat Beziehung zu Akteur</rdfs:label>
    </rdf:Description>
    <rdf:Description rdf:about="http://iirds.tekom.de/iirds#relates-to-product-feature">
        <iirds:description xml:lang="en">Cardinality: http://iirds.tekom.de/iirds#InformationUnit [0..*]</iirds:description>
        <rdfs:label xml:lang="de">bezieht sich auf Produkteigenschaft</rdfs:label>
        <rdfs:label xml:lang="en">relates to product feature</rdfs:label>
        <schema:domainIncludes rdf:resource="http://iirds.tekom.de/iirds#InformationUnit"/>
        <iirds:description xml:lang="en">That means that the content of the information unit refers to or describes a specific product feature.</iirds:description>
        <rdfs:comment xml:lang="en">Relates to a product feature.</rdfs:comment>
        <schema:rangeIncludes rdf:resource="http://iirds.tekom.de/iirds#ProductFeature"/>
    </rdf:Description>
    <rdf:Description rdf:about="http://iirds.tekom.de/iirds#relates-to-product-lifecycle-phase">
        <rdfs:label xml:lang="de">bezieht sich auf Produktlebenszyklusphase</rdfs:label>
        <rdfs:comment xml:lang="en">Relates to a product lifecycle phase.</rdfs:comment>
        <schema:rangeIncludes rdf:resource="http://iirds.tekom.de/iirds#ProductLifeCyclePhase"/>
        <iirds:description xml:lang="en">Cardinality: http://iirds.tekom.de/iirds#InformationUnit [0..*]</iirds:description>
        <iirds:description xml:lang="en">That means that the content of the information unit describes activities or knowledge related to a specific lifecycle phase. Examples are operation and maintenance.</iirds:description>
        <schema:domainIncludes rdf:resource="http://iirds.tekom.de/iirds#InformationUnit"/>
        <rdfs:label xml:lang="en">relates to phase of the product lifecycle</rdfs:label>
    </rdf:Description>
    <rdf:Description rdf:about="http://iirds.tekom.de/iirds#relates-to-product-metadata">
        <rdfs:label xml:lang="de">bezieht sich auf Produktmetadaten</rdfs:label>
        <schema:domainIncludes rdf:resource="http://iirds.tekom.de/iirds#InformationUnit"/>
        <iirds:description xml:lang="en">Cardinality: http://iirds.tekom.de/iirds#InformationUnit [0..*]</iirds:description>
        <rdfs:label xml:lang="en">relates to product metadata</rdfs:label>
        <iirds:description xml:lang="en"></iirds:description>
        <schema:rangeIncludes rdf:resource="http://iirds.tekom.de/iirds#ProductMetadata"/>
        <rdfs:comment xml:lang="en">Relates to product metadata.</rdfs:comment>
    </rdf:Description>
    <rdf:Description rdf:about="http://iirds.tekom.de/iirds#relates-to-product-variant">
        <iirds:description xml:lang="en">Cardinality: http://iirds.tekom.de/iirds#InformationUnit [0..*]</iirds:description>
        <rdfs:label xml:lang="de">bezieht sich auf Produktvariante</rdfs:label>
        <rdfs:comment xml:lang="en">Relates to product variant.</rdfs:comment>
        <schema:domainIncludes rdf:resource="http://iirds.tekom.de/iirds#InformationUnit"/>
        <rdfs:label xml:lang="en">relates to product variant</rdfs:label>
        <schema:rangeIncludes rdf:resource="http://iirds.tekom.de/iirds#ProductVariant"/>
        <iirds:description xml:lang="en">That means that the content of the information unit refers to or describes a specific variant of the product.</iirds:description>
    </rdf:Description>
    <rdf:Description rdf:about="http://iirds.tekom.de/iirds#relates-to-qualification">
        <rdfs:label xml:lang="de">bezieht sich auf Qualifikation</rdfs:label>
        <rdfs:comment xml:lang="en">Relates to a qualification that is required for the tasks or activities described in the information unit.</rdfs:comment>
        <iirds:description xml:lang="en"></iirds:description>
        <schema:rangeIncludes rdf:resource="http://iirds.tekom.de/iirds#Qualification"/>
        <rdfs:label xml:lang="en">relates to qualification</rdfs:label>
        <iirds:description xml:lang="en">Cardinality: http://iirds.tekom.de/iirds#InformationUnit [0..*]</iirds:description>
        <schema:domainIncludes rdf:resource="http://iirds.tekom.de/iirds#InformationUnit"/>
    </rdf:Description>
    <rdf:Description rdf:about="http://iirds.tekom.de/iirds#relates-to-supply">
        <rdfs:comment xml:lang="en">Relates to a supply that is required for the tasks or activities described in the information unit.</rdfs:comment>
        <schema:rangeIncludes rdf:resource="http://iirds.tekom.de/iirds#Supply"/>
        <iirds:description xml:lang="en"></iirds:description>
        <schema:domainIncludes rdf:resource="http://iirds.tekom.de/iirds#InformationUnit"/>
        <rdfs:label xml:lang="de">bezieht sich auf Hilfsmittel</rdfs:label>
        <iirds:description xml:lang="en">Cardinality: http://iirds.tekom.de/iirds#InformationUnit [0..*]</iirds:description>
        <rdfs:label xml:lang="en">relates to supply</rdfs:label>
    </rdf:Description>
    <rdf:Description rdf:about="http://iirds.tekom.de/iirds#relates-to-vcard">
        <rdfs:label xml:lang="en">relates to vCard</rdfs:label>
        <iirds:description xml:lang="en">Cardinality: http://iirds.tekom.de/iirds#Party [0..1]</iirds:description>
        <rdfs:comment xml:lang="en">Relates to a vCard providing detailed information about the party.</rdfs:comment>
        <schema:rangeIncludes rdf:resource="http://www.w3.org/2006/vcard/ns#Kind"/>
        <rdfs:label xml:lang="de">bezieht sich auf vCard</rdfs:label>
        <schema:domainIncludes rdf:resource="http://iirds.tekom.de/iirds#Party"/>
        <iirds:description xml:lang="en"></iirds:description>
    </rdf:Description>
    <rdf:Description rdf:about="http://iirds.tekom.de/iirds#revision">
        <schema:domainIncludes rdf:resource="http://iirds.tekom.de/iirds#InformationUnit"/>
        <schema:rangeIncludes rdf:resource="http://www.w3.org/2000/01/rdf-schema#Literal"/>
        <rdfs:label xml:lang="de">Revision</rdfs:label>
        <rdfs:comment xml:lang="en">Version of the information unit.</rdfs:comment>
        <iirds:description xml:lang="en">Cardinality: http://iirds.tekom.de/iirds#InformationUnit [0..1]</iirds:description>
        <iirds:description xml:lang="en"></iirds:description>
        <rdfs:label xml:lang="en">Revision</rdfs:label>
    </rdf:Description>
    <rdf:Description rdf:about="http://iirds.tekom.de/iirds#rights">
        <schema:domainIncludes rdf:resource="http://iirds.tekom.de/iirds#InformationUnit"/>
        <iirds:description xml:lang="en"></iirds:description>
        <rdfs:label xml:lang="en">Rights</rdfs:label>
        <iirds:description xml:lang="en">Cardinality: http://iirds.tekom.de/iirds#InformationUnit [0..*]</iirds:description>
        <rdfs:label xml:lang="de">Rechte</rdfs:label>
        <rdfs:comment xml:lang="en">Information about rights held in and over the resource.</rdfs:comment>
        <schema:rangeIncludes rdf:resource="http://www.w3.org/2000/01/rdf-schema#Literal"/>
    </rdf:Description>
    <rdf:Description rdf:about="http://iirds.tekom.de/iirds#source">
        <iirds:description xml:lang="en">Cardinality: http://iirds.tekom.de/iirds#Rendition [1]</iirds:description>
        <iirds:description xml:lang="de">The path is relative to the root directory of the package, e.g., &quot;content/overview.html&quot;.</iirds:description>
        <rdfs:label xml:lang="de">Quelle</rdfs:label>
        <schema:rangeIncludes rdf:resource="http://www.w3.org/2000/01/rdf-schema#Literal"/>
        <rdfs:comment xml:lang="en">Relative path to the file containing the content of a rendition.</rdfs:comment>
        <rdfs:label xml:lang="en">Source</rdfs:label>
        <schema:domainIncludes rdf:resource="http://iirds.tekom.de/iirds#Rendition"/>
    </rdf:Description>
    <rdf:Description rdf:about="http://iirds.tekom.de/iirds#statusComment">
        <iirds:description xml:lang="en">Cardinality: http://iirds.tekom.de/iirds#ContentLifeCycleStatus [0..*]</iirds:description>
        <iirds:description xml:lang="en"></iirds:description>
        <rdfs:label xml:lang="de">Kommentar zum Status</rdfs:label>
        <schema:domainIncludes rdf:resource="http://iirds.tekom.de/iirds#ContentLifeCycleStatus"/>
        <rdfs:comment xml:lang="en">Comment describing the status change.</rdfs:comment>
        <rdfs:comment xml:lang="de">Anmerkungen im Zusammenhang mit der Vergabe des Status</rdfs:comment>
        <schema:rangeIncludes rdf:resource="http://www.w3.org/2000/01/rdf-schema#Literal"/>
        <rdfs:label xml:lang="en">Status comment</rdfs:label>
    </rdf:Description>
    <rdf:Description rdf:about="http://iirds.tekom.de/iirds#synonym">
        <schema:domainIncludes rdf:resource="http://iirds.tekom.de/iirds#iirdsDomainEntity"/>
        <rdfs:label xml:lang="en">Synonym</rdfs:label>
        <iirds:description xml:lang="en"></iirds:description>
        <rdfs:comment xml:lang="en">A word or phrase that means exactly or nearly the same as another word or phrase in the same language.</rdfs:comment>
        <rdfs:label xml:lang="de">Synonym</rdfs:label>
        <iirds:description xml:lang="en">Cardinality: http://iirds.tekom.de/iirds#iirdsDomainEntity [0..*]</iirds:description>
        <schema:rangeIncludes rdf:resource="http://www.w3.org/2000/01/rdf-schema#Literal"/>
    </rdf:Description>
    <rdf:Description rdf:about="http://iirds.tekom.de/iirds#title">
        <iirds:description xml:lang="en">Cardinality: http://iirds.tekom.de/iirds#InformationUnit [0..1]</iirds:description>
        <schema:domainIncludes rdf:resource="http://iirds.tekom.de/iirds#InformationUnit"/>
        <schema:rangeIncludes rdf:resource="http://www.w3.org/2000/01/rdf-schema#Literal"/>
        <rdfs:label xml:lang="en">Title</rdfs:label>
        <rdfs:label xml:lang="de">Titel</rdfs:label>
        <rdfs:comment xml:lang="en">A name given to the information unit.</rdfs:comment>
        <iirds:description xml:lang="en">Typically, a title will be a name by which the information unit is formally known.</iirds:description>
    </rdf:Description>
    <rdf:Description rdf:about="http://www.w3.org/2003/01/geo/wgs84_pos#">
        <dc:date>$Date: 2009/04/20 15:00:30 $</dc:date>
        <rdfs:label>geo</rdfs:label>
        <dc:description>A vocabulary for representing latitude, longitude and 
 altitude information in the WGS84 geodetic reference datum. 
 Version $Id: wgs84_pos.rdf,v 1.22 2009/04/20 15:00:30 timbl Exp $. See http://www.w3.org/2003/01/geo/ for more details.</dc:description>
        <rdfs:comment>
Recent changes to this namespace:
$Log: wgs84_pos.rdf,v $
Revision 1.22  2009/04/20 15:00:30  timbl
Remove the time bits which have been deal with elsewhere eg in iCal.

Revision 1.21  2009/04/20 12:52:47  timbl
try again

Revision 1.20  2009/04/20 12:42:11  timbl
Add Event (edited ages ago and never checked in), and location (following discussion http://chatlogs.planetrdf.com/swig/2009-04-20#T12-36-09)

Revision 1.19  2009/04/20 12:36:31  timbl
Add Event (edited ages ago and never checked in), and location (following discussion http://chatlogs.planetrdf.com/swig/2009-04-20#T12-36-09)

Revision 1.18  2006/02/01 22:01:04  danbri
Clarified that lat and long are decimal degrees, and that alt is decimal metres about local reference ellipsoid

Revision 1.17  2004/02/06 17:38:12  danbri
Fixed a bad commit screwup

Revision 1.15  2003/04/19 11:24:08  danbri
Fixed the typo even more.

Revision 1.14  2003/04/19 11:16:56  danbri
fixed a typo

Revision 1.13  2003/02/19 22:27:27  connolly
relaxed domain constraints on lat/long/alt from Point to SpatialThing

Revision 1.12  2003/01/12 01:41:41  danbri
Trying local copy of XSLT doc.

Revision 1.11  2003/01/12 01:20:18  danbri
added a link to morten&apos;s xslt rdfs viewer.

Revision 1.10  2003/01/11 18:56:49  danbri
Removed datatype range from lat and long properties, since they would
have required each occurance of the property to mention the datatype.

Revision 1.9  2003/01/11 11:41:31  danbri
Another typo; repaired rdfs:Property to rdf:Property x4

Revision 1.8  2003/01/11 11:05:02  danbri
Added an rdfs:range for each lat/long/alt property,
http://www.w3.org/2001/XMLSchema#float

Revision 1.7  2003/01/10 20:25:16  danbri
Longer rdfs:comment for Point, trying to be Earth-centric and neutral about
coordinate system(s) at the same time. Feedback welcomed.

Revision 1.6  2003/01/10 20:18:30  danbri
Added CVS log comments into the RDF/XML as an rdfs:comment property of the
vocabulary. Note that this is not common practice (but seems both harmless
and potentially useful).


revision 1.5
date: 2003/01/10 20:14:31;  author: danbri;  state: Exp;  lines: +16 -5
Updated schema:
Added a dc:date, added url for more info. Changed the rdfs:label of the
namespace from gp to geo. Added a class Point, set as the rdfs:domain of
each property. Added XML comment on the lat_long property suggesting that
we might not need it (based on #rdfig commentary from implementors).

revision 1.4
date: 2003/01/10 20:01:07;  author: danbri;  state: Exp;  lines: +6 -5
Fixed typo; several rdfs:about attributes are now rdf:about. Thanks to MortenF in
#rdfig for catching this error.

revision 1.3
date: 2003/01/10 11:59:03;  author: danbri;  state: Exp;  lines: +4 -3
fixed buglet in vocab, added more wgs links

revision 1.2
date: 2003/01/10 11:01:11;  author: danbri;  state: Exp;  lines: +4 -4
Removed alt from the as-a-flat-string property, and switched from
space separated to comma separated.

revision 1.1
date: 2003/01/10 10:53:23;  author: danbri;  state: Exp;
basic geo vocab

</rdfs:comment>
        <dc:title>WGS84 Geo Positioning: an RDF vocabulary</dc:title>
    </rdf:Description>
    <rdf:Description rdf:about="http://www.w3.org/2003/01/geo/wgs84_pos#lat_long">
        <rdfs:comment>A comma-separated representation of a latitude, longitude coordinate.</rdfs:comment>
        <rdfs:label>lat/long</rdfs:label>
    </rdf:Description>
    <rdf:Description rdf:about="http://www.w3.org/2003/01/geo/wgs84_pos#location">
        <rdfs:label>location</rdfs:label>
        <rdfs:comment>The relation between something and the point, 
 or other geometrical thing in space, where it is.  For example, the realtionship between
 a radio tower and a Point with a given lat and long.
 Or a relationship between a park and its outline as a closed arc of points, or a road and
 its location as a arc (a sequence of points).
 Clearly in practice there will be limit to the accuracy of any such statement, but one would expect
 an accuracy appropriate for the size of the object and uses such as mapping .
 </rdfs:comment>
    </rdf:Description>
</rdf:RDF>



<!-- Generated by the OWL API (version 4.5.7.2018-12-02T02:23:35Z) https://github.com/owlcs/owlapi -->

